@prefix : <http://purl.org/ontology/mo/> .
@prefix ao: <http://purl.org/ontology/ao/core#> .
@prefix cc: <http://web.resource.org/cc/> .
@prefix dc: <http://purl.org/dc/elements/1.1/> .
@prefix mo: <http://purl.org/ontology/mo/> .
@prefix vs: <http://www.w3.org/2003/06/sw-vocab-status/ns#> .
@prefix bio: <http://purl.org/vocab/bio/0.1/> .
@prefix geo: <http://www.w3.org/2003/01/geo/wgs84_pos#> .
@prefix owl: <http://www.w3.org/2002/07/owl#> .
@prefix rdf: <http://www.w3.org/1999/02/22-rdf-syntax-ns#> .
@prefix wot: <http://xmlns.com/wot/0.1/> .
@prefix xml: <http://www.w3.org/XML/1998/namespace> .
@prefix xsd: <http://www.w3.org/2001/XMLSchema#> .
@prefix foaf: <http://xmlns.com/foaf/0.1/> .
@prefix frbr: <http://purl.org/vocab/frbr/core#> .
@prefix keys: <http://purl.org/NET/c4dm/keys.owl#> .
@prefix rdfs: <http://www.w3.org/2000/01/rdf-schema#> .
@prefix time: <http://www.w3.org/2006/time#> .
@prefix vann: <http://purl.org/vocab/vann/> .
@prefix event: <http://purl.org/NET/c4dm/event.owl#> .
@prefix dcterms: <http://purl.org/dc/terms/> .
@base <http://purl.org/ontology/mo/> .

<http://purl.org/ontology/mo/> rdf:type owl:Ontology ;
                                owl:imports <http://purl.org/NET/c4dm/keys.owl> ,
                                            bio: ,
                                            <http://www.w3.org/2006/time> ,
                                            <http://purl.org/NET/c4dm/event.owl> ,
                                            <http://purl.org/ontology/ao/core> ,
                                            <http://purl.org/vocab/frbr/core> ,
                                            foaf: ;
                                vann:preferredNamespacePrefix "mo" ;
                                vann:preferredNamespaceUri "http://purl.org/ontology/mo/" ;
                                dc:description """
        The Music Ontology Specification provides main concepts and 
        properties fo describing music (i.e. artists, albums and tracks) 
        on the Semantic Web. 
    """ ;
                                owl:versionInfo "Revision: 2.1.5" ;
                                dc:created "2006/12/21 12:00:00" ;
                                dc:title "The Music Ontology" ;
                                dc:date "2013/07/22 16:54:19" .

#################################################################
#    Annotation properties
#################################################################

###  http://purl.org/dc/terms/abstract
dcterms:abstract rdfs:subPropertyOf dc:description ,
                                    dcterms:description .


###  http://purl.org/dc/terms/accessRights
dcterms:accessRights rdfs:subPropertyOf dc:rights .


###  http://purl.org/dc/terms/alternative
dcterms:alternative rdfs:subPropertyOf dc:title .


###  http://purl.org/dc/terms/available
dcterms:available rdfs:subPropertyOf dc:date .


###  http://purl.org/dc/terms/bibliographicCitation
dcterms:bibliographicCitation rdfs:subPropertyOf dc:identifier .


###  http://purl.org/dc/terms/conformsTo
dcterms:conformsTo rdfs:subPropertyOf dc:relation ,
                                      dcterms:relation .


###  http://purl.org/dc/terms/contributor
dcterms:contributor rdfs:subPropertyOf dc:contributor .


###  http://purl.org/dc/terms/coverage
dcterms:coverage rdfs:subPropertyOf dc:coverage .


###  http://purl.org/dc/terms/created
dcterms:created rdfs:subPropertyOf dc:date .


###  http://purl.org/dc/terms/creator
dcterms:creator rdfs:subPropertyOf dc:creator .


###  http://purl.org/dc/terms/date
dcterms:date rdfs:subPropertyOf dc:date .


###  http://purl.org/dc/terms/dateAccepted
dcterms:dateAccepted rdfs:subPropertyOf dc:date .


###  http://purl.org/dc/terms/dateCopyrighted
dcterms:dateCopyrighted rdfs:subPropertyOf dc:date .


###  http://purl.org/dc/terms/dateSubmitted
dcterms:dateSubmitted rdfs:subPropertyOf dc:date .


###  http://purl.org/dc/terms/description
dcterms:description rdfs:subPropertyOf dc:description .


###  http://purl.org/dc/terms/extent
dcterms:extent rdfs:subPropertyOf dc:format .


###  http://purl.org/dc/terms/format
dcterms:format rdfs:subPropertyOf dc:format .


###  http://purl.org/dc/terms/hasFormat
dcterms:hasFormat rdfs:subPropertyOf dc:relation ,
                                     dcterms:relation .


###  http://purl.org/dc/terms/hasPart
dcterms:hasPart rdfs:subPropertyOf dc:relation ,
                                   dcterms:relation .


###  http://purl.org/dc/terms/hasVersion
dcterms:hasVersion rdfs:subPropertyOf dc:relation ,
                                      dcterms:relation .


###  http://purl.org/dc/terms/identifier
dcterms:identifier rdfs:subPropertyOf dc:identifier .


###  http://purl.org/dc/terms/isFormatOf
dcterms:isFormatOf rdfs:subPropertyOf dc:relation ,
                                      dcterms:relation .


###  http://purl.org/dc/terms/isPartOf
dcterms:isPartOf rdfs:subPropertyOf dc:relation ,
                                    dcterms:relation .


###  http://purl.org/dc/terms/isReferencedBy
dcterms:isReferencedBy rdfs:subPropertyOf dc:relation ,
                                          dcterms:relation .


###  http://purl.org/dc/terms/isReplacedBy
dcterms:isReplacedBy rdfs:subPropertyOf dc:relation ,
                                        dcterms:relation .


###  http://purl.org/dc/terms/isRequiredBy
dcterms:isRequiredBy rdfs:subPropertyOf dc:relation ,
                                        dcterms:relation .


###  http://purl.org/dc/terms/isVersionOf
dcterms:isVersionOf rdfs:subPropertyOf dc:relation ,
                                       dcterms:relation .


###  http://purl.org/dc/terms/issued
dcterms:issued rdfs:subPropertyOf dc:date .


###  http://purl.org/dc/terms/language
dcterms:language rdfs:subPropertyOf dc:language .


###  http://purl.org/dc/terms/license
dcterms:license rdfs:subPropertyOf dc:rights .


###  http://purl.org/dc/terms/medium
dcterms:medium rdfs:subPropertyOf dc:format .


###  http://purl.org/dc/terms/modified
dcterms:modified rdfs:subPropertyOf dc:date .


###  http://purl.org/dc/terms/publisher
dcterms:publisher rdfs:subPropertyOf dc:publisher .


###  http://purl.org/dc/terms/references
dcterms:references rdfs:subPropertyOf dc:relation ,
                                      dcterms:relation .


###  http://purl.org/dc/terms/relation
dcterms:relation rdfs:subPropertyOf dc:relation .


###  http://purl.org/dc/terms/replaces
dcterms:replaces rdfs:subPropertyOf dc:relation ,
                                    dcterms:relation .


###  http://purl.org/dc/terms/requires
dcterms:requires rdfs:subPropertyOf dc:relation ,
                                    dcterms:relation .


###  http://purl.org/dc/terms/rights
dcterms:rights rdfs:subPropertyOf dc:rights .


###  http://purl.org/dc/terms/source
dcterms:source rdfs:subPropertyOf dc:source ,
                                  dcterms:relation .


###  http://purl.org/dc/terms/spatial
dcterms:spatial rdfs:subPropertyOf dc:coverage .


###  http://purl.org/dc/terms/subject
dcterms:subject rdfs:subPropertyOf dc:subject .


###  http://purl.org/dc/terms/tableOfContents
dcterms:tableOfContents rdfs:subPropertyOf dc:description ,
                                           dcterms:description .


###  http://purl.org/dc/terms/temporal
dcterms:temporal rdfs:subPropertyOf dc:coverage .


###  http://purl.org/dc/terms/title
dcterms:title rdfs:subPropertyOf dc:title .


###  http://purl.org/dc/terms/type
dcterms:type rdfs:subPropertyOf dc:type .


###  http://purl.org/dc/terms/valid
dcterms:valid rdfs:subPropertyOf dc:date .


###  http://purl.org/ontology/mo/derived_from
mo:derived_from rdf:type owl:AnnotationProperty ;
                rdfs:subPropertyOf dcterms:source .


###  http://purl.org/ontology/mo/genre
mo:genre rdf:type owl:AnnotationProperty ;
         rdfs:subPropertyOf ao:genre .


###  http://purl.org/ontology/mo/level
mo:level rdf:type owl:AnnotationProperty ;
         rdfs:comment """
        This annotation property associates to a particular Music Ontology term the corresponding
        expressiveness level. These levels can be:

            - 1: Only editorial/Musicbrainz type information
            - 2: Workflow information
            - 3: Even decomposition
        
        This property is mainly used for specification generation.
    """ ;
         rdfs:isDefinedBy <http://purl.org/ontology/mo/> ;
         rdfs:label "level" .


###  http://www.w3.org/2003/06/sw-vocab-status/ns#term_status
vs:term_status rdf:type owl:AnnotationProperty .


#################################################################
#    Datatypes
#################################################################

###  http://purl.org/dc/terms/Box
dcterms:Box rdf:type rdfs:Datatype .


###  http://purl.org/dc/terms/ISO3166
dcterms:ISO3166 rdf:type rdfs:Datatype .


###  http://purl.org/dc/terms/ISO639-2
dcterms:ISO639-2 rdf:type rdfs:Datatype .


###  http://purl.org/dc/terms/ISO639-3
dcterms:ISO639-3 rdf:type rdfs:Datatype .


###  http://purl.org/dc/terms/Period
dcterms:Period rdf:type rdfs:Datatype .


###  http://purl.org/dc/terms/Point
dcterms:Point rdf:type rdfs:Datatype .


###  http://purl.org/dc/terms/RFC1766
dcterms:RFC1766 rdf:type rdfs:Datatype .


###  http://purl.org/dc/terms/RFC3066
dcterms:RFC3066 rdf:type rdfs:Datatype .


###  http://purl.org/dc/terms/RFC4646
dcterms:RFC4646 rdf:type rdfs:Datatype .


###  http://purl.org/dc/terms/RFC5646
dcterms:RFC5646 rdf:type rdfs:Datatype .


###  http://purl.org/dc/terms/URI
dcterms:URI rdf:type rdfs:Datatype .


###  http://purl.org/dc/terms/W3CDTF
dcterms:W3CDTF rdf:type rdfs:Datatype .


#################################################################
#    Object Properties
#################################################################

###  http://purl.org/dc/terms/accessRights
dcterms:accessRights rdfs:subPropertyOf dcterms:rights ;
                     rdfs:range dcterms:RightsStatement .


###  http://purl.org/dc/terms/accrualMethod
dcterms:accrualMethod rdfs:domain <http://purl.org/dc/dcmitype/Collection> ;
                      rdfs:range dcterms:MethodOfAccrual .


###  http://purl.org/dc/terms/accrualPeriodicity
dcterms:accrualPeriodicity rdfs:domain <http://purl.org/dc/dcmitype/Collection> ;
                           rdfs:range dcterms:Frequency .


###  http://purl.org/dc/terms/accrualPolicy
dcterms:accrualPolicy rdfs:domain <http://purl.org/dc/dcmitype/Collection> ;
                      rdfs:range dcterms:Policy .


###  http://purl.org/dc/terms/audience
dcterms:audience rdfs:range dcterms:AgentClass .


###  http://purl.org/dc/terms/conformsTo
dcterms:conformsTo rdfs:range dcterms:Standard .


###  http://purl.org/dc/terms/contributor
dcterms:contributor rdfs:range dcterms:Agent .


###  http://purl.org/dc/terms/coverage
dcterms:coverage rdfs:range dcterms:LocationPeriodOrJurisdiction .


###  http://purl.org/dc/terms/creator
dcterms:creator rdfs:subPropertyOf dcterms:contributor ;
                rdfs:range dcterms:Agent .


###  http://purl.org/dc/terms/educationLevel
dcterms:educationLevel rdfs:subPropertyOf dcterms:audience ;
                       rdfs:range dcterms:AgentClass .


###  http://purl.org/dc/terms/extent
dcterms:extent rdfs:subPropertyOf dcterms:format ;
               rdfs:range dcterms:SizeOrDuration .


###  http://purl.org/dc/terms/format
dcterms:format rdfs:range dcterms:MediaTypeOrExtent .


###  http://purl.org/dc/terms/instructionalMethod
dcterms:instructionalMethod rdfs:range dcterms:MethodOfInstruction .


###  http://purl.org/dc/terms/language
dcterms:language rdfs:range dcterms:LinguisticSystem .


###  http://purl.org/dc/terms/license
dcterms:license rdfs:subPropertyOf dcterms:rights ;
                rdfs:range dcterms:LicenseDocument .


###  http://purl.org/dc/terms/mediator
dcterms:mediator rdfs:subPropertyOf dcterms:audience ;
                 rdfs:range dcterms:AgentClass .


###  http://purl.org/dc/terms/medium
dcterms:medium rdfs:subPropertyOf dcterms:format ;
               rdfs:domain dcterms:PhysicalResource ;
               rdfs:range dcterms:PhysicalMedium .


###  http://purl.org/dc/terms/provenance
dcterms:provenance rdfs:range dcterms:ProvenanceStatement .


###  http://purl.org/dc/terms/publisher
dcterms:publisher rdfs:range dcterms:Agent .


###  http://purl.org/dc/terms/rights
dcterms:rights rdfs:range dcterms:RightsStatement .


###  http://purl.org/dc/terms/rightsHolder
dcterms:rightsHolder rdfs:range dcterms:Agent .


###  http://purl.org/dc/terms/spatial
dcterms:spatial rdfs:subPropertyOf dcterms:coverage ;
                rdfs:range dcterms:Location .


###  http://purl.org/dc/terms/temporal
dcterms:temporal rdfs:subPropertyOf dcterms:coverage ;
                 rdfs:range dcterms:PeriodOfTime .


###  http://purl.org/dc/terms/type
dcterms:type rdfs:range rdfs:Class .


###  http://purl.org/ontology/mo/activity
mo:activity rdf:type owl:ObjectProperty ;
            rdfs:domain mo:MusicArtist ;
            rdfs:range mo:Activity ;
            mo:level "1" ;
            rdfs:comment "Relates an artist to an activity period" ;
            rdfs:isDefinedBy <http://purl.org/ontology/mo/> ;
            rdfs:label "activity" ;
            vs:term_status "testing" .


###  http://purl.org/ontology/mo/amazon_asin
mo:amazon_asin rdf:type owl:ObjectProperty ;
               rdfs:subPropertyOf foaf:isPrimaryTopicOf ;
               rdfs:domain [ rdf:type owl:Class ;
                             owl:unionOf ( frbr:Expression
                                           frbr:Item
                                           frbr:Manifestation
                                           frbr:Work
                                         )
                           ] ;
               rdfs:range foaf:Document ;
               mo:level "1" ;
               rdfs:comment "Used to link a work or the expression of a work to its corresponding Amazon ASINs page." ;
               rdfs:isDefinedBy <http://purl.org/ontology/mo/> ;
               rdfs:label "amazon_asin" ;
               vs:term_status "stable" .


###  http://purl.org/ontology/mo/arranged_in
mo:arranged_in rdf:type owl:ObjectProperty ;
               rdfs:subPropertyOf event:isFactorOf ;
               owl:inverseOf mo:arrangement_of ;
               rdfs:domain mo:MusicalWork ;
               rdfs:range mo:Arrangement ;
               mo:level "2" ;
               rdfs:comment """
        Associates a work to an arrangement event where it was arranged
    """ ;
               rdfs:isDefinedBy <http://purl.org/ontology/mo/> ;
               rdfs:label "arranged in" ;
               vs:term_status "unstable" .


###  http://purl.org/ontology/mo/arrangement_of
mo:arrangement_of rdf:type owl:ObjectProperty ;
                  rdfs:subPropertyOf event:factor ;
                  rdfs:domain mo:Arrangement ;
                  rdfs:range mo:MusicalWork ;
                  mo:level "2" ;
                  rdfs:comment """
                Associates an arrangement event to a work
        """ ;
                  rdfs:isDefinedBy <http://purl.org/ontology/mo/> ;
                  rdfs:label "arrangement of" ;
                  vs:term_status "unstable" .


###  http://purl.org/ontology/mo/artist
mo:artist rdf:type owl:ObjectProperty ;
          rdfs:domain mo:Membership ;
          rdfs:range foaf:Agent ;
          mo:level "1" ;
          rdfs:comment "Relates a membership event with the corresponding artist" ;
          rdfs:isDefinedBy <http://purl.org/ontology/mo/> ;
          rdfs:label "artist" ;
          vs:term_status "testing" .


###  http://purl.org/ontology/mo/availableAs
mo:availableAs rdf:type owl:ObjectProperty ;
               owl:equivalentProperty mo:available_as ;
               vs:term_status "deprecated" .


###  http://purl.org/ontology/mo/available_as
mo:available_as rdf:type owl:ObjectProperty ;
                rdfs:subPropertyOf frbr:exemplar ;
                rdfs:domain mo:MusicalManifestation ;
                rdfs:range mo:MusicalItem ;
                mo:level "1" ;
                rdfs:comment """
        Relates a musical manifestation to a musical item (this album, and my particular cd). By using
        this property, there is no assumption on wether the full content is available on the linked item.
        To be explicit about this, you can use a sub-property, such as mo:item (the full manifestation
        is available on that item) or mo:preview (only a part of the manifestation is available on
        that item).

        This is a subproperty of frbr:examplar.
    """ ;
                rdfs:isDefinedBy <http://purl.org/ontology/mo/> ;
                vs:term_status "stable" .


###  http://purl.org/ontology/mo/biography
mo:biography rdf:type owl:ObjectProperty ;
             rdfs:subPropertyOf foaf:isPrimaryTopicOf ;
             rdfs:domain mo:MusicArtist ;
             rdfs:range foaf:Document ;
             mo:level "1" ;
             rdfs:comment "Used to link an artist to their online biography." ;
             rdfs:isDefinedBy <http://purl.org/ontology/mo/> ;
             rdfs:label "biography" ;
             vs:term_status "stable" .


###  http://purl.org/ontology/mo/collaborated_with
mo:collaborated_with rdf:type owl:ObjectProperty ,
                              owl:SymmetricProperty ;
                     rdfs:domain foaf:Agent ;
                     rdfs:range foaf:Agent ;
                     mo:level "1" ;
                     rdfs:comment "Used to relate two collaborating people on a work." ;
                     rdfs:isDefinedBy <http://purl.org/ontology/mo/> ;
                     rdfs:label "collaborated_with" ;
                     vs:term_status "unstable" .


###  http://purl.org/ontology/mo/compilation_of
mo:compilation_of rdf:type owl:ObjectProperty ;
                  rdfs:domain mo:MusicalManifestation ;
                  rdfs:range mo:Signal ;
                  mo:level "1" ;
                  rdfs:comment "Indicates that a musical manifestation is a compilation of several Signals." ;
                  rdfs:isDefinedBy <http://purl.org/ontology/mo/> ;
                  rdfs:label "compilation_of" ;
                  vs:term_status "unstable" .


###  http://purl.org/ontology/mo/compiled
mo:compiled rdf:type owl:ObjectProperty ;
            owl:inverseOf mo:compiler ;
            rdfs:domain mo:MusicArtist ;
            rdfs:range mo:MusicalManifestation ;
            mo:level "1" ;
            rdfs:comment "Used to relate an person or a group of person who compiled the manifestation of a musical work." ;
            rdfs:isDefinedBy <http://purl.org/ontology/mo/> ;
            rdfs:label "compiled" ;
            vs:term_status "unstable" .


###  http://purl.org/ontology/mo/compiler
mo:compiler rdf:type owl:ObjectProperty ;
            rdfs:domain mo:MusicalManifestation ;
            rdfs:range mo:MusicArtist ;
            mo:level "1" ;
            rdfs:comment "Used to relate the manifestation of a musical work to a person or a group of person who compiled it." ;
            rdfs:isDefinedBy <http://purl.org/ontology/mo/> ;
            rdfs:label "compiler" ;
            vs:term_status "unstable" .


###  http://purl.org/ontology/mo/composed_in
mo:composed_in rdf:type owl:ObjectProperty ;
               owl:equivalentProperty mo:productOfComposition ;
               rdfs:subPropertyOf event:producedIn ;
               owl:inverseOf mo:produced_work ;
               rdfs:domain mo:MusicalWork ;
               rdfs:range mo:Composition ;
               mo:level "2" ;
               rdfs:comment """
        Associates a MusicalWork to the Composition event pertaining
        to its creation. For example, I might use this property to associate
        the Magic Flute to its composition event, occuring during 1782 and having as
        a mo:composer Mozart.
    """ ;
               rdfs:isDefinedBy <http://purl.org/ontology/mo/> ;
               rdfs:label "composed in" ;
               vs:term_status "unstable" .


###  http://purl.org/ontology/mo/composer
mo:composer rdf:type owl:ObjectProperty ;
            rdfs:subPropertyOf event:agent ;
            rdfs:domain mo:Composition ;
            rdfs:range foaf:Agent ;
            mo:level "2" ;
            rdfs:comment """
        Associates a composition event to the actual composer. For example,
        this property could link the event corresponding to the composition of the
        Magic Flute in 1782 to Mozart himself (who obviously has a FOAF profile:-) ).
    """ ;
            rdfs:isDefinedBy <http://purl.org/ontology/mo/> ;
            rdfs:label "composer" ;
            vs:term_status "stable" .


###  http://purl.org/ontology/mo/conducted
mo:conducted rdf:type owl:ObjectProperty ;
             rdfs:subPropertyOf event:isAgentIn ,
                                bio:event ;
             owl:inverseOf mo:conductor ;
             rdfs:domain foaf:Agent ;
             rdfs:range mo:Performance ;
             mo:level "2" ;
             rdfs:comment "Relates agents to the performances they were conducting" ;
             rdfs:isDefinedBy <http://purl.org/ontology/mo/> ;
             rdfs:label "conducted" ;
             vs:term_status "unstable" .


###  http://purl.org/ontology/mo/conductor
mo:conductor rdf:type owl:ObjectProperty ;
             rdfs:subPropertyOf event:agent ;
             rdfs:domain mo:Performance ;
             rdfs:range foaf:Agent ;
             mo:level "2" ;
             rdfs:comment "Relates a performance to the conductor involved" ;
             rdfs:isDefinedBy <http://purl.org/ontology/mo/> ;
             vs:term_status "stable" .


###  http://purl.org/ontology/mo/contains_sample_from
mo:contains_sample_from rdf:type owl:ObjectProperty ;
                        rdfs:subPropertyOf mo:derived_from ;
                        mo:level "1" ;
                        rdfs:comment """
        Relates a signal to another signal, which has been sampled.
        """ ;
                        rdfs:isDefinedBy <http://purl.org/ontology/mo/> ;
                        rdfs:label "contains_sample_from" ;
                        vs:term_status "unstable" .


###  http://purl.org/ontology/mo/derived_from
mo:derived_from rdf:type owl:ObjectProperty ;
                rdfs:domain mo:Signal ;
                rdfs:range mo:Signal .


###  http://purl.org/ontology/mo/discography
mo:discography rdf:type owl:ObjectProperty ;
               rdfs:subPropertyOf foaf:isPrimaryTopicOf ;
               rdfs:domain mo:MusicArtist ;
               rdfs:range foaf:Document ;
               mo:level "1" ;
               rdfs:comment "Used to links an artist to an online discography of their musical works. The discography should provide a summary of each released musical work of the artist." ;
               rdfs:isDefinedBy <http://purl.org/ontology/mo/> ;
               rdfs:label "discography" ;
               vs:term_status "stable" .


###  http://purl.org/ontology/mo/discogs
mo:discogs rdf:type owl:ObjectProperty ;
           rdfs:subPropertyOf foaf:isPrimaryTopicOf ;
           rdfs:domain [ rdf:type owl:Class ;
                         owl:unionOf ( mo:CorporateBody
                                       mo:MusicArtist
                                       mo:MusicalExpression
                                       mo:MusicalManifestation
                                       mo:MusicalWork
                                     )
                       ] ;
           rdfs:range foaf:Document ;
           mo:level "1" ;
           rdfs:comment "Used to link a musical work or the expression of a musical work, an artist or a corporate body to to its corresponding Discogs page." ;
           rdfs:isDefinedBy <http://purl.org/ontology/mo/> ;
           rdfs:label "discogs" ;
           vs:term_status "stable" .


###  http://purl.org/ontology/mo/djmix_of
mo:djmix_of rdf:type owl:ObjectProperty ;
            rdfs:subPropertyOf mo:derived_from ;
            mo:level "1" ;
            rdfs:comment """Indicates that all (or most of) the tracks of a musical work or the expression of a musical work were mixed together from all (or most of) the tracks from another musical work or the expression of a musical work to form a so called DJ-Mix. 
    
The tracks might have been altered by pitching (so that the tempo of one track matches the tempo of the following track) and fading (so that one track blends in smoothly with the other). If the tracks have been more substantially altered, the \"mo:remix\" relationship type is more appropriate. """ ;
            rdfs:isDefinedBy <http://purl.org/ontology/mo/> ;
            rdfs:label "djmix_of" ;
            vs:term_status "unstable" .


###  http://purl.org/ontology/mo/djmixed
mo:djmixed rdf:type owl:ObjectProperty ;
           owl:inverseOf mo:djmixed_by ;
           rdfs:domain mo:MusicArtist ;
           rdfs:range mo:Signal ;
           mo:level "1" ;
           rdfs:comment """Used to relate an artist who djmixed a musical work or the expression of a musical work. 
    
The artist usually selected the tracks, chose their sequence, and slightly changed them by fading (so that one track blends in smoothly with the other) or pitching (so that the tempo of one track matches the tempo of the following track). This applies to a 'Mixtape' in which all tracks were DJ-mixed together into one single long track. """ ;
           rdfs:isDefinedBy <http://purl.org/ontology/mo/> ;
           rdfs:label "djmixed" ;
           vs:term_status "unstable" .


###  http://purl.org/ontology/mo/djmixed_by
mo:djmixed_by rdf:type owl:ObjectProperty ;
              rdfs:domain mo:Signal ;
              rdfs:range mo:MusicArtist ;
              mo:level "1" ;
              rdfs:comment """Used to relate a work or the expression of a work to an artist who djmixed it. 
    
The artist usually selected the tracks, chose their sequence, and slightly changed them by fading (so that one track blends in smoothly with the other) or pitching (so that the tempo of one track matches the tempo of the following track). This applies to a 'Mixtape' in which all tracks were DJ-mixed together into one single long track. """ ;
              rdfs:isDefinedBy <http://purl.org/ontology/mo/> ;
              rdfs:label "djmixed_by" ;
              vs:term_status "unstable" .


###  http://purl.org/ontology/mo/download
mo:download rdf:type owl:ObjectProperty ;
            rdfs:subPropertyOf foaf:isPrimaryTopicOf ;
            rdfs:domain [ rdf:type owl:Class ;
                          owl:unionOf ( mo:CorporateBody
                                        frbr:Manifestation
                                        foaf:Agent
                                      )
                        ] ;
            rdfs:range foaf:Document ;
            mo:level "1" ;
            rdfs:comment """
                This property can be used to link from a person to the website where they make their works available, or from
                a manifestation (a track or an album, for example) to a web page where it is available for
                download.
        
        It is better to use one of the three sub-properties instead of this one in order to specify wether the
        content can be accessed for free (mo:freedownload), if it is just free preview material (mo:previewdownload), or
        if it can be accessed for some money (mo:paiddownload) (this includes links to the Amazon store, for example).

                This property MUST be used only if the content is just available through a web page (holding, for example
                a Flash application) - it is better to link to actual content directly through the use of mo:available_as and
                mo:Stream, mo:Torrent or mo:ED2K, etc. Therefore, Semantic Web user agents that don't know how to read HTML and even
                less to rip streams from Flash applications can still access the audio content.
        """ ;
            rdfs:isDefinedBy <http://purl.org/ontology/mo/> ;
            rdfs:label "download" ;
            vs:term_status "stable" .


###  http://purl.org/ontology/mo/encodes
mo:encodes rdf:type owl:ObjectProperty ;
           rdfs:domain mo:MusicalItem ;
           rdfs:range mo:Signal ;
           mo:level "1" ;
           rdfs:comment """
        Relates a MusicalItem (a track on a particular CD, an audio file, a stream somewhere) to the signal it encodes.

        This is usually a lower-resolution version of the master signal (issued from a Recording event).
    """ ;
           rdfs:isDefinedBy <http://purl.org/ontology/mo/> ;
           rdfs:label "encodes" ;
           vs:term_status "unstable" .


###  http://purl.org/ontology/mo/engineer
mo:engineer rdf:type owl:ObjectProperty ;
            rdfs:subPropertyOf event:agent ;
            owl:inverseOf mo:engineered ;
            rdfs:domain [ rdf:type owl:Class ;
                          owl:unionOf ( mo:Performance
                                        mo:Recording
                                        mo:RecordingSession
                                      )
                        ] ;
            rdfs:range foaf:Agent ;
            mo:level "2" ;
            rdfs:comment "Relates a performance or a recording to the engineer involved" ;
            rdfs:isDefinedBy <http://purl.org/ontology/mo/> ;
            vs:term_status "stable" .


###  http://purl.org/ontology/mo/engineered
mo:engineered rdf:type owl:ObjectProperty ;
              rdfs:subPropertyOf event:isAgentIn ,
                                 bio:event ;
              rdfs:domain foaf:Agent ;
              rdfs:range [ rdf:type owl:Class ;
                           owl:unionOf ( mo:Performance
                                         mo:Recording
                                         mo:RecordingSession
                                       )
                         ] ;
              mo:level "2" ;
              rdfs:comment "Relates agents to the performances/recordings they were engineering in" ;
              rdfs:isDefinedBy <http://purl.org/ontology/mo/> ;
              rdfs:label "engineered" ;
              vs:term_status "unstable" .


###  http://purl.org/ontology/mo/eventHomePage
mo:eventHomePage rdf:type owl:ObjectProperty ;
                 owl:equivalentProperty mo:event_homepage ;
                 vs:term_status "deprecated" .


###  http://purl.org/ontology/mo/event_homepage
mo:event_homepage rdf:type owl:ObjectProperty ;
                  rdfs:subPropertyOf foaf:isPrimaryTopicOf ;
                  rdfs:domain event:Event ;
                  rdfs:range foaf:Document ;
                  mo:level "2" ;
                  rdfs:comment "Links a particular event to a web page" ;
                  rdfs:isDefinedBy <http://purl.org/ontology/mo/> ;
                  rdfs:label "event homepage" ;
                  vs:term_status "stable" .


###  http://purl.org/ontology/mo/exchange_item
mo:exchange_item rdf:type owl:ObjectProperty ;
                 rdfs:domain foaf:Agent ;
                 rdfs:range frbr:Item ;
                 mo:level "1" ;
                 rdfs:comment "A person, a group of person or an organization exchanging an exemplar of a single manifestation." ;
                 rdfs:isDefinedBy <http://purl.org/ontology/mo/> ;
                 rdfs:label "exchange_item" ;
                 vs:term_status "stable" .


###  http://purl.org/ontology/mo/fanpage
mo:fanpage rdf:type owl:ObjectProperty ;
           rdfs:subPropertyOf foaf:isPrimaryTopicOf ;
           rdfs:domain mo:MusicArtist ;
           rdfs:range foaf:Document ;
           mo:level "1" ;
           rdfs:comment "Used to link an artist to a fan-created webpage devoted to that artist." ;
           rdfs:isDefinedBy <http://purl.org/ontology/mo/> ;
           rdfs:label "fanpage" ;
           vs:term_status "stable" .


###  http://purl.org/ontology/mo/free_download
mo:free_download rdf:type owl:ObjectProperty ;
                 owl:equivalentProperty mo:freedownload ;
                 rdfs:subPropertyOf mo:download ,
                                    foaf:isPrimaryTopicOf ;
                 rdfs:domain [ rdf:type owl:Class ;
                               owl:unionOf ( mo:CorporateBody
                                             frbr:Manifestation
                                             foaf:Agent
                                           )
                             ] ;
                 rdfs:range foaf:Document ;
                 mo:level "1" ;
                 rdfs:comment """
        This property can be used to link from a person to the website where they make their works available, or from
        a manifestation (a track or an album, for example) to a web page where it is available for free 
        download.

        This property MUST be used only if the content is just available through a web page (holding, for example
        a Flash application) - it is better to link to actual content directly through the use of mo:available_as and 
        mo:Stream, mo:Torrent or mo:ED2K, etc. Therefore, Semantic Web user agents that don't know how to read HTML and even
        less to rip streams from Flash applications can still access the audio content.
    """ ;
                 rdfs:isDefinedBy <http://purl.org/ontology/mo/> ;
                 rdfs:label "free download" ;
                 vs:term_status "stable" .


###  http://purl.org/ontology/mo/freedownload
mo:freedownload rdf:type owl:ObjectProperty ;
                rdfs:isDefinedBy <http://purl.org/ontology/mo/> ;
                vs:term_status "deprecated" .


###  http://purl.org/ontology/mo/genre
mo:genre rdf:type owl:ObjectProperty ;
         rdfs:domain [ rdf:type owl:Class ;
                       owl:unionOf ( mo:Arrangement
                                     mo:Composition
                                     mo:MusicalExpression
                                     mo:MusicalItem
                                     mo:MusicalManifestation
                                     mo:MusicalWork
                                     mo:Performance
                                     mo:Recording
                                     mo:RecordingSession
                                     foaf:Agent
                                   )
                     ] ;
         rdfs:range mo:Genre .


###  http://purl.org/ontology/mo/group
mo:group rdf:type owl:ObjectProperty ;
         rdfs:domain mo:Membership ;
         rdfs:range foaf:Group ;
         mo:level "1" ;
         rdfs:comment "Relates a membership event with the corresponding group" ;
         rdfs:isDefinedBy <http://purl.org/ontology/mo/> ;
         rdfs:label "group" ;
         vs:term_status "testing" .


###  http://purl.org/ontology/mo/has_track
mo:has_track rdf:type owl:ObjectProperty ;
             owl:equivalentProperty mo:track ;
             rdfs:isDefinedBy <http://purl.org/ontology/mo/> ;
             vs:term_status "deprecated" .


###  http://purl.org/ontology/mo/headliner
mo:headliner rdf:type owl:ObjectProperty ;
             rdfs:subPropertyOf mo:performer ;
             mo:level "2" ;
             rdfs:comment "Relates a performance to the headliner(s) involved" ;
             rdfs:isDefinedBy <http://purl.org/ontology/mo/> ;
             rdfs:label "headliner" ;
             vs:term_status "testing" .


###  http://purl.org/ontology/mo/homepage
mo:homepage rdf:type owl:ObjectProperty ;
            rdfs:subPropertyOf foaf:isPrimaryTopicOf ;
            rdfs:domain [ rdf:type owl:Class ;
                          owl:unionOf ( mo:MusicArtist
                                        mo:MusicalExpression
                                        mo:MusicalItem
                                        mo:MusicalManifestation
                                        mo:MusicalWork
                                      )
                        ] ;
            rdfs:range foaf:Document ;
            mo:level "1" ;
            rdfs:comment "Links an artist, a record, etc. to a corresponding web page" ;
            rdfs:isDefinedBy <http://purl.org/ontology/mo/> ;
            rdfs:label "homepage" ;
            vs:term_status "stable" .


###  http://purl.org/ontology/mo/image
mo:image rdf:type owl:ObjectProperty ;
         rdfs:subPropertyOf foaf:depiction ;
         rdfs:domain [ rdf:type owl:Class ;
                       owl:unionOf ( mo:MusicArtist
                                     mo:MusicalExpression
                                     mo:MusicalItem
                                     mo:MusicalManifestation
                                     mo:MusicalWork
                                   )
                     ] ;
         rdfs:range foaf:Image ;
         mo:level "1" ;
         rdfs:comment "Indicates a pictorial image (JPEG, GIF, PNG, Etc.) of a musical work, the expression of a musical work, the manifestation of a work or the examplar of a manifestation." ;
         rdfs:isDefinedBy <http://purl.org/ontology/mo/> ;
         rdfs:label "image" ;
         vs:term_status "stable" .


###  http://purl.org/ontology/mo/imdb
mo:imdb rdf:type owl:ObjectProperty ;
        rdfs:subPropertyOf foaf:isPrimaryTopicOf ;
        rdfs:domain [ rdf:type owl:Class ;
                      owl:unionOf ( mo:CorporateBody
                                    mo:MusicArtist
                                    mo:MusicalExpression
                                    mo:MusicalManifestation
                                    mo:MusicalWork
                                  )
                    ] ;
        rdfs:range foaf:Document ;
        mo:level "1" ;
        rdfs:comment "Used to link an artist, a musical work or the expression of a musical work to their equivalent page on IMDb, the InternetMovieDatabase." ;
        rdfs:isDefinedBy <http://purl.org/ontology/mo/> ;
        rdfs:label "imdb" ;
        vs:term_status "stable" .


###  http://purl.org/ontology/mo/instrument
mo:instrument rdf:type owl:ObjectProperty ;
              rdfs:subPropertyOf event:factor ;
              rdfs:domain mo:Performance ;
              rdfs:range mo:Instrument ;
              mo:level "2" ;
              rdfs:comment "Relates a performance to a musical instrument involved" ;
              rdfs:isDefinedBy <http://purl.org/ontology/mo/> ;
              vs:term_status "stable" .


###  http://purl.org/ontology/mo/interpreter
mo:interpreter rdf:type owl:ObjectProperty ;
               rdfs:domain mo:Signal ;
               rdfs:range mo:MusicArtist ;
               mo:level "1" ;
               rdfs:comment "Adds an involved music artist, who interpreted, remixed, or otherwise modified an existing signal, which resulted in the signal that is here the subject of this relation." ;
               rdfs:isDefinedBy <http://purl.org/ontology/mo/> ;
               rdfs:label "has interpeter" ;
               vs:term_status "testing" .


###  http://purl.org/ontology/mo/item
mo:item rdf:type owl:ObjectProperty ;
        rdfs:subPropertyOf mo:available_as ;
        rdfs:domain mo:MusicalManifestation ;
        rdfs:range mo:MusicalItem ;
        mo:level "1" ;
        rdfs:comment """
                Relates a musical manifestation to a musical item (this album, and my particular cd) holding the
                entire manifestation, and not just a part of it.
        """ ;
        rdfs:isDefinedBy <http://purl.org/ontology/mo/> ;
        vs:term_status "testing" .


###  http://purl.org/ontology/mo/key
mo:key rdf:type owl:ObjectProperty ;
       rdfs:domain [ rdf:type owl:Class ;
                     owl:unionOf ( mo:MusicalWork
                                   mo:Performance
                                   mo:Signal
                                 )
                   ] ;
       rdfs:range keys:Key ;
       mo:level "2" ;
       rdfs:comment """
        Indicated the key used by the musicians during a performance, or the key of a MusicalWork.
        Any of 24 major or minor diatonic scales that provide the tonal framework for a piece of music.""" ;
       rdfs:isDefinedBy <http://purl.org/ontology/mo/> ;
       rdfs:label "key" ;
       vs:term_status "stable" .


###  http://purl.org/ontology/mo/label
mo:label rdf:type owl:ObjectProperty ;
         rdfs:domain [ rdf:type owl:Class ;
                       owl:unionOf ( mo:MusicArtist
                                     mo:Release
                                   )
                     ] ;
         rdfs:range mo:Label ;
         mo:level "1" ;
         rdfs:comment "Associates a release event with the label releasing the record" ;
         rdfs:isDefinedBy <http://purl.org/ontology/mo/> ;
         rdfs:label "label" ;
         vs:term_status "testing" .


###  http://purl.org/ontology/mo/licence
mo:licence rdf:type owl:ObjectProperty ;
           rdfs:domain [ rdf:type owl:Class ;
                         owl:unionOf ( frbr:Expression
                                       frbr:Manifestation
                                       frbr:Work
                                     )
                       ] ;
           rdfs:range cc:License ;
           mo:level "1" ;
           rdfs:comment """Used to link a work or the expression of a work to the license under which they can be manipulated (downloaded, modified, etc). 
    
This is usually used to link to a Creative Commons licence.""" ;
           rdfs:isDefinedBy <http://purl.org/ontology/mo/> ;
           rdfs:label "licence" ;
           vs:term_status "stable" .


###  http://purl.org/ontology/mo/listened
mo:listened rdf:type owl:ObjectProperty ;
            rdfs:subPropertyOf event:isAgentIn ,
                               bio:event ;
            owl:inverseOf mo:listener ;
            rdfs:domain foaf:Agent ;
            rdfs:range mo:Performance ;
            mo:level "2" ;
            rdfs:comment "Relates agents to the performances they were listening in" ;
            rdfs:isDefinedBy <http://purl.org/ontology/mo/> ;
            rdfs:label "listened" ;
            vs:term_status "unstable" .


###  http://purl.org/ontology/mo/listener
mo:listener rdf:type owl:ObjectProperty ;
            rdfs:subPropertyOf event:agent ;
            rdfs:domain mo:Performance ;
            rdfs:range foaf:Agent ;
            mo:level "2" ;
            rdfs:comment "Relates a performance to the listener involved" ;
            rdfs:isDefinedBy <http://purl.org/ontology/mo/> ;
            vs:term_status "stable" .


###  http://purl.org/ontology/mo/lyrics
mo:lyrics rdf:type owl:ObjectProperty ;
          rdfs:domain mo:MusicalWork ;
          rdfs:range mo:Lyrics ;
          mo:level "2" ;
          rdfs:comment "Associates lyrics with a musical work" ;
          rdfs:isDefinedBy <http://purl.org/ontology/mo/> ;
          rdfs:label "lyrics" ;
          vs:term_status "testing" .


###  http://purl.org/ontology/mo/mailorder
mo:mailorder rdf:type owl:ObjectProperty ;
             rdfs:subPropertyOf foaf:isPrimaryTopicOf ;
             rdfs:domain [ rdf:type owl:Class ;
                           owl:unionOf ( mo:CorporateBody
                                         mo:MusicArtist
                                         frbr:Manifestation
                                       )
                         ] ;
             rdfs:range foaf:Document ;
             mo:level "1" ;
             rdfs:comment "Used to link a musical work or the expression of a musical work to a website where people can buy a copy of the musical manifestation." ;
             rdfs:isDefinedBy <http://purl.org/ontology/mo/> ;
             rdfs:label "mailorder" ;
             vs:term_status "stable" .


###  http://purl.org/ontology/mo/mashup_of
mo:mashup_of rdf:type owl:ObjectProperty ;
             rdfs:subPropertyOf mo:derived_from ;
             mo:level "1" ;
             rdfs:comment """Indicates that musical works or the expressions of a musical work were mashed up on this album or track. 
    
This means that two musical works or the expressions of a musical work by different artists are mixed together, over each other, or otherwise combined into a single musical work (usually by a third artist, the remixer).""" ;
             rdfs:isDefinedBy <http://purl.org/ontology/mo/> ;
             rdfs:label "mashup_of" ;
             vs:term_status "unstable" .


###  http://purl.org/ontology/mo/media_type
mo:media_type rdf:type owl:ObjectProperty ;
              rdfs:subPropertyOf dcterms:format ;
              rdfs:domain mo:MusicalManifestation ;
              rdfs:range dcterms:MediaType ;
              mo:level "1" ;
              rdfs:comment "The mediatype (file format or MIME type, or physical medium) of a musical manifestation, e.g. a MP3, CD or vinyl." ;
              rdfs:isDefinedBy <http://purl.org/ontology/mo/> ;
              rdfs:label "has media type" ;
              vs:term_status "testing" .


###  http://purl.org/ontology/mo/medley_of
mo:medley_of rdf:type owl:ObjectProperty ;
             rdfs:subPropertyOf mo:derived_from ;
             mo:level "1" ;
             rdfs:comment """Indicates that a musical expression is a medley of several other musical expressions. 
    
This means that the orignial musical expression were rearranged to create a new musical expression in the form of a medley. """ ;
             rdfs:isDefinedBy <http://purl.org/ontology/mo/> ;
             rdfs:label "medley_of" ;
             vs:term_status "unstable" .


###  http://purl.org/ontology/mo/member
mo:member rdf:type owl:ObjectProperty ;
          rdfs:subPropertyOf foaf:member ;
          rdfs:domain mo:MusicGroup ;
          rdfs:range foaf:Agent ;
          mo:level "1" ;
          rdfs:comment """
        Indicates a member of a musical group
    """ ;
          rdfs:isDefinedBy <http://purl.org/ontology/mo/> ;
          rdfs:label "member" ;
          vs:term_status "stable" .


###  http://purl.org/ontology/mo/member_of
mo:member_of rdf:type owl:ObjectProperty ;
             owl:inverseOf foaf:member ;
             rdfs:domain foaf:Agent ;
             rdfs:range foaf:Group ;
             mo:level "1" ;
             rdfs:comment "Inverse of the foaf:member property" ;
             rdfs:isDefinedBy <http://purl.org/ontology/mo/> ;
             rdfs:label "member_of" ;
             vs:term_status "unstable" .


###  http://purl.org/ontology/mo/membership
mo:membership rdf:type owl:ObjectProperty ;
              rdfs:domain foaf:Agent ;
              rdfs:range mo:Membership ;
              mo:level "1" ;
              rdfs:comment "Relates an agent with related membership events" ;
              rdfs:isDefinedBy <http://purl.org/ontology/mo/> ;
              rdfs:label "membership" ;
              vs:term_status "testing" .


###  http://purl.org/ontology/mo/movement
mo:movement rdf:type owl:ObjectProperty ;
            rdfs:domain mo:MusicalWork ;
            rdfs:range mo:Movement ;
            mo:level "2" ;
            rdfs:comment "Indicates that a musical work has movements" ;
            rdfs:isDefinedBy <http://purl.org/ontology/mo/> ;
            rdfs:label "has_movement" ;
            vs:term_status "unstable" .


###  http://purl.org/ontology/mo/musicbrainz
mo:musicbrainz rdf:type owl:ObjectProperty ;
               rdfs:subPropertyOf foaf:isPrimaryTopicOf ;
               rdfs:domain [ rdf:type owl:Class ;
                             owl:unionOf ( mo:MusicalManifestation
                                           mo:MusicalWork
                                           mo:Signal
                                           foaf:Agent
                                         )
                           ] ;
               rdfs:range foaf:Document ;
               mo:level "1" ;
               rdfs:comment """
        Linking an agent, a track or a record to its corresponding Musicbrainz page.
        """ ;
               rdfs:isDefinedBy <http://purl.org/ontology/mo/> ;
               rdfs:label "musicbrainz" ;
               vs:term_status "stable" .


###  http://purl.org/ontology/mo/musicmoz
mo:musicmoz rdf:type owl:ObjectProperty ;
            rdfs:subPropertyOf foaf:isPrimaryTopicOf ;
            rdfs:domain [ rdf:type owl:Class ;
                          owl:unionOf ( mo:MusicArtist
                                        mo:MusicalExpression
                                        mo:MusicalManifestation
                                        mo:MusicalWork
                                      )
                        ] ;
            rdfs:range foaf:Document ;
            mo:level "1" ;
            rdfs:comment "Used to link an artist, a musical work or the expression of a musical work to its corresponding MusicMoz page." ;
            rdfs:isDefinedBy <http://purl.org/ontology/mo/> ;
            rdfs:label "musicmoz" ;
            vs:term_status "stable" .


###  http://purl.org/ontology/mo/myspace
mo:myspace rdf:type owl:ObjectProperty ;
           rdfs:subPropertyOf foaf:isPrimaryTopicOf ;
           rdfs:domain foaf:Agent ;
           rdfs:range foaf:Document ;
           mo:level "1" ;
           rdfs:comment "Used to link a person to its corresponding MySpace page." ;
           rdfs:isDefinedBy <http://purl.org/ontology/mo/> ;
           rdfs:label "myspace" ;
           vs:term_status "stable" .


###  http://purl.org/ontology/mo/olga
mo:olga rdf:type owl:ObjectProperty ;
        rdfs:subPropertyOf foaf:isPrimaryTopicOf ;
        rdfs:domain mo:Track ;
        rdfs:range foaf:Document ;
        mo:level "1" ;
        rdfs:comment "Used to link a track to a tabulature file for track in the On-Line Guitar Archive." ;
        rdfs:isDefinedBy <http://purl.org/ontology/mo/> ;
        rdfs:label "olga" ;
        vs:term_status "stable" .


###  http://purl.org/ontology/mo/onlinecommunity
mo:onlinecommunity rdf:type owl:ObjectProperty ;
                   rdfs:subPropertyOf foaf:isPrimaryTopicOf ;
                   rdfs:domain foaf:Agent ;
                   rdfs:range foaf:Document ;
                   mo:level "1" ;
                   rdfs:comment "Used to link a person with an online community web page like a blog, a wiki, a forum, a livejournal page, Etc." ;
                   rdfs:isDefinedBy <http://purl.org/ontology/mo/> ;
                   rdfs:label "onlinecommunity" ;
                   vs:term_status "stable" .


###  http://purl.org/ontology/mo/origin
mo:origin rdf:type owl:ObjectProperty ;
          rdfs:domain mo:MusicArtist ;
          rdfs:range geo:SpatialThing ;
          mo:level "1" ;
          rdfs:comment "Relates an artist to its geographic origin" ;
          rdfs:isDefinedBy <http://purl.org/ontology/mo/> ;
          rdfs:label "origin" ;
          vs:term_status "testing" .


###  http://purl.org/ontology/mo/other_release_of
mo:other_release_of rdf:type owl:ObjectProperty ,
                             owl:SymmetricProperty ;
                    rdfs:domain mo:MusicalManifestation ;
                    rdfs:range mo:MusicalManifestation ;
                    mo:level "1" ;
                    rdfs:comment "Indicates that two musical manifestations are essentially the same." ;
                    rdfs:isDefinedBy <http://purl.org/ontology/mo/> ;
                    rdfs:label "other_release_of" ;
                    vs:term_status "unstable" .


###  http://purl.org/ontology/mo/paid_download
mo:paid_download rdf:type owl:ObjectProperty ;
                 owl:equivalentProperty mo:paiddownload ;
                 rdfs:subPropertyOf mo:download ,
                                    foaf:isPrimaryTopicOf ;
                 rdfs:domain [ rdf:type owl:Class ;
                               owl:unionOf ( mo:CorporateBody
                                             mo:MusicArtist
                                             frbr:Manifestation
                                           )
                             ] ;
                 rdfs:range foaf:Document ;
                 mo:level "1" ;
                 rdfs:comment """
                Provide a link from an artist to a web page where all of that artist's musical work is available for some money,
                or a link from a manifestation (record/track, for example) to a web page providing a paid access to this manifestation.
        """ ;
                 rdfs:isDefinedBy <http://purl.org/ontology/mo/> ;
                 rdfs:label "paid download" ;
                 vs:term_status "stable" .


###  http://purl.org/ontology/mo/paiddownload
mo:paiddownload rdf:type owl:ObjectProperty ;
                rdfs:isDefinedBy <http://purl.org/ontology/mo/> ;
                vs:term_status "deprecated" .


###  http://purl.org/ontology/mo/performance_of
mo:performance_of rdf:type owl:ObjectProperty ;
                  owl:equivalentProperty mo:usesWork ;
                  rdfs:subPropertyOf event:factor ;
                  owl:inverseOf mo:performed_in ;
                  rdfs:domain mo:Performance ;
                  rdfs:range [ rdf:type owl:Class ;
                               owl:unionOf ( mo:MusicalWork
                                             mo:Score
                                           )
                             ] ;
                  mo:level "2" ;
                  rdfs:comment """
        Associates a Performance to a musical work or an arrangement that is being used as a factor in it.
        For example, I might use this property to attach the Magic Flute musical work to 
        a particular Performance.
    """ ;
                  rdfs:isDefinedBy <http://purl.org/ontology/mo/> ;
                  rdfs:label "performance of" ;
                  vs:term_status "unstable" .


###  http://purl.org/ontology/mo/performed
mo:performed rdf:type owl:ObjectProperty ;
             rdfs:subPropertyOf event:isAgentIn ,
                                bio:event ;
             owl:inverseOf mo:performer ;
             rdfs:domain foaf:Agent ;
             rdfs:range mo:Performance ;
             mo:level "2" ;
             rdfs:comment "Relates agents to the performances they were performing in" ;
             rdfs:isDefinedBy <http://purl.org/ontology/mo/> ;
             rdfs:label "performed" ;
             vs:term_status "unstable" .


###  http://purl.org/ontology/mo/performed_in
mo:performed_in rdf:type owl:ObjectProperty ;
                owl:equivalentProperty mo:usedInPerformance ;
                rdfs:subPropertyOf event:isFactorOf ;
                rdfs:domain [ rdf:type owl:Class ;
                              owl:unionOf ( mo:MusicalWork
                                            mo:Score
                                          )
                            ] ;
                rdfs:range mo:Performance ;
                mo:level "2" ;
                rdfs:comment """
        Associates a Musical Work or an Score to Performances in which they were
        a factor. For example, I might use this property in order to 
        associate the Magic Flute to a particular performance at the Opera
        Bastille last year.""" ;
                rdfs:isDefinedBy <http://purl.org/ontology/mo/> ;
                rdfs:label "performed in" ;
                vs:term_status "unstable" .


###  http://purl.org/ontology/mo/performer
mo:performer rdf:type owl:ObjectProperty ;
             rdfs:subPropertyOf event:agent ;
             rdfs:domain mo:Performance ;
             rdfs:range foaf:Agent ;
             mo:level "2" ;
             rdfs:comment "Relates a performance to the performers involved" ;
             rdfs:isDefinedBy <http://purl.org/ontology/mo/> ;
             vs:term_status "stable" .


###  http://purl.org/ontology/mo/possess_item
mo:possess_item rdf:type owl:ObjectProperty ;
                rdfs:domain foaf:Agent ;
                rdfs:range frbr:Item ;
                mo:level "1" ;
                rdfs:comment "A person, a group of person or an organization possessing an exemplar of a single manifestation." ;
                rdfs:isDefinedBy <http://purl.org/ontology/mo/> ;
                rdfs:label "possess_item" ;
                vs:term_status "stable" .


###  http://purl.org/ontology/mo/preview
mo:preview rdf:type owl:ObjectProperty ;
           rdfs:subPropertyOf mo:available_as ;
           rdfs:domain mo:MusicalManifestation ;
           rdfs:range mo:MusicalItem ;
           mo:level "1" ;
           rdfs:comment """
                Relates a musical manifestation to a musical item (this album, and my particular cd), which holds
                a preview of the manifestation (eg. one track for an album, or a snippet for a track)
        """ ;
           rdfs:isDefinedBy <http://purl.org/ontology/mo/> ;
           vs:term_status "testing" .


###  http://purl.org/ontology/mo/preview_download
mo:preview_download rdf:type owl:ObjectProperty ;
                    rdfs:subPropertyOf mo:download ,
                                       foaf:isPrimaryTopicOf ;
                    rdfs:domain [ rdf:type owl:Class ;
                                  owl:unionOf ( mo:CorporateBody
                                                frbr:Manifestation
                                                foaf:Agent
                                              )
                                ] ;
                    rdfs:range foaf:Document ;
                    mo:level "1" ;
                    rdfs:comment """
                This property can be used to link from a person to the website where they make previews of their works available, or from
                a manifestation (a track or an album, for example) to a web page where a preview download is available.

                This property MUST be used only if the content is just available through a web page (holding, for example
                a Flash application) - it is better to link to actual content directly through the use of mo:available_as and
                mo:Stream, mo:Torrent or mo:ED2K, etc. Therefore, Semantic Web user agents that don't know how to read HTML and even
                less to rip streams from Flash applications can still access the audio content.
        """ ;
                    rdfs:isDefinedBy <http://purl.org/ontology/mo/> ;
                    rdfs:label "preview download" ;
                    vs:term_status "stable" .


###  http://purl.org/ontology/mo/primary_instrument
mo:primary_instrument rdf:type owl:ObjectProperty ;
                      rdfs:domain [ rdf:type owl:Class ;
                                    owl:unionOf ( mo:Membership
                                                  foaf:Agent
                                                )
                                  ] ;
                      rdfs:range mo:Instrument ;
                      mo:level "1" ;
                      rdfs:comment "Indicates that an artist primarily plays an instrument, or that a member was primarily playing a particular instrument during his membership" ;
                      rdfs:isDefinedBy <http://purl.org/ontology/mo/> ;
                      rdfs:label "primary instrument" ;
                      vs:term_status "testing" .


###  http://purl.org/ontology/mo/produced
mo:produced rdf:type owl:ObjectProperty ;
            owl:inverseOf mo:producer ;
            rdfs:domain foaf:Agent ;
            rdfs:range mo:MusicalManifestation ;
            mo:level "1" ;
            rdfs:comment "Used to relate an person or a group of person who produced the manifestation of a work." ;
            rdfs:isDefinedBy <http://purl.org/ontology/mo/> ;
            rdfs:label "produced" ;
            vs:term_status "stable" .


###  http://purl.org/ontology/mo/produced_score
mo:produced_score rdf:type owl:ObjectProperty ;
                  rdfs:subPropertyOf event:product ;
                  rdfs:domain [ rdf:type owl:Class ;
                                owl:unionOf ( mo:Arrangement
                                              mo:Composition
                                            )
                              ] ;
                  rdfs:range mo:Score ;
                  mo:level "2" ;
                  rdfs:comment """
        Associates an arrangement or a composition event to a score product (score here does not refer to a published score, but more
        an abstract arrangement of a particular work).
    """ ;
                  rdfs:isDefinedBy <http://purl.org/ontology/mo/> ;
                  rdfs:label "produced score" ;
                  vs:term_status "unstable" .


###  http://purl.org/ontology/mo/produced_signal
mo:produced_signal rdf:type owl:ObjectProperty ;
                   owl:equivalentProperty mo:producesSignal ;
                   rdfs:subPropertyOf event:product ;
                   rdfs:domain mo:Recording ;
                   rdfs:range mo:Signal ;
                   mo:level "2" ;
                   rdfs:comment """
                Associates a Recording to the outputted signal.
        """ ;
                   rdfs:isDefinedBy <http://purl.org/ontology/mo/> ;
                   rdfs:label "produced signal" ;
                   vs:term_status "stable" .


###  http://purl.org/ontology/mo/produced_signal_group
mo:produced_signal_group rdf:type owl:ObjectProperty ;
                         rdfs:subPropertyOf event:product ;
                         rdfs:domain mo:RecordingSession ;
                         rdfs:range mo:SignalGroup ;
                         mo:level "2" ;
                         rdfs:comment "Associates a recording session with a group of master signals produced by it." ;
                         rdfs:isDefinedBy <http://purl.org/ontology/mo/> ;
                         rdfs:label "produced signal group" ;
                         vs:term_status "testing" .


###  http://purl.org/ontology/mo/produced_sound
mo:produced_sound rdf:type owl:ObjectProperty ;
                  owl:equivalentProperty mo:producesSound ;
                  rdfs:subPropertyOf event:product ;
                  rdfs:domain mo:Performance ;
                  rdfs:range mo:Sound ;
                  mo:level "2" ;
                  rdfs:comment """
                Associates a Performance to a physical Sound that is being produced by it.
        """ ;
                  rdfs:isDefinedBy <http://purl.org/ontology/mo/> ;
                  rdfs:label "produced sound" ;
                  vs:term_status "stable" .


###  http://purl.org/ontology/mo/produced_work
mo:produced_work rdf:type owl:ObjectProperty ;
                 owl:equivalentProperty mo:producesWork ;
                 rdfs:subPropertyOf event:product ;
                 rdfs:domain mo:Composition ;
                 rdfs:range mo:MusicalWork ;
                 mo:level "2" ;
                 rdfs:comment """
                Associates a composition event to the produced MusicalWork. For example,
                this property could link the event corresponding to the composition of the
                Magic Flute in 1782 to the Magic Flute musical work itself. This musical work
                can then be used in particular performances.
        """ ;
                 rdfs:isDefinedBy <http://purl.org/ontology/mo/> ;
                 rdfs:label "produced work" ;
                 vs:term_status "stable" .


###  http://purl.org/ontology/mo/producer
mo:producer rdf:type owl:ObjectProperty ;
            rdfs:domain mo:MusicalManifestation ;
            rdfs:range foaf:Agent ;
            mo:level "1" ;
            rdfs:comment "Used to relate the manifestation of a work to a person or a group of person who produced it." ;
            rdfs:isDefinedBy <http://purl.org/ontology/mo/> ;
            rdfs:label "producer" ;
            vs:term_status "stable" .


###  http://purl.org/ontology/mo/producesSignal
mo:producesSignal rdf:type owl:ObjectProperty ;
                  rdfs:isDefinedBy <http://purl.org/ontology/mo/> ;
                  vs:term_status "deprecated" .


###  http://purl.org/ontology/mo/producesSound
mo:producesSound rdf:type owl:ObjectProperty ;
                 rdfs:isDefinedBy <http://purl.org/ontology/mo/> ;
                 vs:term_status "deprecated" .


###  http://purl.org/ontology/mo/producesWork
mo:producesWork rdf:type owl:ObjectProperty .


###  http://purl.org/ontology/mo/productOfComposition
mo:productOfComposition rdf:type owl:ObjectProperty ;
                        rdfs:isDefinedBy <http://purl.org/ontology/mo/> ;
                        vs:term_status "deprecated" .


###  http://purl.org/ontology/mo/publicationOf
mo:publicationOf rdf:type owl:ObjectProperty ;
                 owl:equivalentProperty mo:publication_of ;
                 vs:term_status "deprecated" .


###  http://purl.org/ontology/mo/publication_of
mo:publication_of rdf:type owl:ObjectProperty ;
                  owl:inverseOf mo:published_as ;
                  rdfs:domain mo:MusicalManifestation ;
                  rdfs:range mo:MusicalExpression ;
                  mo:level "1" ;
                  rdfs:comment "Link a particular manifestation to the related signal, score, libretto, or lyrics" ;
                  rdfs:isDefinedBy <http://purl.org/ontology/mo/> ;
                  rdfs:label "publication of" ;
                  vs:term_status "unstable" .


###  http://purl.org/ontology/mo/published
mo:published rdf:type owl:ObjectProperty ;
             owl:inverseOf mo:publisher ;
             rdfs:domain foaf:Agent ;
             rdfs:range mo:MusicalManifestation ;
             mo:level "1" ;
             rdfs:comment "Used to relate an person or a group of person who published the manifestation of a work." ;
             rdfs:isDefinedBy <http://purl.org/ontology/mo/> ;
             rdfs:label "published" ;
             vs:term_status "unstable" .


###  http://purl.org/ontology/mo/publishedAs
mo:publishedAs rdf:type owl:ObjectProperty ;
               owl:equivalentProperty mo:published_as ;
               vs:term_status "deprecated" .


###  http://purl.org/ontology/mo/published_as
mo:published_as rdf:type owl:ObjectProperty ;
                rdfs:subPropertyOf frbr:embodiment ;
                rdfs:domain mo:MusicalExpression ;
                rdfs:range mo:MusicalManifestation ;
                mo:level "1" ;
                rdfs:comment """
        Links a musical expression (e.g. a signal or a score) to one of its manifestations (e.g. a track on a particular record or a published score).
    """ ;
                rdfs:isDefinedBy <http://purl.org/ontology/mo/> ;
                rdfs:label "published as" ;
                vs:term_status "stable" .


###  http://purl.org/ontology/mo/publisher
mo:publisher rdf:type owl:ObjectProperty ;
             rdfs:domain mo:MusicalManifestation ;
             rdfs:range foaf:Agent ;
             mo:level "1" ;
             rdfs:comment "Used to relate a musical manifestation to a person or a group of person who published it." ;
             rdfs:isDefinedBy <http://purl.org/ontology/mo/> ;
             rdfs:label "publisher" ;
             vs:term_status "unstable" .


###  http://purl.org/ontology/mo/publishingLocation
mo:publishingLocation rdf:type owl:ObjectProperty ;
                      owl:equivalentProperty mo:publishing_location ;
                      vs:term_status "deprecated" .


###  http://purl.org/ontology/mo/publishing_location
mo:publishing_location rdf:type owl:ObjectProperty ;
                       rdfs:domain mo:MusicalManifestation ;
                       rdfs:range geo:SpatialThing ;
                       mo:level "1" ;
                       rdfs:comment """
        Relates a musical manifestation to its publication location.
        """ ;
                       rdfs:isDefinedBy <http://purl.org/ontology/mo/> ;
                       rdfs:label "publishingLocation" ;
                       vs:term_status "stable" .


###  http://purl.org/ontology/mo/record
mo:record rdf:type owl:ObjectProperty ;
          rdfs:domain mo:Release ;
          rdfs:range mo:Record ;
          mo:level "1" ;
          rdfs:comment "Associates a release with the records it contains. A single release can be associated with multiple records, for example for a multi-disc release." ;
          rdfs:isDefinedBy <http://purl.org/ontology/mo/> ;
          rdfs:label "released record" ;
          vs:term_status "testing" .


###  http://purl.org/ontology/mo/recordedAs
mo:recordedAs rdf:type owl:ObjectProperty ;
              owl:equivalentProperty mo:recorded_as ;
              owl:inverseOf mo:records .


###  http://purl.org/ontology/mo/recorded_as
mo:recorded_as rdf:type owl:ObjectProperty ;
               owl:inverseOf mo:records ;
               rdfs:domain mo:Performance ;
               rdfs:range mo:Signal ;
               mo:level "2" ;
               rdfs:comment """
        This is a shortcut property, allowing to bypass all the Sound/Recording steps. This property
        allows to directly link a Performance to the recorded Signal. This is recommended for \"normal\"
        users. However, advanced users wanting to express things such as the location of the microphone will
        have to create this shortcut as well as the whole workflow, in order to let the \"normal\" users access
        simply the, well, simple information:-) .
    """ ;
               rdfs:isDefinedBy <http://purl.org/ontology/mo/> ;
               rdfs:label "recorded as" ;
               vs:term_status "stable" .


###  http://purl.org/ontology/mo/recorded_in
mo:recorded_in rdf:type owl:ObjectProperty ;
               owl:equivalentProperty mo:usedInRecording ;
               rdfs:subPropertyOf event:isFactorOf ;
               owl:inverseOf mo:recording_of ;
               rdfs:domain mo:Sound ;
               rdfs:range mo:Recording ;
               mo:level "2" ;
               rdfs:comment """
            Associates a physical Sound to a Recording event where it is being used 
        in order to produce a signal. For example, I might use this property to 
        associate the sound produced by a particular performance of the magic flute
        to a given recording, done using my cell-phone.
    """ ;
               rdfs:isDefinedBy <http://purl.org/ontology/mo/> ;
               rdfs:label "recorded in" ;
               vs:term_status "unstable" .


###  http://purl.org/ontology/mo/recording_of
mo:recording_of rdf:type owl:ObjectProperty ;
                owl:equivalentProperty mo:usesSound ;
                rdfs:subPropertyOf event:factor ;
                rdfs:domain mo:Recording ;
                rdfs:range mo:Sound ;
                mo:level "2" ;
                rdfs:comment """
            Associates a Recording event to a physical Sound being recorded.
                For example, I might use this property to
                associate a given recording, done using my cell phone, to the 
        sound produced by a particular performance of the magic flute.
    """ ;
                rdfs:isDefinedBy <http://purl.org/ontology/mo/> ;
                rdfs:label "recorded sound" ;
                vs:term_status "stable" .


###  http://purl.org/ontology/mo/records
mo:records rdf:type owl:ObjectProperty ;
           rdfs:domain mo:Signal ;
           rdfs:range mo:Performance ;
           mo:level "2" ;
           rdfs:comment """
        This is the inverse of the shortcut property recordedAs, allowing to relate directly a performance
        to a signal.
    """ ;
           rdfs:isDefinedBy <http://purl.org/ontology/mo/> ;
           rdfs:label "records" ;
           vs:term_status "unstable" .


###  http://purl.org/ontology/mo/release
mo:release rdf:type owl:ObjectProperty ;
           rdfs:subPropertyOf event:product ;
           rdfs:domain mo:ReleaseEvent ;
           rdfs:range mo:Release ;
           mo:level "1" ;
           rdfs:comment "Associates a release with the corresponding release event" ;
           rdfs:isDefinedBy <http://purl.org/ontology/mo/> ;
           rdfs:label "release" ;
           vs:term_status "testing" .


###  http://purl.org/ontology/mo/releaseStatus
mo:releaseStatus rdf:type owl:ObjectProperty ;
                 owl:equivalentProperty mo:release_status ;
                 vs:term_status "deprecated" .


###  http://purl.org/ontology/mo/releaseType
mo:releaseType rdf:type owl:ObjectProperty ;
               owl:equivalentProperty mo:release_type ;
               vs:term_status "deprecated" .


###  http://purl.org/ontology/mo/release_status
mo:release_status rdf:type owl:ObjectProperty ;
                  rdfs:domain mo:MusicalManifestation ;
                  rdfs:range mo:ReleaseStatus ;
                  mo:level "1" ;
                  rdfs:comment """
                Relates a musical manifestation to its release status (bootleg, ...)
        """ ;
                  rdfs:isDefinedBy <http://purl.org/ontology/mo/> ;
                  vs:term_status "stable" .


###  http://purl.org/ontology/mo/release_type
mo:release_type rdf:type owl:ObjectProperty ;
                rdfs:domain mo:MusicalManifestation ;
                rdfs:range mo:ReleaseType ;
                mo:level "1" ;
                rdfs:comment """
        Relates a musical manifestation to its release type (interview, spoken word, album, ...)
    """ ;
                rdfs:isDefinedBy <http://purl.org/ontology/mo/> ;
                vs:term_status "stable" .


###  http://purl.org/ontology/mo/remaster_of
mo:remaster_of rdf:type owl:ObjectProperty ;
               rdfs:subPropertyOf mo:derived_from ;
               mo:level "1" ;
               rdfs:comment """This relates two musical work or the expression of a musical work, where one is a remaster of the other. 
    
A remaster is a new version made for release from source recordings that were earlier released separately. This is usually done to improve the audio quality or adjust for more modern playback equipment. The process generally doesn't involve changing the music in any artistically important way. It may, however, result in tracks that are a few seconds longer or shorter.""" ;
               rdfs:isDefinedBy <http://purl.org/ontology/mo/> ;
               rdfs:label "remaster_of" ;
               vs:term_status "unstable" .


###  http://purl.org/ontology/mo/remix_of
mo:remix_of rdf:type owl:ObjectProperty ;
            rdfs:subPropertyOf mo:derived_from ;
            mo:level "1" ;
            rdfs:comment "Used to relate the remix of a musical work in a substantially altered version produced by mixing together individual tracks or segments of an original musical source work." ;
            rdfs:isDefinedBy <http://purl.org/ontology/mo/> ;
            rdfs:label "remix_of" ;
            vs:term_status "unstable" .


###  http://purl.org/ontology/mo/remixed
mo:remixed rdf:type owl:ObjectProperty ;
           owl:inverseOf mo:remixer ;
           rdfs:domain mo:MusicArtist ;
           rdfs:range mo:Signal ;
           mo:level "1" ;
           rdfs:comment """Used to relate an artist who remixed a musical work or the expression of a musical work. 
    
This involves taking just one other musical work and using audio editing to make it sound like a significantly different, but usually still recognisable, song. It can be used to link an artist to a single song that they remixed, or, if they remixed an entire musical work.""" ;
           rdfs:isDefinedBy <http://purl.org/ontology/mo/> ;
           rdfs:label "remixed" ;
           vs:term_status "unstable" .


###  http://purl.org/ontology/mo/remixer
mo:remixer rdf:type owl:ObjectProperty ;
           rdfs:subPropertyOf mo:interpreter ;
           mo:level "1" ;
           rdfs:comment """Used to relate a musical work or the expression of a musical work to an artist who remixed it. 
    
This involves taking just one other musical work and using audio editing to make it sound like a significantly different, but usually still recognisable, song. It can be used to link an artist to a single song that they remixed, or, if they remixed an entire musical work.""" ;
           rdfs:isDefinedBy <http://purl.org/ontology/mo/> ;
           rdfs:label "remixer" ;
           vs:term_status "unstable" .


###  http://purl.org/ontology/mo/review
mo:review rdf:type owl:ObjectProperty ;
          rdfs:subPropertyOf foaf:isPrimaryTopicOf ;
          rdfs:domain [ rdf:type owl:Class ;
                        owl:unionOf ( frbr:Expression
                                      frbr:Manifestation
                                      frbr:Work
                                    )
                      ] ;
          rdfs:range foaf:Document ;
          mo:level "1" ;
          rdfs:comment """Used to link a work or the expression of a work to a review. 
    
The review does not have to be open content, as long as it is accessible to the general internet population.""" ;
          rdfs:isDefinedBy <http://purl.org/ontology/mo/> ;
          rdfs:label "review" ;
          vs:term_status "stable" .


###  http://purl.org/ontology/mo/sampled
mo:sampled rdf:type owl:ObjectProperty ;
           owl:inverseOf mo:sampler ;
           rdfs:domain mo:MusicArtist ;
           rdfs:range mo:Signal ;
           mo:level "1" ;
           rdfs:comment "Used to relate an artist who sampled a Signal." ;
           rdfs:isDefinedBy <http://purl.org/ontology/mo/> ;
           rdfs:label "sampled" ;
           vs:term_status "unstable" .


###  http://purl.org/ontology/mo/sampledVersionOf
mo:sampledVersionOf rdf:type owl:ObjectProperty ;
                    owl:equivalentProperty mo:sampled_version_of ;
                    rdfs:isDefinedBy <http://purl.org/ontology/mo/> ;
                    vs:term_status "deprecated" .


###  http://purl.org/ontology/mo/sampled_version
mo:sampled_version rdf:type owl:ObjectProperty ;
                   owl:inverseOf mo:sampled_version_of ;
                   rdfs:domain mo:AnalogSignal ;
                   rdfs:range mo:DigitalSignal ;
                   mo:level "2" ;
                   rdfs:comment """
        Associates an analog signal with a sampled version of it
    """ ;
                   rdfs:isDefinedBy <http://purl.org/ontology/mo/> ;
                   rdfs:label "sampled version" ;
                   vs:term_status "stable" .


###  http://purl.org/ontology/mo/sampled_version_of
mo:sampled_version_of rdf:type owl:ObjectProperty ;
                      rdfs:subPropertyOf mo:derived_from ;
                      rdf:type owl:FunctionalProperty ;
                      rdfs:domain mo:DigitalSignal ;
                      rdfs:range mo:AnalogSignal ;
                      mo:level "2" ;
                      rdfs:comment """
        Associates a digital signal with the analog version of it
    """ ;
                      rdfs:isDefinedBy <http://purl.org/ontology/mo/> ;
                      rdfs:label "sampled version of" ;
                      vs:term_status "stable" .


###  http://purl.org/ontology/mo/sampler
mo:sampler rdf:type owl:ObjectProperty ;
           rdfs:subPropertyOf mo:interpreter ;
           mo:level "1" ;
           rdfs:comment "Used to relate the signal of a musical work to an artist who sampled it." ;
           rdfs:isDefinedBy <http://purl.org/ontology/mo/> ;
           rdfs:label "sampler" ;
           vs:term_status "unstable" .


###  http://purl.org/ontology/mo/sell_item
mo:sell_item rdf:type owl:ObjectProperty ;
             rdfs:domain foaf:Agent ;
             rdfs:range frbr:Item ;
             mo:level "1" ;
             rdfs:comment "A person, a group of person or an organization selling an exemplar of a single manifestation." ;
             rdfs:isDefinedBy <http://purl.org/ontology/mo/> ;
             rdfs:label "sell_item" ;
             vs:term_status "stable" .


###  http://purl.org/ontology/mo/signal
mo:signal rdf:type owl:ObjectProperty ;
          rdfs:domain mo:SignalGroup ;
          rdfs:range mo:Signal ;
          mo:level "1" ;
          rdfs:comment "Associates a group of signals with one of the signals it contains" ;
          rdfs:isDefinedBy <http://purl.org/ontology/mo/> ;
          rdfs:label "signal" ;
          vs:term_status "testing" .


###  http://purl.org/ontology/mo/signalTime
mo:signalTime rdf:type owl:ObjectProperty ;
              owl:equivalentProperty mo:time ;
              rdfs:isDefinedBy <http://purl.org/ontology/mo/> ;
              vs:term_status "deprecated" .


###  http://purl.org/ontology/mo/similar_to
mo:similar_to rdf:type owl:ObjectProperty ;
              rdfs:domain [ rdf:type owl:Class ;
                            owl:unionOf ( mo:Genre
                                          mo:MusicalExpression
                                          mo:MusicalItem
                                          mo:MusicalManifestation
                                          mo:MusicalWork
                                          foaf:Agent
                                        )
                          ] ;
              rdfs:range [ rdf:type owl:Class ;
                           owl:unionOf ( mo:Genre
                                         mo:MusicalExpression
                                         mo:MusicalItem
                                         mo:MusicalManifestation
                                         mo:MusicalWork
                                         foaf:Agent
                                       )
                         ] ;
              mo:level "1" ;
              rdfs:comment """
            A similarity relationships between two objects (so far, either an agent, a signal or a genre, but
        this could grow).
        This relationship is pretty general and doesn't make any assumptions on how the similarity claim
        was derived.
        Such similarity statements can come from a range of different sources (Musicbrainz similarities between
        artists, or coming from some automatic content analysis).
        However, the origin of such statements should be kept using a named graph approach - and ultimately, the 
        documents providing such statements should attach some metadata to themselves (confidence of the claim, etc.).
        """ ;
              rdfs:isDefinedBy <http://purl.org/ontology/mo/> ;
              rdfs:label "similar_to" ;
              vs:term_status "unstable" .


###  http://purl.org/ontology/mo/singer
mo:singer rdf:type owl:ObjectProperty ;
          rdfs:subPropertyOf mo:performer ;
          rdfs:domain mo:Performance ;
          rdfs:range foaf:Agent ;
          mo:level "2" ;
          rdfs:comment "Relates a performance to an involved singer" ;
          rdfs:isDefinedBy <http://purl.org/ontology/mo/> ;
          vs:term_status "stable" .


###  http://purl.org/ontology/mo/supporting_musician
mo:supporting_musician rdf:type owl:ObjectProperty ;
                       rdfs:domain mo:MusicArtist ;
                       rdfs:range mo:MusicArtist ;
                       mo:level "1" ;
                       rdfs:comment "Used to relate an artist doing long-time instrumental or vocal support for another artist." ;
                       rdfs:isDefinedBy <http://purl.org/ontology/mo/> ;
                       rdfs:label "supporting_musician" ;
                       vs:term_status "unstable" .


###  http://purl.org/ontology/mo/time
mo:time rdf:type owl:ObjectProperty ,
                 owl:FunctionalProperty ;
        rdfs:domain mo:Signal ;
        rdfs:range time:TemporalEntity ;
        mo:level "1" ;
        rdfs:comment """
        Associates a Signal to a time object - its actual domain
    """ ;
        rdfs:isDefinedBy <http://purl.org/ontology/mo/> ;
        rdfs:label "time" ;
        vs:term_status "stable" .


###  http://purl.org/ontology/mo/track
mo:track rdf:type owl:ObjectProperty ;
         rdfs:domain mo:Record ;
         rdfs:range mo:Track ;
         mo:level "1" ;
         rdfs:comment "Indicates a part of a musical manifestation - in this particular case, a track." ;
         rdfs:isDefinedBy <http://purl.org/ontology/mo/> ;
         rdfs:label "track" ;
         vs:term_status "stable" .


###  http://purl.org/ontology/mo/translation_of
mo:translation_of rdf:type owl:ObjectProperty ;
                  rdfs:domain frbr:Expression ;
                  rdfs:range frbr:Expression ;
                  mo:level "1" ;
                  rdfs:comment "Indicates that a work or the expression of a work has translated or transliterated into another expression of a work." ;
                  rdfs:isDefinedBy <http://purl.org/ontology/mo/> ;
                  rdfs:label "translation_of" ;
                  vs:term_status "unstable" .


###  http://purl.org/ontology/mo/tribute_to
mo:tribute_to rdf:type owl:ObjectProperty ;
              rdfs:domain mo:MusicalManifestation ;
              rdfs:range mo:MusicArtist ;
              mo:level "1" ;
              rdfs:comment "Indicates a musical work or the expression of a musical work that is a tribute to an artist - normally consisting of music being composed by the artist but performed by other artists. " ;
              rdfs:isDefinedBy <http://purl.org/ontology/mo/> ;
              rdfs:label "tribute_to" ;
              vs:term_status "unstable" .


###  http://purl.org/ontology/mo/usedInPerformance
mo:usedInPerformance rdf:type owl:ObjectProperty ;
                     rdfs:isDefinedBy <http://purl.org/ontology/mo/> ;
                     vs:term_status "deprecated" .


###  http://purl.org/ontology/mo/usedInRecording
mo:usedInRecording rdf:type owl:ObjectProperty ;
                   rdfs:isDefinedBy <http://purl.org/ontology/mo/> ;
                   vs:term_status "deprecated" .


###  http://purl.org/ontology/mo/usesSound
mo:usesSound rdf:type owl:ObjectProperty ;
             rdfs:isDefinedBy <http://purl.org/ontology/mo/> ;
             vs:term_status "deprecated" .


###  http://purl.org/ontology/mo/usesWork
mo:usesWork rdf:type owl:ObjectProperty ;
            rdfs:isDefinedBy <http://purl.org/ontology/mo/> ;
            vs:term_status "deprecated" .


###  http://purl.org/ontology/mo/want_item
mo:want_item rdf:type owl:ObjectProperty ;
             rdfs:domain foaf:Agent ;
             rdfs:range frbr:Item ;
             mo:level "1" ;
             rdfs:comment "A person, a group of person or an organization wanting an exemplar of a single manifestation." ;
             rdfs:isDefinedBy <http://purl.org/ontology/mo/> ;
             rdfs:label "want_item" ;
             vs:term_status "stable" .


###  http://purl.org/ontology/mo/wikipedia
mo:wikipedia rdf:type owl:ObjectProperty ;
             rdfs:subPropertyOf foaf:isPrimaryTopicOf ;
             rdfs:domain [ rdf:type owl:Class ;
                           owl:unionOf ( mo:Genre
                                         mo:Instrument
                                         frbr:Expression
                                         frbr:Item
                                         frbr:Manifestation
                                         frbr:Work
                                         foaf:Agent
                                       )
                         ] ;
             rdfs:range foaf:Document ;
             mo:level "1" ;
             rdfs:comment """
        Used to link an work, an expression of a work, a manifestation of a work, 
        a person, an instrument or a musical genre to its corresponding WikiPedia page. 
        The full URL should be used, not just the WikiName.
    """ ;
             rdfs:isDefinedBy <http://purl.org/ontology/mo/> ;
             rdfs:label "wikipedia" ;
             vs:term_status "stable" .


###  http://purl.org/vocab/bio/0.1/event
bio:event rdf:type owl:ObjectProperty .


###  http://purl.org/vocab/frbr/core#embodiment
frbr:embodiment rdf:type owl:ObjectProperty .


###  http://purl.org/vocab/frbr/core#exemplar
frbr:exemplar rdf:type owl:ObjectProperty .


###  http://xmlns.com/foaf/0.1/member

#################################################################
#    Data properties
#################################################################

###  http://purl.org/dc/terms/alternative
dcterms:alternative rdfs:subPropertyOf dcterms:title ;
                    rdfs:range rdfs:Literal .


###  http://purl.org/dc/terms/available
dcterms:available rdfs:subPropertyOf dcterms:date ;
                  rdfs:range rdfs:Literal .


###  http://purl.org/dc/terms/bibliographicCitation
dcterms:bibliographicCitation rdfs:subPropertyOf dcterms:identifier ;
                              rdfs:domain dcterms:BibliographicResource ;
                              rdfs:range rdfs:Literal .


###  http://purl.org/dc/terms/created
dcterms:created rdfs:subPropertyOf dcterms:date ;
                rdfs:range rdfs:Literal .


###  http://purl.org/dc/terms/date
dcterms:date rdfs:range rdfs:Literal .


###  http://purl.org/dc/terms/dateAccepted
dcterms:dateAccepted rdfs:subPropertyOf dcterms:date ;
                     rdfs:range rdfs:Literal .


###  http://purl.org/dc/terms/dateCopyrighted
dcterms:dateCopyrighted rdfs:subPropertyOf dcterms:date ;
                        rdfs:range rdfs:Literal .


###  http://purl.org/dc/terms/dateSubmitted
dcterms:dateSubmitted rdfs:subPropertyOf dcterms:date ;
                      rdfs:range rdfs:Literal .


###  http://purl.org/dc/terms/identifier
dcterms:identifier rdfs:range rdfs:Literal .


###  http://purl.org/dc/terms/issued
dcterms:issued rdfs:subPropertyOf dcterms:date ;
               rdfs:range rdfs:Literal .


###  http://purl.org/dc/terms/modified
dcterms:modified rdfs:subPropertyOf dcterms:date ;
                 rdfs:range rdfs:Literal .


###  http://purl.org/dc/terms/title
dcterms:title rdfs:range rdfs:Literal .


###  http://purl.org/dc/terms/valid
dcterms:valid rdfs:subPropertyOf dcterms:date ;
              rdfs:range rdfs:Literal .


###  http://purl.org/ontology/mo/activity_end
mo:activity_end rdf:type owl:DatatypeProperty ;
                rdfs:domain mo:MusicArtist ;
                rdfs:range xsd:date ;
                mo:level "1" ;
                rdfs:comment "Relates an artist to a date at which its activity ended" ;
                rdfs:isDefinedBy <http://purl.org/ontology/mo/> ;
                rdfs:label "activity end" ;
                vs:term_status "testing" .


###  http://purl.org/ontology/mo/activity_start
mo:activity_start rdf:type owl:DatatypeProperty ;
                  rdfs:domain mo:MusicArtist ;
                  rdfs:range xsd:date ;
                  mo:level "1" ;
                  rdfs:comment "Relates an artist to a date at which its activity started" ;
                  rdfs:isDefinedBy <http://purl.org/ontology/mo/> ;
                  rdfs:label "activity start" ;
                  vs:term_status "testing" .


###  http://purl.org/ontology/mo/bitsPerSample
mo:bitsPerSample rdf:type owl:DatatypeProperty ,
                          owl:FunctionalProperty ;
                 rdfs:domain mo:DigitalSignal ;
                 rdfs:range xsd:int ;
                 mo:level "1" ;
                 rdfs:comment """
        Associates a digital signal to the number a bits used to encode one sample. Range is xsd:int.
    """ ;
                 rdfs:isDefinedBy <http://purl.org/ontology/mo/> ;
                 vs:term_status "stable" .


###  http://purl.org/ontology/mo/bpm
mo:bpm rdf:type owl:DatatypeProperty ;
       rdfs:domain [ rdf:type owl:Class ;
                     owl:unionOf ( mo:MusicalWork
                                   mo:Performance
                                   mo:Signal
                                 )
                   ] ;
       rdfs:range xsd:float ;
       mo:level "2" ;
       rdfs:comment """
        Indicates the BPM of a MusicalWork or a particular Performance 
        Beats per minute: the pace of music measured by the number of beats occurring in 60 seconds.
    """ ;
       rdfs:isDefinedBy <http://purl.org/ontology/mo/> ;
       rdfs:label "bpm" ;
       vs:term_status "stable" .


###  http://purl.org/ontology/mo/catalogue_number
mo:catalogue_number rdf:type owl:DatatypeProperty ;
                    rdfs:subPropertyOf mo:uuid ;
                    rdfs:domain mo:Release ;
                    rdfs:range xsd:string ;
                    mo:level "1" ;
                    rdfs:comment "Links a release with the corresponding catalogue number" ;
                    rdfs:isDefinedBy <http://purl.org/ontology/mo/> ;
                    rdfs:label "catalogue number" ;
                    vs:term_status "testing" .


###  http://purl.org/ontology/mo/channels
mo:channels rdf:type owl:DatatypeProperty ,
                     owl:FunctionalProperty ;
            rdfs:domain mo:Signal ;
            rdfs:range xsd:int ;
            mo:level "1" ;
            rdfs:comment """
        Associates a signal to the number of channels it holds (mono --> 1, stereo --> 2). Range is xsd:int.
    """ ;
            rdfs:isDefinedBy <http://purl.org/ontology/mo/> ;
            vs:term_status "stable" .


###  http://purl.org/ontology/mo/duration
mo:duration rdf:type owl:DatatypeProperty ;
            rdfs:domain [ rdf:type owl:Class ;
                          owl:unionOf ( mo:Signal
                                        mo:Track
                                      )
                        ] ;
            rdfs:range xsd:float ;
            mo:level "1" ;
            rdfs:comment "The duration of a track or a signal in ms" ;
            rdfs:isDefinedBy <http://purl.org/ontology/mo/> ;
            vs:term_status "testing" .


###  http://purl.org/ontology/mo/ean
mo:ean rdf:type owl:DatatypeProperty ;
       rdfs:subPropertyOf mo:gtin ;
       rdfs:domain mo:Release ;
       rdfs:range xsd:string ;
       mo:level "1" ;
       rdfs:comment "The European Article Number (EAN) is a universal identifier for products, commonly printed in form of barcodes on them. The numbers represented by those codes can either be 8 or 13 digits long, with the 13-digit-version being most common. EANs form a superset of the North American Universal Product Code (UPC) as every UPC can be made an EAN by adding a leading zero to it. Additionally every EAN is also a Japanese Article Number (JAN). The identifiers were formerly assigned by EAN International which merged with Uniform Code Council (UCC, the guys behind the UPCs) and Electronic Commerce Council of Canada (ECCC) to become GS1. " ;
       rdfs:isDefinedBy <http://purl.org/ontology/mo/> ;
       rdfs:label "ean" ;
       vs:term_status "testing" .


###  http://purl.org/ontology/mo/encoding
mo:encoding rdf:type owl:DatatypeProperty ;
            rdfs:domain mo:AudioFile ;
            rdfs:range rdfs:Literal ;
            mo:level "1" ;
            rdfs:comment "Method used to convert analog electronic signals into digital format such as \"MP3 CBR @ 128kbps\", \"OGG @ 160kbps\", \"FLAC\", etc." ;
            rdfs:isDefinedBy <http://purl.org/ontology/mo/> ;
            rdfs:label "encoding" ;
            vs:term_status "unstable" .


###  http://purl.org/ontology/mo/grid
mo:grid rdf:type owl:DatatypeProperty ;
        rdfs:subPropertyOf mo:uuid ;
        rdfs:domain mo:Release ;
        rdfs:range xsd:string ;
        mo:level "1" ;
        rdfs:comment "The Global Release Identifier (GRid) is a system for uniquely identifying Releases of music over electronic networks (that is, online stores where you can buy music as digital files). As that it can be seen as the equivalent of the BarCode (or more correctly the GTIN) as found on physical releases of music. Like the ISRC (a code for identifying single recordings as found on releases) it was developed by the IFPI but it does not appear to be a standard of the ISO." ;
        rdfs:isDefinedBy <http://purl.org/ontology/mo/> ;
        rdfs:label "GRid" ;
        vs:term_status "testing" .


###  http://purl.org/ontology/mo/gtin
mo:gtin rdf:type owl:DatatypeProperty ;
        rdfs:domain mo:Release ;
        rdfs:range xsd:string ;
        mo:level "1" ;
        rdfs:comment "GTIN is a grouping term for EANs and UPCs. In common speech those are called barcodes although the barcodes are just a representation of those identifying numbers." ;
        rdfs:isDefinedBy <http://purl.org/ontology/mo/> ;
        rdfs:label "gtin" ;
        vs:term_status "testing" .


###  http://purl.org/ontology/mo/ipi
mo:ipi rdf:type owl:DatatypeProperty ;
       rdfs:subPropertyOf mo:uuid ;
       rdfs:domain mo:MusicArtist ;
       rdfs:range xsd:string ;
       mo:level "1" ;
       rdfs:comment "The Interested Parties Information Code (IPI) is an ISO standard similar to ISBNs for identifying the people or groups with some involvement with a particular musical work / compositions." ;
       rdfs:isDefinedBy <http://purl.org/ontology/mo/> ;
       rdfs:label "ipi" ;
       vs:term_status "testing" .


###  http://purl.org/ontology/mo/ismn
mo:ismn rdf:type owl:DatatypeProperty ;
        rdfs:subPropertyOf mo:uuid ;
        rdfs:domain [ rdf:type owl:Class ;
                      owl:unionOf ( mo:PublishedLibretto
                                    mo:PublishedLyrics
                                    mo:PublishedScore
                                  )
                    ] ;
        rdfs:range xsd:string ;
        mo:level "1" ;
        rdfs:comment "The International Standard Music Number (ISMN) is an ISO standard similar to ISBNs for identifying printed music publications" ;
        rdfs:isDefinedBy <http://purl.org/ontology/mo/> ;
        rdfs:label "ismn" ;
        vs:term_status "testing" .


###  http://purl.org/ontology/mo/isrc
mo:isrc rdf:type owl:DatatypeProperty ;
        rdfs:subPropertyOf mo:uuid ;
        rdfs:domain mo:Signal ;
        rdfs:range xsd:string ;
        mo:level "1" ;
        rdfs:comment """
    The ISRC (International Standard Recording Code) is the international identification system for sound recordings and music videorecordings. 
    Each ISRC is a unique and permanent identifier for a specific recording which can be permanently encoded into a product as its digital fingerprint. 
    Encoded ISRC provide the means to automatically identify recordings for royalty payments.
    """ ;
        rdfs:isDefinedBy <http://purl.org/ontology/mo/> ;
        rdfs:label "isrc" ;
        vs:term_status "stable" .


###  http://purl.org/ontology/mo/iswc
mo:iswc rdf:type owl:DatatypeProperty ;
        rdfs:subPropertyOf mo:uuid ;
        rdfs:domain mo:MusicalWork ;
        rdfs:range xsd:string ;
        mo:level "1" ;
        rdfs:comment "Links a musical work to the corresponding ISWC number" ;
        rdfs:isDefinedBy <http://purl.org/ontology/mo/> ;
        rdfs:label "iswc" ;
        vs:term_status "testing" .


###  http://purl.org/ontology/mo/lc
mo:lc rdf:type owl:DatatypeProperty ;
      rdfs:subPropertyOf mo:uuid ;
      rdfs:domain mo:Label ;
      rdfs:range xsd:string ;
      mo:level "1" ;
      rdfs:comment "The Label Code (LC) was introduced in 1977 by the IFPI (International Federation of Phonogram and Videogram Industries) in order to unmistakably identify the different record labels (see Introduction, Record labels) for rights purposes. The Label Code consists historically of 4 figures, presently being extended to 5 figures, preceded by LC and a dash (e.g. LC-0193 = Electrola; LC-0233 = His Master's Voice). Note that the number of countries using the LC is limited, and that the code given on the item is not always accurate." ;
      rdfs:isDefinedBy <http://purl.org/ontology/mo/> ;
      rdfs:label "lc" ;
      vs:term_status "testing" .


###  http://purl.org/ontology/mo/meter
mo:meter rdf:type owl:DatatypeProperty ;
         rdfs:domain [ rdf:type owl:Class ;
                       owl:unionOf ( mo:MusicalWork
                                     mo:Score
                                   )
                     ] ;
         mo:level "2" ;
         rdfs:comment "Associates a musical work or a score with its meter" ;
         rdfs:isDefinedBy <http://purl.org/ontology/mo/> ;
         rdfs:label "meter" ;
         vs:term_status "testing" .


###  http://purl.org/ontology/mo/movementNum
mo:movementNum rdf:type owl:DatatypeProperty ;
               owl:equivalentProperty mo:movement_number .


###  http://purl.org/ontology/mo/movement_number
mo:movement_number rdf:type owl:DatatypeProperty ;
                   rdfs:domain mo:Movement ;
                   rdfs:range xsd:int ;
                   mo:level "2" ;
                   rdfs:comment "Indicates the position of a movement in a musical work." ;
                   rdfs:isDefinedBy <http://purl.org/ontology/mo/> ;
                   rdfs:label "movement number" ;
                   vs:term_status "unstable" .


###  http://purl.org/ontology/mo/musicbrainz_guid
mo:musicbrainz_guid rdf:type owl:DatatypeProperty ;
                    rdfs:subPropertyOf mo:uuid ;
                    rdfs:domain [ rdf:type owl:Class ;
                                  owl:unionOf ( mo:Label
                                                mo:MusicArtist
                                                mo:Record
                                                mo:ReleaseEvent
                                                mo:Signal
                                                mo:SignalGroup
                                                mo:Track
                                              )
                                ] ;
                    mo:level "1" ;
                    rdfs:comment "Links an object to the corresponding Musicbrainz identifier" ;
                    rdfs:isDefinedBy <http://purl.org/ontology/mo/> ;
                    rdfs:label "Musicbrainz GUID" ;
                    vs:term_status "testing" .


###  http://purl.org/ontology/mo/opus
mo:opus rdf:type owl:DatatypeProperty ;
        rdfs:domain mo:MusicalWork ;
        rdfs:range rdfs:Literal ;
        mo:level "2" ;
        rdfs:comment """
        Used to define a creative work, especially a musical composition numbered to designate the order of a composer's works.
    """ ;
        rdfs:isDefinedBy <http://purl.org/ontology/mo/> ;
        rdfs:label "opus" ;
        vs:term_status "stable" .


###  http://purl.org/ontology/mo/puid
mo:puid rdf:type owl:DatatypeProperty ;
        rdfs:domain mo:Signal ;
        rdfs:range xsd:string ;
        mo:level "1" ;
        rdfs:comment """
        Link a signal to the PUIDs associated with it, that is, PUID computed from MusicalItems (mo:AudioFile) 
        derived from this signal.
        PUIDs (Portable Unique IDentifier) are the IDs used in the 
        proprietary MusicDNS AudioFingerprinting system which is operated by MusicIP.

        Using PUIDs, one (with some luck) can identify the Signal object associated with a particular audio file, therefore allowing
        to access further information (on which release this track is featured? etc.). Using some more metadata one can identify
        the particular Track corresponding to the audio file (a track on a particular release).""" ;
        rdfs:isDefinedBy <http://purl.org/ontology/mo/> ;
        rdfs:label "puid" ;
        vs:term_status "stable" .


###  http://purl.org/ontology/mo/record_count
mo:record_count rdf:type owl:DatatypeProperty ;
                rdfs:domain mo:Release ;
                rdfs:range xsd:int ;
                mo:level "1" ;
                rdfs:comment "Associates a release with the number of records it contains, e.g. the number of discs it contains in the case of a multi-disc release." ;
                rdfs:isDefinedBy <http://purl.org/ontology/mo/> ;
                rdfs:label "record count" ;
                vs:term_status "testing" .


###  http://purl.org/ontology/mo/record_number
mo:record_number rdf:type owl:DatatypeProperty ;
                 rdfs:domain mo:Record ;
                 rdfs:range xsd:nonNegativeInteger ;
                 mo:level "1" ;
                 rdfs:comment "Indicates the position of a record in a release (e.g. a 2xLP, etc.)." ;
                 rdfs:isDefinedBy <http://purl.org/ontology/mo/> ;
                 rdfs:label "has record number" ;
                 vs:term_status "testing" .


###  http://purl.org/ontology/mo/record_side
mo:record_side rdf:type owl:DatatypeProperty ;
               rdfs:domain mo:Track ;
               rdfs:range xsd:string ;
               mo:level "1" ;
               rdfs:comment """Associates the side on a vinyl record, where a track is located, e.g. A, B, C, etc. This property can then also be used 
in conjunction with mo:track_number, so that one can infer e.g. \"A1\", that means, track number 1 on side A.""" ;
               rdfs:isDefinedBy <http://purl.org/ontology/mo/> ;
               rdfs:label "has record side" ;
               vs:term_status "testing" .


###  http://purl.org/ontology/mo/sampleRate
mo:sampleRate rdf:type owl:DatatypeProperty ;
              owl:equivalentProperty mo:sample_rate ;
              vs:term_status "deprecated" .


###  http://purl.org/ontology/mo/sample_rate
mo:sample_rate rdf:type owl:DatatypeProperty ,
                        owl:FunctionalProperty ;
               rdfs:domain mo:DigitalSignal ;
               rdfs:range xsd:float ;
               mo:level "1" ;
               rdfs:comment """
        Associates a digital signal to its sample rate. It might be easier to express it this way instead of
        defining a timeline map:-) Range is xsd:float.
    """ ;
               rdfs:isDefinedBy <http://purl.org/ontology/mo/> ;
               vs:term_status "stable" .


###  http://purl.org/ontology/mo/tempo
mo:tempo rdf:type owl:DatatypeProperty ;
         rdfs:domain [ rdf:type owl:Class ;
                       owl:unionOf ( mo:MusicalWork
                                     mo:Performance
                                     mo:Signal
                                   )
                     ] ;
         rdfs:range xsd:string ;
         mo:level "2" ;
         rdfs:comment """
        Rate of speed or pace of music. Tempo markings are traditionally given in Italian; 
        common markings include: grave (solemn; very, very slow); largo (broad; very slow); 
        adagio (quite slow); andante (a walking pace); moderato (moderate); allegro (fast; cheerful); 
        vivace (lively); presto (very fast); accelerando (getting faster); ritardando (getting slower); 
        and a tempo (in time; returning to the original pace).
    """ ;
         rdfs:isDefinedBy <http://purl.org/ontology/mo/> ;
         rdfs:label "tempo" ;
         vs:term_status "stable" .


###  http://purl.org/ontology/mo/text
mo:text rdf:type owl:DatatypeProperty ;
        rdfs:domain mo:Lyrics ;
        mo:level "2" ;
        rdfs:comment "Associates lyrics with their text." ;
        rdfs:isDefinedBy <http://purl.org/ontology/mo/> ;
        rdfs:label "text" ;
        vs:term_status "testing" .


###  http://purl.org/ontology/mo/trackNum
mo:trackNum rdf:type owl:DatatypeProperty ;
            owl:equivalentProperty mo:track_number ;
            rdfs:isDefinedBy <http://purl.org/ontology/mo/> ;
            vs:term_status "deprecated" .


###  http://purl.org/ontology/mo/track_count
mo:track_count rdf:type owl:DatatypeProperty ;
               rdfs:domain mo:Record ;
               rdfs:range xsd:int ;
               mo:level "1" ;
               rdfs:comment "The track count of a record" ;
               rdfs:isDefinedBy <http://purl.org/ontology/mo/> ;
               rdfs:label "track count" ;
               vs:term_status "testing" .


###  http://purl.org/ontology/mo/track_number
mo:track_number rdf:type owl:DatatypeProperty ;
                rdfs:domain mo:Track ;
                rdfs:range xsd:nonNegativeInteger ;
                mo:level "1" ;
                rdfs:comment "Indicates the position of a track on a record medium (a CD, etc.)." ;
                rdfs:isDefinedBy <http://purl.org/ontology/mo/> ;
                rdfs:label "track number" ;
                vs:term_status "stable" .


###  http://purl.org/ontology/mo/trmid
mo:trmid rdf:type owl:DatatypeProperty ;
         rdfs:domain mo:Signal ;
         rdfs:range xsd:string ;
         mo:level "1" ;
         rdfs:comment """
        Indicates the TRMID of a track.
        TRM IDs are MusicBrainz' old AudioFingerprinting system. 
        TRM (TRM Recognizes Music) IDs are (somewhat) unique ids that represent 
        the audio signature of a musical piece (see AudioFingerprint).
    """ ;
         rdfs:isDefinedBy <http://purl.org/ontology/mo/> ;
         rdfs:label "trmid" ;
         vs:term_status "stable" .


###  http://purl.org/ontology/mo/upc
mo:upc rdf:type owl:DatatypeProperty ;
       rdfs:subPropertyOf mo:gtin ;
       rdfs:domain mo:Release ;
       rdfs:range xsd:string ;
       mo:level "1" ;
       rdfs:comment "UPC stands for \"Universal Product Code\", which was the original barcode used in the United States and Canada. The UPC (now officially EAN.UCC-12 is a numerical method of identifying products without redundancy worldwide for all types of products in the retail sector. The EAN is a superset of the original UPC increasing the digits to 13 with the prefix 0 reserved for UPC. As of 2005, manufacturers are only allowed to use the new 13-digit codes on their items, rather than having two separate numbers." ;
       rdfs:isDefinedBy <http://purl.org/ontology/mo/> ;
       rdfs:label "upc" ;
       vs:term_status "testing" .


###  http://purl.org/ontology/mo/uuid
mo:uuid rdf:type owl:DatatypeProperty ;
        rdfs:subPropertyOf dcterms:identifier ;
        rdfs:domain owl:Thing ;
        mo:level "1" ;
        rdfs:comment """
            Links an object to an universally unique identifier for it.
    """ ;
        rdfs:label "universally unique identifier" ;
        vs:term_status "testing" .


#################################################################
#    Classes
#################################################################

###  http://purl.org/dc/terms/Agent
dcterms:Agent rdf:type owl:Class .


###  http://purl.org/dc/terms/AgentClass
dcterms:AgentClass rdf:type owl:Class ;
                   rdfs:subClassOf rdfs:Class .


###  http://purl.org/dc/terms/BibliographicResource
dcterms:BibliographicResource rdf:type owl:Class .


###  http://purl.org/dc/terms/FileFormat
dcterms:FileFormat rdf:type owl:Class ;
                   rdfs:subClassOf dcterms:MediaType .


###  http://purl.org/dc/terms/Frequency
dcterms:Frequency rdf:type owl:Class .


###  http://purl.org/dc/terms/Jurisdiction
dcterms:Jurisdiction rdf:type owl:Class ;
                     rdfs:subClassOf dcterms:LocationPeriodOrJurisdiction .


###  http://purl.org/dc/terms/LicenseDocument
dcterms:LicenseDocument rdf:type owl:Class ;
                        rdfs:subClassOf dcterms:RightsStatement .


###  http://purl.org/dc/terms/LinguisticSystem
dcterms:LinguisticSystem rdf:type owl:Class .


###  http://purl.org/dc/terms/Location
dcterms:Location rdf:type owl:Class ;
                 rdfs:subClassOf dcterms:LocationPeriodOrJurisdiction .


###  http://purl.org/dc/terms/LocationPeriodOrJurisdiction
dcterms:LocationPeriodOrJurisdiction rdf:type owl:Class .


###  http://purl.org/dc/terms/MediaType
dcterms:MediaType rdf:type owl:Class ;
                  rdfs:subClassOf dcterms:MediaTypeOrExtent .


###  http://purl.org/dc/terms/MediaTypeOrExtent
dcterms:MediaTypeOrExtent rdf:type owl:Class .


###  http://purl.org/dc/terms/MethodOfAccrual
dcterms:MethodOfAccrual rdf:type owl:Class .


###  http://purl.org/dc/terms/MethodOfInstruction
dcterms:MethodOfInstruction rdf:type owl:Class .


###  http://purl.org/dc/terms/PeriodOfTime
dcterms:PeriodOfTime rdf:type owl:Class ;
                     rdfs:subClassOf dcterms:LocationPeriodOrJurisdiction .


###  http://purl.org/dc/terms/PhysicalMedium
dcterms:PhysicalMedium rdf:type owl:Class ;
                       rdfs:subClassOf dcterms:MediaType .


###  http://purl.org/dc/terms/PhysicalResource
dcterms:PhysicalResource rdf:type owl:Class .


###  http://purl.org/dc/terms/Policy
dcterms:Policy rdf:type owl:Class .


###  http://purl.org/dc/terms/ProvenanceStatement
dcterms:ProvenanceStatement rdf:type owl:Class .


###  http://purl.org/dc/terms/RightsStatement
dcterms:RightsStatement rdf:type owl:Class .


###  http://purl.org/dc/terms/SizeOrDuration
dcterms:SizeOrDuration rdf:type owl:Class ;
                       rdfs:subClassOf dcterms:MediaTypeOrExtent .


###  http://purl.org/dc/terms/Standard
dcterms:Standard rdf:type owl:Class .


###  http://purl.org/ontology/mo/Activity
mo:Activity rdf:type owl:Class ;
            rdfs:subClassOf event:Event ;
            mo:level "1" ;
            rdfs:comment """
        An activity period, defining when an artist was musically active.
    """ ;
            rdfs:isDefinedBy <http://purl.org/ontology/mo/> ;
            rdfs:label "activity" ;
            vs:term_status "testing" .


###  http://purl.org/ontology/mo/AnalogSignal
mo:AnalogSignal rdf:type owl:Class ;
                rdfs:subClassOf mo:Signal ;
                owl:disjointWith mo:DigitalSignal ;
                mo:level "2" ;
                rdfs:comment """
        An analog signal.
    """ ;
                rdfs:isDefinedBy <http://purl.org/ontology/mo/> ;
                rdfs:label "analogue signal" ;
                vs:term_status "stable" .


###  http://purl.org/ontology/mo/Arrangement
mo:Arrangement rdf:type owl:Class ;
               rdfs:subClassOf event:Event ;
               mo:level "2" ;
               rdfs:comment """
        An arrangement event.
        Takes as agent the arranger, and produces a score (informational object, not the actually published score).
    """ ;
               rdfs:isDefinedBy <http://purl.org/ontology/mo/> ;
               rdfs:label "arrangement" ;
               vs:term_status "stable" .


###  http://purl.org/ontology/mo/Arranger
mo:Arranger rdf:type owl:Class ;
            owl:equivalentClass [ rdf:type owl:Restriction ;
                                  owl:onProperty event:isAgentIn ;
                                  owl:someValuesFrom mo:Arrangement
                                ] ;
            rdfs:subClassOf foaf:Agent ;
            mo:level "2" ;
            rdfs:label "arranger" ;
            vs:term_status "unstable" .


###  http://purl.org/ontology/mo/AudioFile
mo:AudioFile rdf:type owl:Class ;
             rdfs:subClassOf mo:Medium ,
                             foaf:Document ;
             mo:level "1" ;
             rdfs:comment "An audio file, which may be available on a local file system or through http, ftp, etc." ;
             rdfs:isDefinedBy <http://purl.org/ontology/mo/> ;
             rdfs:label "audio file" ;
             vs:term_status "unstable" .


###  http://purl.org/ontology/mo/CD
mo:CD rdf:type owl:Class ;
      rdfs:subClassOf mo:Medium ;
      mo:level "1" ;
      rdfs:comment "Compact Disc used as medium to record a musical manifestation." ;
      rdfs:isDefinedBy <http://purl.org/ontology/mo/> ;
      rdfs:label "CD" ;
      vs:term_status "unstable" .


###  http://purl.org/ontology/mo/Composer
mo:Composer rdf:type owl:Class ;
            owl:equivalentClass [ rdf:type owl:Restriction ;
                                  owl:onProperty event:isAgentIn ;
                                  owl:someValuesFrom mo:Composition
                                ] ;
            rdfs:subClassOf foaf:Agent ;
            mo:level "2" ;
            rdfs:label "composer" ;
            vs:term_status "unstable" .


###  http://purl.org/ontology/mo/Composition
mo:Composition rdf:type owl:Class ;
               rdfs:subClassOf event:Event ;
               mo:level "2" ;
               rdfs:comment """
        A composition event.
        Takes as agent the composer himself.
        It produces a MusicalWork, or a MusicalExpression (when the initial \"product\" is a score, for example), or both...
    """ ;
               rdfs:isDefinedBy <http://purl.org/ontology/mo/> ;
               rdfs:label "composition" ;
               vs:term_status "stable" .


###  http://purl.org/ontology/mo/Conductor
mo:Conductor rdf:type owl:Class ;
             owl:equivalentClass [ rdf:type owl:Restriction ;
                                   owl:onProperty mo:conducted ;
                                   owl:someValuesFrom mo:Performance
                                 ] ;
             rdfs:subClassOf foaf:Agent ;
             mo:level "2" ;
             rdfs:label "conductor" ;
             vs:term_status "unstable" .


###  http://purl.org/ontology/mo/CorporateBody
mo:CorporateBody rdf:type owl:Class ;
                 rdfs:subClassOf foaf:Organization ;
                 mo:level "1" ;
                 rdfs:comment "Organization or group of individuals and/or other organizations involved in the music market." ;
                 rdfs:isDefinedBy <http://purl.org/ontology/mo/> ;
                 rdfs:label "corporate body" ;
                 vs:term_status "stable" .


###  http://purl.org/ontology/mo/DAT
mo:DAT rdf:type owl:Class ;
       rdfs:subClassOf mo:Medium ;
       mo:level "1" ;
       rdfs:comment "Digital Audio Tape used as medium to record a musical manifestation." ;
       rdfs:isDefinedBy <http://purl.org/ontology/mo/> ;
       rdfs:label "DAT" ;
       vs:term_status "unstable" .


###  http://purl.org/ontology/mo/DCC
mo:DCC rdf:type owl:Class ;
       rdfs:subClassOf mo:Medium ;
       mo:level "1" ;
       rdfs:comment "Digital Compact Cassette used as medium to record a musical manifestation." ;
       rdfs:isDefinedBy <http://purl.org/ontology/mo/> ;
       rdfs:label "DCC" ;
       vs:term_status "unstable" .


###  http://purl.org/ontology/mo/DVDA
mo:DVDA rdf:type owl:Class ;
        rdfs:subClassOf mo:Medium ;
        mo:level "1" ;
        rdfs:comment "DVD-Audio used as medium to record a musical manifestation." ;
        rdfs:isDefinedBy <http://purl.org/ontology/mo/> ;
        rdfs:label "DVDA" ;
        vs:term_status "unstable" .


###  http://purl.org/ontology/mo/DigitalSignal
mo:DigitalSignal rdf:type owl:Class ;
                 rdfs:subClassOf mo:Signal ;
                 mo:level "2" ;
                 rdfs:comment """
        A digital signal
    """ ;
                 rdfs:isDefinedBy <http://purl.org/ontology/mo/> ;
                 rdfs:label "digital signal" ;
                 vs:term_status "stable" .


###  http://purl.org/ontology/mo/ED2K
mo:ED2K rdf:type owl:Class ;
        rdfs:subClassOf mo:Medium ;
        mo:level "1" ;
        rdfs:comment "Something available on the E-Donkey peer-2-peer filesharing network" ;
        rdfs:isDefinedBy <http://purl.org/ontology/mo/> ;
        rdfs:label "ED2K" ;
        vs:term_status "unstable" .


###  http://purl.org/ontology/mo/Festival
mo:Festival rdf:type owl:Class ;
            rdfs:subClassOf event:Event ;
            mo:level "2" ;
            rdfs:comment """
        A festival - musical/artistic event lasting several days, like Glastonbury, Rock Am Ring...
        We migth decompose this event (which is in fact just a classification of the space/time region related to 
        a particular festival) using hasSubEvent in several performances at different space/time.
    """ ;
            rdfs:isDefinedBy <http://purl.org/ontology/mo/> ;
            rdfs:label "Festival" ;
            vs:term_status "stable" .


###  http://purl.org/ontology/mo/Genre
mo:Genre rdf:type owl:Class ;
         mo:level "2" ;
         rdfs:comment """
        An expressive style of music.
        
        Any taxonomy can be plug-in here. You can either define a genre by yourself, like this:

        :mygenre a mo:Genre; dc:title \"electro rock\".

        Or you can refer to a DBPedia genre (such as http://dbpedia.org/resource/Baroque_music), allowing semantic web
        clients to access easily really detailed structured information about the genre you are refering to.
    """ ;
         rdfs:isDefinedBy <http://purl.org/ontology/mo/> ;
         rdfs:label "Genre" ;
         vs:term_status "stable" .


###  http://purl.org/ontology/mo/Instrument
mo:Instrument rdf:type owl:Class ;
              mo:level "2" ;
              rdfs:comment """
        Any of various devices or contrivances that can be used to produce musical tones or sound.
        
        Any taxonomy can be used to subsume this concept. The default one is one extracted by Ivan Herman
        from the Musicbrainz instrument taxonomy, conforming to SKOS. This concept holds a seeAlso link 
        towards this taxonomy.
    """ ;
              rdfs:isDefinedBy <http://purl.org/ontology/mo/> ;
              rdfs:label "Instrument" ;
              rdfs:seeAlso <http://purl.org/ontology/mo/mit#> ;
              vs:term_status "stable" .


###  http://purl.org/ontology/mo/Instrumentation
mo:Instrumentation rdf:type owl:Class ;
                   rdfs:subClassOf mo:Arrangement ;
                   mo:level "2" ;
                   rdfs:comment """
        Instrumentation deals with the techniques of writing music for a specific instrument, 
        including the limitations of the instrument, playing techniques and idiomatic handling of the instrument.
    """ ;
                   rdfs:isDefinedBy <http://purl.org/ontology/mo/> ;
                   rdfs:label "instrumentation" ;
                   vs:term_status "stable" .


###  http://purl.org/ontology/mo/Label
mo:Label rdf:type owl:Class ;
         rdfs:subClassOf mo:CorporateBody ;
         mo:level "1" ;
         rdfs:comment "Trade name of a company that produces musical works or expression of musical works." ;
         rdfs:isDefinedBy <http://purl.org/ontology/mo/> ;
         rdfs:label "label" ;
         vs:term_status "stable" .


###  http://purl.org/ontology/mo/Libretto
mo:Libretto rdf:type owl:Class ;
            rdfs:subClassOf mo:MusicalExpression ;
            mo:level "2" ;
            rdfs:comment """
                Libretto
        """ ;
            rdfs:isDefinedBy <http://purl.org/ontology/mo/> ;
            rdfs:label "libretto" ;
            vs:term_status "stable" .


###  http://purl.org/ontology/mo/Listener
mo:Listener rdf:type owl:Class ;
            owl:equivalentClass [ rdf:type owl:Restriction ;
                                  owl:onProperty mo:listened ;
                                  owl:someValuesFrom mo:Performance
                                ] ;
            rdfs:subClassOf foaf:Agent ;
            mo:level "2" ;
            rdfs:label "listened" ;
            vs:term_status "unstable" .


###  http://purl.org/ontology/mo/Lyrics
mo:Lyrics rdf:type owl:Class ;
          rdfs:subClassOf mo:MusicalExpression ;
          mo:level "2" ;
          rdfs:comment """
        Lyrics
    """ ;
          rdfs:isDefinedBy <http://purl.org/ontology/mo/> ;
          rdfs:label "lyrics" ;
          vs:term_status "stable" .


###  http://purl.org/ontology/mo/MD
mo:MD rdf:type owl:Class ;
      rdfs:subClassOf mo:Medium ;
      mo:level "1" ;
      rdfs:comment "Mini Disc used as medium to record a musical manifestation." ;
      rdfs:isDefinedBy <http://purl.org/ontology/mo/> ;
      rdfs:label "MD" ;
      vs:term_status "unstable" .


###  http://purl.org/ontology/mo/MagneticTape
mo:MagneticTape rdf:type owl:Class ;
                rdfs:subClassOf mo:Medium ;
                mo:level "1" ;
                rdfs:comment "Magnetic analogue tape used as medium to record a musical manifestation." ;
                rdfs:isDefinedBy <http://purl.org/ontology/mo/> ;
                rdfs:label "MagneticTape" ;
                vs:term_status "unstable" .


###  http://purl.org/ontology/mo/Medium
mo:Medium rdf:type owl:Class ;
          rdfs:subClassOf mo:MusicalItem ;
          mo:level "1" ;
          rdfs:comment "A means or instrumentality for storing or communicating musical manifestation." ;
          rdfs:isDefinedBy <http://purl.org/ontology/mo/> ;
          rdfs:label "Medium" ;
          vs:term_status "unstable" .


###  http://purl.org/ontology/mo/Membership
mo:Membership rdf:type owl:Class ;
              rdfs:subClassOf event:Event ;
              mo:level "1" ;
              rdfs:comment "A membership event, where one or several people belongs to a group during a particular time period." ;
              rdfs:isDefinedBy <http://purl.org/ontology/mo/> ;
              rdfs:label "membership" ;
              vs:term_status "testing" .


###  http://purl.org/ontology/mo/Movement
mo:Movement rdf:type owl:Class ;
            rdfs:subClassOf mo:MusicalWork ;
            mo:level "2" ;
            rdfs:comment """A movement is a self-contained part of a musical work. While individual or selected movements from a composition are sometimes performed separately, a performance of the complete work requires all the movements to be performed in succession.

Often a composer attempts to interrelate the movements thematically, or sometimes in more subtle ways, in order that the individual
movements exert a cumulative effect. In some forms, composers sometimes link the movements, or ask for them to be played without a
pause between them.
    """ ;
            rdfs:isDefinedBy <http://purl.org/ontology/mo/> ;
            rdfs:label "movement" ;
            vs:term_status "unstable" .


###  http://purl.org/ontology/mo/MusicArtist
mo:MusicArtist rdf:type owl:Class ;
               rdfs:subClassOf foaf:Agent ;
               mo:level "1" ;
               rdfs:comment """
        A person or a group of people (or a computer :-) ), whose musical 
        creative work shows sensitivity and imagination 
    """ ;
               rdfs:isDefinedBy <http://purl.org/ontology/mo/> ;
               rdfs:label "music artist" ;
               vs:term_status "stable" .


###  http://purl.org/ontology/mo/MusicGroup
mo:MusicGroup rdf:type owl:Class ;
              rdfs:subClassOf mo:MusicArtist ,
                              foaf:Group ;
              mo:level "1" ;
              rdfs:comment "Group of musicians, or musical ensemble, usually popular or folk, playing parts of or improvising off of a musical arrangement. " ;
              rdfs:isDefinedBy <http://purl.org/ontology/mo/> ;
              rdfs:label "music group" ;
              vs:term_status "stable" .


###  http://purl.org/ontology/mo/MusicalExpression
mo:MusicalExpression rdf:type owl:Class ;
                     rdfs:subClassOf frbr:Expression ;
                     mo:level "1" ;
                     rdfs:comment """
The intellectual or artistic realization of a work in the form of alpha-numeric, musical, or choreographic notation, sound, etc., or any combination of such forms.    


For example:

Work #1 Franz Schubert's Trout quintet

    * Expression #1 the composer's score
    * Expression #2 sound issued from the performance by the Amadeus Quartet and Hephzibah Menuhin on piano
    * Expression #3 sound issued from the performance by the Cleveland Quartet and Yo-Yo Ma on the cello
    * . . . . 

The Music Ontology defines the following sub-concepts of a MusicalExpression, which should be used instead of MusicalExpression itself: Score (the
result of an arrangement), Sound (produced during a performance), Signal. However, it is possible to stick to FRBR and bypass the worflow
mechanism this ontology defines by using the core FRBR properties on such objects. But it is often better to use events to interconnect such 
expressions (allowing to go deeply into the production process - `this performer was playing this particular instrument at that
particular time').
    
    """ ;
                     rdfs:isDefinedBy <http://purl.org/ontology/mo/> ;
                     rdfs:label "musical expression" ;
                     vs:term_status "unstable" .


###  http://purl.org/ontology/mo/MusicalItem
mo:MusicalItem rdf:type owl:Class ;
               mo:level "1" ;
               rdfs:comment """A single exemplar of a musical expression.
    
For example, it could be a single exemplar of a CD. This is normally an single object (a CD) possessed by somebody.

From the FRBR final report: The entity defined as item is a concrete entity. It is in many instances a single physical object (e.g., a copy of a one-volume monograph, a single audio cassette, etc.). There are instances, however, where the entity defined as item comprises more than one physical object (e.g., a monograph issued as two separately bound volumes, a recording issued on three separate compact discs, etc.).

In terms of intellectual content and physical form, an item exemplifying a manifestation is normally the same as the manifestation itself. However, variations may occur from one item to another, even when the items exemplify the same manifestation, where those variations are the result of actions external to the intent of the producer of the manifestation (e.g., damage occurring after the item was produced, binding performed by a library, etc.). 
    """ ;
               rdfs:isDefinedBy <http://purl.org/ontology/mo/> ;
               rdfs:label "MusicalItem" ;
               vs:term_status "unstable" .


###  http://purl.org/ontology/mo/MusicalManifestation
mo:MusicalManifestation rdf:type owl:Class ;
                        rdfs:subClassOf frbr:Manifestation ;
                        mo:level "1" ;
                        rdfs:comment """

This entity is related to the edition/production/publication of a musical expression (musical manifestation are closely related with the music industry (their terms, concepts, definitions, methods (production, publication, etc.), etc.)
    
From the FRBR final report: The entity defined as manifestation encompasses a wide range of materials, including manuscripts, books, periodicals, maps, posters, sound recordings, films, video recordings, CD-ROMs, multimedia kits, etc. As an entity, manifestation represents all the physical objects that bear the same characteristics, in respect to both intellectual content and physical form.


Work #1 J. S. Bach's Six suites for unaccompanied cello

    * Expression #1 sound issued during the performance by Janos Starker recorded in 1963 and 1965
          o Manifestation #1 recordings released on 33 1/3 rpm sound discs in 1965 by Mercury
          o Manifestation #2 recordings re-released on compact disc in 1991 by Mercury 
    * Expression #2 sound issued during the performances by Yo-Yo Ma recorded in 1983
          o Manifestation #1 recordings released on 33 1/3 rpm sound discs in 1983 by CBS Records
          o Manifestation #2 recordings re-released on compact disc in 1992 by CBS Records 

          
Changes that occur deliberately or even inadvertently in the production process that affect the copies result, strictly speaking, in a new manifestation. A manifestation resulting from such a change may be identified as a particular \"state\" or \"issue\" of the publication.

Changes that occur to an individual copy after the production process is complete (e.g., the loss of a page, rebinding, etc.) are not considered to result in a new manifestation. That copy is simply considered to be an exemplar (or item) of the manifestation that deviates from the copy as produced.

With the entity defined as manifestation we can describe the physical characteristics of a set of items and the characteristics associated with the production and distribution of that set of items that may be important factors in enabling users to choose a manifestation appropriate to their physical needs and constraints, and to identify and acquire a copy of that manifestation.

Defining manifestation as an entity also enables us to draw relationships between specific manifestations of a work. We can use the relationships between manifestations to identify, for example, the specific publication that was used to create a microreproduction.          

""" ;
                        rdfs:isDefinedBy <http://purl.org/ontology/mo/> ;
                        rdfs:label "musical manifestation" ;
                        vs:term_status "stable" .


###  http://purl.org/ontology/mo/MusicalWork
mo:MusicalWork rdf:type owl:Class ;
               rdfs:subClassOf frbr:Work ;
               mo:level "2" ;
               rdfs:comment """
    Distinct intellectual or artistic musical creation.
    
From the FRBR final report: A work is an abstract entity; there is no single material object one can point to as the work. We recognize the work through individual realizations or expressions of the work, but the work itself exists only in the commonality of
content between and among the various expressions of the work. When we speak of Homer's Iliad as a work, our point of reference is not a particular recitation or text of the work, but the intellectual creation that lies behind all the various expressions of the work.     

For example:

work #1 J. S. Bach's The art of the fugue

    
    """ ;
               rdfs:isDefinedBy <http://purl.org/ontology/mo/> ;
               rdfs:label "musical work" ;
               vs:term_status "stable" .


###  http://purl.org/ontology/mo/Orchestration
mo:Orchestration rdf:type owl:Class ;
                 rdfs:subClassOf mo:Arrangement ;
                 mo:level "2" ;
                 rdfs:comment """
            Orchestration includes, in addition to instrumentation, the handling of groups of instruments and their balance and interaction.
    """ ;
                 rdfs:isDefinedBy <http://purl.org/ontology/mo/> ;
                 rdfs:label "orchestration" ;
                 vs:term_status "stable" .


###  http://purl.org/ontology/mo/Performance
mo:Performance rdf:type owl:Class ;
               rdfs:subClassOf event:Event ;
               mo:level "2" ;
               rdfs:comment """
        A performance event. 
        It might include as agents performers, engineers, conductors, or even listeners.
        It might include as factors a score, a MusicalWork, musical instruments. 
        It might produce a sound:-)
    """ ;
               rdfs:isDefinedBy <http://purl.org/ontology/mo/> ;
               rdfs:label "performance" ;
               vs:term_status "stable" .


###  http://purl.org/ontology/mo/Performer
mo:Performer rdf:type owl:Class ;
             owl:equivalentClass [ rdf:type owl:Restriction ;
                                   owl:onProperty mo:performed ;
                                   owl:someValuesFrom mo:Performance
                                 ] ;
             rdfs:subClassOf foaf:Agent ;
             mo:level "2" ;
             rdfs:label "performer" ;
             vs:term_status "unstable" .


###  http://purl.org/ontology/mo/PublishedLibretto
mo:PublishedLibretto rdf:type owl:Class ;
                     rdfs:subClassOf mo:MusicalManifestation ;
                     mo:level "2" ;
                     rdfs:comment "A published libretto" ;
                     rdfs:isDefinedBy <http://purl.org/ontology/mo/> ;
                     rdfs:label "published libretto" ;
                     vs:term_status "stable" .


###  http://purl.org/ontology/mo/PublishedLyrics
mo:PublishedLyrics rdf:type owl:Class ;
                   rdfs:subClassOf mo:MusicalManifestation ;
                   mo:level "2" ;
                   rdfs:comment "Published lyrics, as a book or as a text file, for example" ;
                   rdfs:isDefinedBy <http://purl.org/ontology/mo/> ;
                   rdfs:label "published lyrics" ;
                   vs:term_status "stable" .


###  http://purl.org/ontology/mo/PublishedScore
mo:PublishedScore rdf:type owl:Class ;
                  rdfs:subClassOf mo:MusicalManifestation ;
                  mo:level "2" ;
                  rdfs:comment "A published score (subclass of MusicalManifestation)" ;
                  rdfs:isDefinedBy <http://purl.org/ontology/mo/> ;
                  rdfs:label "published score" ;
                  vs:term_status "stable" .


###  http://purl.org/ontology/mo/Record
mo:Record rdf:type owl:Class ;
          rdfs:subClassOf mo:MusicalManifestation ;
          mo:level "1" ;
          rdfs:comment "A published record (manifestation which first aim is to render the product of a recording)" ;
          rdfs:isDefinedBy <http://purl.org/ontology/mo/> ;
          rdfs:label "record" ;
          vs:term_status "stable" .


###  http://purl.org/ontology/mo/Recording
mo:Recording rdf:type owl:Class ;
             rdfs:subClassOf event:Event ;
             mo:level "2" ;
             rdfs:comment """
        A recording event.
        Takes a sound as a factor to produce a signal (analog or digital).
        The location of such events (if any) is the actual location of the corresponding
        microphone or the \"recording device\".
    """ ;
             rdfs:isDefinedBy <http://purl.org/ontology/mo/> ;
             rdfs:label "recording" ;
             vs:term_status "stable" .


###  http://purl.org/ontology/mo/RecordingSession
mo:RecordingSession rdf:type owl:Class ;
                    rdfs:subClassOf event:Event ;
                    mo:level "2" ;
                    rdfs:comment "A set of performances/recordings/mastering events. This event can be decomposed in its constituent events using event:sub_event" ;
                    rdfs:isDefinedBy <http://purl.org/ontology/mo/> ;
                    rdfs:label "recording session" ;
                    vs:term_status "testing" .


###  http://purl.org/ontology/mo/Release
mo:Release rdf:type owl:Class ;
           rdfs:subClassOf mo:MusicalManifestation ;
           mo:level "1" ;
           rdfs:comment "A specific release, with barcode, box, liner notes, cover art, and a number of records" ;
           rdfs:isDefinedBy <http://purl.org/ontology/mo/> ;
           rdfs:label "release" ;
           vs:term_status "testing" .


###  http://purl.org/ontology/mo/ReleaseEvent
mo:ReleaseEvent rdf:type owl:Class ;
                rdfs:subClassOf event:Event ;
                mo:level "1" ;
                rdfs:comment "A release event, in a particular place (e.g. a country) at a particular time. Other factors of this event might include cover art, liner notes, box, etc. or a release grouping all these." ;
                rdfs:isDefinedBy <http://purl.org/ontology/mo/> ;
                rdfs:label "release event" ;
                vs:term_status "testing" .


###  http://purl.org/ontology/mo/ReleaseStatus
mo:ReleaseStatus rdf:type owl:Class ;
                 mo:level "1" ;
                 rdfs:comment "Musical manifestation release status." ;
                 rdfs:isDefinedBy <http://purl.org/ontology/mo/> ;
                 rdfs:label "release status" ;
                 vs:term_status "stable" .


###  http://purl.org/ontology/mo/ReleaseType
mo:ReleaseType rdf:type owl:Class ;
               mo:level "1" ;
               rdfs:comment """
        Release type of a particular manifestation, such as \"album\" or \"interview\"...
    """ ;
               rdfs:isDefinedBy <http://purl.org/ontology/mo/> ;
               rdfs:label "Release type" ;
               vs:term_status "stable" .


###  http://purl.org/ontology/mo/SACD
mo:SACD rdf:type owl:Class ;
        rdfs:subClassOf mo:Medium ;
        mo:level "1" ;
        rdfs:comment "Super Audio Compact Disc used as medium to record a musical manifestation." ;
        rdfs:isDefinedBy <http://purl.org/ontology/mo/> ;
        rdfs:label "SACD" ;
        vs:term_status "unstable" .


###  http://purl.org/ontology/mo/Score
mo:Score rdf:type owl:Class ;
         rdfs:subClassOf mo:MusicalExpression ;
         mo:level "2" ;
         rdfs:comment """
        Here, we are dealing with the informational object (the MusicalExpression), not the actually \"published\" score.
        This may be, for example, the product of an arrangement process.
    """ ;
         rdfs:isDefinedBy <http://purl.org/ontology/mo/> ;
         rdfs:label "score" ;
         vs:term_status "stable" .


###  http://purl.org/ontology/mo/Show
mo:Show rdf:type owl:Class ;
        rdfs:subClassOf event:Event ;
        mo:level "2" ;
        rdfs:comment """
        A show - a musical event lasting several days, in a particular venue. Examples can be
        \"The Magic Flute\" at the Opera Bastille, August 2005, or a musical in the west end...
    """ ;
        rdfs:isDefinedBy <http://purl.org/ontology/mo/> ;
        rdfs:label "Show" ;
        vs:term_status "stable" .


###  http://purl.org/ontology/mo/Signal
mo:Signal rdf:type owl:Class ;
          rdfs:subClassOf mo:MusicalExpression ;
          mo:level "1" ;
          rdfs:comment """
        A subclass of MusicalExpression, representing a signal, for example a master signal produced by a performance and a recording.
    """ ;
          rdfs:isDefinedBy <http://purl.org/ontology/mo/> ;
          rdfs:label "signal" ;
          vs:term_status "stable" .


###  http://purl.org/ontology/mo/SignalGroup
mo:SignalGroup rdf:type owl:Class ;
               rdfs:subClassOf mo:MusicalExpression ;
               mo:level "1" ;
               rdfs:comment """
        A musical expression representing a group of signals, for example a set of masters resulting from a whole recording/mastering session.
    """ ;
               rdfs:isDefinedBy <http://purl.org/ontology/mo/> ;
               rdfs:label "signal group" ;
               vs:term_status "testing" .


###  http://purl.org/ontology/mo/SoloMusicArtist
mo:SoloMusicArtist rdf:type owl:Class ;
                   rdfs:subClassOf mo:MusicArtist ,
                                   foaf:Person ;
                   mo:level "1" ;
                   rdfs:comment "Single person whose musical creative work shows sensitivity and imagination." ;
                   rdfs:isDefinedBy <http://purl.org/ontology/mo/> ;
                   rdfs:label "solo music artist" ;
                   vs:term_status "stable" .


###  http://purl.org/ontology/mo/Sound
mo:Sound rdf:type owl:Class ;
         rdfs:subClassOf event:Event ,
                         mo:MusicalExpression ;
         mo:level "2" ;
         rdfs:comment """
        A subclass of MusicalExpression, representing a sound. Realisation of a MusicalWork during a musical Performance.
    """ ;
         rdfs:isDefinedBy <http://purl.org/ontology/mo/> ;
         rdfs:label "sound" ;
         vs:term_status "stable" .


###  http://purl.org/ontology/mo/SoundEngineer
mo:SoundEngineer rdf:type owl:Class ;
                 owl:equivalentClass [ rdf:type owl:Restriction ;
                                       owl:onProperty mo:engineered ;
                                       owl:someValuesFrom mo:Performance
                                     ] ;
                 rdfs:subClassOf foaf:Agent ;
                 mo:level "2" ;
                 rdfs:label "sound engineer" ;
                 vs:term_status "unstable" .


###  http://purl.org/ontology/mo/Stream
mo:Stream rdf:type owl:Class ;
          rdfs:subClassOf mo:Medium ;
          mo:level "1" ;
          rdfs:comment "Transmission over a network  used as medium to broadcast a musical manifestation" ;
          rdfs:isDefinedBy <http://purl.org/ontology/mo/> ;
          rdfs:label "Stream" ;
          vs:term_status "unstable" .


###  http://purl.org/ontology/mo/Torrent
mo:Torrent rdf:type owl:Class ;
           rdfs:subClassOf mo:Medium ;
           mo:level "1" ;
           rdfs:comment "Something available on the Bittorrent peer-2-peer filesharing network" ;
           rdfs:isDefinedBy <http://purl.org/ontology/mo/> ;
           rdfs:label "Torrent" ;
           vs:term_status "unstable" .


###  http://purl.org/ontology/mo/Track
mo:Track rdf:type owl:Class ;
         rdfs:subClassOf mo:MusicalManifestation ;
         mo:level "1" ;
         rdfs:comment "A track on a particular record" ;
         rdfs:isDefinedBy <http://purl.org/ontology/mo/> ;
         rdfs:label "track" ;
         vs:term_status "stable" .


###  http://purl.org/ontology/mo/Transcription
mo:Transcription rdf:type owl:Class ;
                 rdfs:subClassOf event:Event ;
                 mo:level "2" ;
                 rdfs:comment "Transcription event" ;
                 rdfs:isDefinedBy <http://purl.org/ontology/mo/> ;
                 rdfs:label "transcription" ;
                 vs:term_status "testing" .


###  http://purl.org/ontology/mo/Vinyl
mo:Vinyl rdf:type owl:Class ;
         rdfs:subClassOf mo:Medium ;
         mo:level "1" ;
         rdfs:comment "Vinyl used as medium to record a musical manifestation" ;
         rdfs:isDefinedBy <http://purl.org/ontology/mo/> ;
         rdfs:label "Vinyl" ;
         vs:term_status "unstable" .


###  http://purl.org/vocab/frbr/core#Expression
frbr:Expression rdf:type owl:Class .


###  http://purl.org/vocab/frbr/core#Item
frbr:Item rdf:type owl:Class .


###  http://purl.org/vocab/frbr/core#Manifestation
frbr:Manifestation rdf:type owl:Class .


###  http://purl.org/vocab/frbr/core#Work
frbr:Work rdf:type owl:Class .


###  http://web.resource.org/cc/License
cc:License rdf:type owl:Class .


#################################################################
#    Individuals
#################################################################

###  http://apassant.net/
<http://apassant.net/> rdf:type owl:NamedIndividual .


###  http://fgiasson.com/
<http://fgiasson.com/> rdf:type owl:NamedIndividual .


###  http://foaf.me/zazi#me
<http://foaf.me/zazi#me> rdf:type owl:NamedIndividual ;
                         foaf:homepage <http://smiy.wordpress.com/> ;
                         foaf:name "Thomas Gängler" .


###  http://kurtisrandom.com/
<http://kurtisrandom.com/> rdf:type owl:NamedIndividual .


###  http://kurtisrandom.com/foaf.rdf#kurtjx
<http://kurtisrandom.com/foaf.rdf#kurtjx> rdf:type owl:NamedIndividual ;
                                          foaf:homepage <http://kurtisrandom.com/> ;
                                          foaf:name "Kurt Jacobson" .


###  http://purl.org/dc/terms/
dcterms: dcterms:publisher <http://purl.org/dc/aboutdcmi#DCMI> ;
         dcterms:modified "2012-06-14"^^xsd:date ;
         dcterms:title "DCMI Metadata Terms - other"@en .


###  http://purl.org/dc/terms/Agent
dcterms:Agent rdf:type dcterms:AgentClass ;
              dcterms:issued "2008-01-14"^^xsd:date .


###  http://purl.org/dc/terms/AgentClass
dcterms:AgentClass dcterms:issued "2008-01-14"^^xsd:date ;
                   dcterms:modified "2012-06-14"^^xsd:date .


###  http://purl.org/dc/terms/BibliographicResource
dcterms:BibliographicResource dcterms:issued "2008-01-14"^^xsd:date .


###  http://purl.org/dc/terms/Box
dcterms:Box dcterms:issued "2000-07-11"^^xsd:date ;
            dcterms:modified "2008-01-14"^^xsd:date .


###  http://purl.org/dc/terms/DCMIType
dcterms:DCMIType rdf:type <http://purl.org/dc/dcam/VocabularyEncodingScheme> ;
                 dcterms:issued "2000-07-11"^^xsd:date ;
                 dcterms:modified "2012-06-14"^^xsd:date ;
                 dcterms:hasVersion <http://dublincore.org/usage/terms/history/#DCMIType-005> ;
                 rdfs:comment "The set of classes specified by the DCMI Type Vocabulary, used to categorize the nature or genre of the resource."@en ;
                 rdfs:isDefinedBy dcterms: ;
                 rdfs:label "DCMI Type Vocabulary"@en ;
                 rdfs:seeAlso <http://purl.org/dc/dcmitype/> .


###  http://purl.org/dc/terms/DDC
dcterms:DDC rdf:type <http://purl.org/dc/dcam/VocabularyEncodingScheme> ;
            dcterms:issued "2000-07-11"^^xsd:date ;
            dcterms:modified "2008-01-14"^^xsd:date ;
            dcterms:hasVersion <http://dublincore.org/usage/terms/history/#DDC-003> ;
            rdfs:comment "The set of conceptual resources specified by the Dewey Decimal Classification."@en ;
            rdfs:isDefinedBy dcterms: ;
            rdfs:label "DDC"@en ;
            rdfs:seeAlso <http://www.oclc.org/dewey/> .


###  http://purl.org/dc/terms/FileFormat
dcterms:FileFormat dcterms:issued "2008-01-14"^^xsd:date .


###  http://purl.org/dc/terms/Frequency
dcterms:Frequency dcterms:issued "2008-01-14"^^xsd:date .


###  http://purl.org/dc/terms/IMT
dcterms:IMT rdf:type <http://purl.org/dc/dcam/VocabularyEncodingScheme> ;
            dcterms:issued "2000-07-11"^^xsd:date ;
            dcterms:modified "2008-01-14"^^xsd:date ;
            dcterms:hasVersion <http://dublincore.org/usage/terms/history/#IMT-004> ;
            rdfs:comment "The set of media types specified by the Internet Assigned Numbers Authority."@en ;
            rdfs:isDefinedBy dcterms: ;
            rdfs:label "IMT"@en ;
            rdfs:seeAlso <http://www.iana.org/assignments/media-types/> .


###  http://purl.org/dc/terms/ISO3166
dcterms:ISO3166 dcterms:issued "2000-07-11"^^xsd:date ;
                dcterms:modified "2008-01-14"^^xsd:date .


###  http://purl.org/dc/terms/ISO639-2
dcterms:ISO639-2 dcterms:issued "2000-07-11"^^xsd:date ;
                 dcterms:modified "2008-01-14"^^xsd:date .


###  http://purl.org/dc/terms/ISO639-3
dcterms:ISO639-3 dcterms:issued "2008-01-14"^^xsd:date .


###  http://purl.org/dc/terms/Jurisdiction
dcterms:Jurisdiction dcterms:issued "2008-01-14"^^xsd:date .


###  http://purl.org/dc/terms/LCC
dcterms:LCC rdf:type <http://purl.org/dc/dcam/VocabularyEncodingScheme> ;
            dcterms:issued "2000-07-11"^^xsd:date ;
            dcterms:modified "2008-01-14"^^xsd:date ;
            dcterms:hasVersion <http://dublincore.org/usage/terms/history/#LCC-003> ;
            rdfs:comment "The set of conceptual resources specified by the Library of Congress Classification."@en ;
            rdfs:isDefinedBy dcterms: ;
            rdfs:label "LCC"@en ;
            rdfs:seeAlso <http://lcweb.loc.gov/catdir/cpso/lcco/lcco.html> .


###  http://purl.org/dc/terms/LCSH
dcterms:LCSH rdf:type <http://purl.org/dc/dcam/VocabularyEncodingScheme> ;
             dcterms:issued "2000-07-11"^^xsd:date ;
             dcterms:modified "2008-01-14"^^xsd:date ;
             dcterms:hasVersion <http://dublincore.org/usage/terms/history/#LCSH-003> ;
             rdfs:comment "The set of labeled concepts specified by the Library of Congress Subject Headings."@en ;
             rdfs:isDefinedBy dcterms: ;
             rdfs:label "LCSH"@en .


###  http://purl.org/dc/terms/LicenseDocument
dcterms:LicenseDocument dcterms:issued "2008-01-14"^^xsd:date .


###  http://purl.org/dc/terms/LinguisticSystem
dcterms:LinguisticSystem dcterms:issued "2008-01-14"^^xsd:date .


###  http://purl.org/dc/terms/Location
dcterms:Location dcterms:issued "2008-01-14"^^xsd:date .


###  http://purl.org/dc/terms/LocationPeriodOrJurisdiction
dcterms:LocationPeriodOrJurisdiction dcterms:issued "2008-01-14"^^xsd:date .


###  http://purl.org/dc/terms/MESH
dcterms:MESH rdf:type <http://purl.org/dc/dcam/VocabularyEncodingScheme> ;
             dcterms:issued "2000-07-11"^^xsd:date ;
             dcterms:modified "2008-01-14"^^xsd:date ;
             dcterms:hasVersion <http://dublincore.org/usage/terms/history/#MESH-003> ;
             rdfs:comment "The set of labeled concepts specified by the Medical Subject Headings."@en ;
             rdfs:isDefinedBy dcterms: ;
             rdfs:label "MeSH"@en ;
             rdfs:seeAlso <http://www.nlm.nih.gov/mesh/meshhome.html> .


###  http://purl.org/dc/terms/MediaType
dcterms:MediaType dcterms:issued "2008-01-14"^^xsd:date .


###  http://purl.org/dc/terms/MediaTypeOrExtent
dcterms:MediaTypeOrExtent dcterms:issued "2008-01-14"^^xsd:date .


###  http://purl.org/dc/terms/MethodOfAccrual
dcterms:MethodOfAccrual dcterms:issued "2008-01-14"^^xsd:date .


###  http://purl.org/dc/terms/MethodOfInstruction
dcterms:MethodOfInstruction dcterms:issued "2008-01-14"^^xsd:date .


###  http://purl.org/dc/terms/NLM
dcterms:NLM rdf:type <http://purl.org/dc/dcam/VocabularyEncodingScheme> ;
            dcterms:issued "2005-06-13"^^xsd:date ;
            dcterms:modified "2008-01-14"^^xsd:date ;
            dcterms:hasVersion <http://dublincore.org/usage/terms/history/#NLM-002> ;
            rdfs:comment "The set of conceptual resources specified by the National Library of Medicine Classification."@en ;
            rdfs:isDefinedBy dcterms: ;
            rdfs:label "NLM"@en ;
            rdfs:seeAlso <http://wwwcf.nlm.nih.gov/class/> .


###  http://purl.org/dc/terms/Period
dcterms:Period dcterms:issued "2000-07-11"^^xsd:date ;
               dcterms:modified "2008-01-14"^^xsd:date .


###  http://purl.org/dc/terms/PeriodOfTime
dcterms:PeriodOfTime dcterms:issued "2008-01-14"^^xsd:date .


###  http://purl.org/dc/terms/PhysicalMedium
dcterms:PhysicalMedium dcterms:issued "2008-01-14"^^xsd:date .


###  http://purl.org/dc/terms/PhysicalResource
dcterms:PhysicalResource dcterms:issued "2008-01-14"^^xsd:date .


###  http://purl.org/dc/terms/Point
dcterms:Point dcterms:issued "2000-07-11"^^xsd:date ;
              dcterms:modified "2008-01-14"^^xsd:date .


###  http://purl.org/dc/terms/Policy
dcterms:Policy dcterms:issued "2008-01-14"^^xsd:date .


###  http://purl.org/dc/terms/ProvenanceStatement
dcterms:ProvenanceStatement dcterms:issued "2008-01-14"^^xsd:date .


###  http://purl.org/dc/terms/RFC1766
dcterms:RFC1766 dcterms:issued "2000-07-11"^^xsd:date ;
                dcterms:modified "2008-01-14"^^xsd:date .


###  http://purl.org/dc/terms/RFC3066
dcterms:RFC3066 dcterms:issued "2002-07-13"^^xsd:date ;
                dcterms:modified "2008-01-14"^^xsd:date .


###  http://purl.org/dc/terms/RFC4646
dcterms:RFC4646 dcterms:issued "2008-01-14"^^xsd:date .


###  http://purl.org/dc/terms/RFC5646
dcterms:RFC5646 dcterms:issued "2010-10-11"^^xsd:date .


###  http://purl.org/dc/terms/RightsStatement
dcterms:RightsStatement dcterms:issued "2008-01-14"^^xsd:date .


###  http://purl.org/dc/terms/SizeOrDuration
dcterms:SizeOrDuration dcterms:issued "2008-01-14"^^xsd:date .


###  http://purl.org/dc/terms/Standard
dcterms:Standard dcterms:issued "2008-01-14"^^xsd:date .


###  http://purl.org/dc/terms/TGN
dcterms:TGN rdf:type <http://purl.org/dc/dcam/VocabularyEncodingScheme> ;
            dcterms:issued "2000-07-11"^^xsd:date ;
            dcterms:modified "2008-01-14"^^xsd:date ;
            dcterms:hasVersion <http://dublincore.org/usage/terms/history/#TGN-003> ;
            rdfs:comment "The set of places specified by the Getty Thesaurus of Geographic Names."@en ;
            rdfs:isDefinedBy dcterms: ;
            rdfs:label "TGN"@en ;
            rdfs:seeAlso <http://www.getty.edu/research/tools/vocabulary/tgn/index.html> .


###  http://purl.org/dc/terms/UDC
dcterms:UDC rdf:type <http://purl.org/dc/dcam/VocabularyEncodingScheme> ;
            dcterms:issued "2000-07-11"^^xsd:date ;
            dcterms:modified "2008-01-14"^^xsd:date ;
            dcterms:hasVersion <http://dublincore.org/usage/terms/history/#UDC-003> ;
            rdfs:comment "The set of conceptual resources specified by the Universal Decimal Classification."@en ;
            rdfs:isDefinedBy dcterms: ;
            rdfs:label "UDC"@en ;
            rdfs:seeAlso <http://www.udcc.org/> .


###  http://purl.org/dc/terms/URI
dcterms:URI dcterms:issued "2000-07-11"^^xsd:date ;
            dcterms:modified "2008-01-14"^^xsd:date .


###  http://purl.org/dc/terms/W3CDTF
dcterms:W3CDTF dcterms:issued "2000-07-11"^^xsd:date ;
               dcterms:modified "2008-01-14"^^xsd:date .


###  http://purl.org/dc/terms/abstract
dcterms:abstract dcterms:issued "2000-07-11"^^xsd:date ;
                 dcterms:modified "2008-01-14"^^xsd:date .


###  http://purl.org/dc/terms/accessRights
dcterms:accessRights dcterms:issued "2003-02-15"^^xsd:date ;
                     dcterms:modified "2008-01-14"^^xsd:date .


###  http://purl.org/dc/terms/accrualMethod
dcterms:accrualMethod dcterms:issued "2005-06-13"^^xsd:date ;
                      dcterms:modified "2010-10-11"^^xsd:date .


###  http://purl.org/dc/terms/accrualPeriodicity
dcterms:accrualPeriodicity dcterms:issued "2005-06-13"^^xsd:date ;
                           dcterms:modified "2010-10-11"^^xsd:date .


###  http://purl.org/dc/terms/accrualPolicy
dcterms:accrualPolicy dcterms:issued "2005-06-13"^^xsd:date ;
                      dcterms:modified "2010-10-11"^^xsd:date .


###  http://purl.org/dc/terms/alternative
dcterms:alternative dcterms:issued "2000-07-11"^^xsd:date ;
                    dcterms:modified "2010-10-11"^^xsd:date .


###  http://purl.org/dc/terms/audience
dcterms:audience dcterms:issued "2001-05-21"^^xsd:date ;
                 dcterms:modified "2008-01-14"^^xsd:date .


###  http://purl.org/dc/terms/available
dcterms:available dcterms:issued "2000-07-11"^^xsd:date ;
                  dcterms:modified "2008-01-14"^^xsd:date .


###  http://purl.org/dc/terms/bibliographicCitation
dcterms:bibliographicCitation dcterms:issued "2003-02-15"^^xsd:date ;
                              dcterms:modified "2008-01-14"^^xsd:date .


###  http://purl.org/dc/terms/conformsTo
dcterms:conformsTo dcterms:issued "2001-05-21"^^xsd:date ;
                   dcterms:modified "2008-01-14"^^xsd:date .


###  http://purl.org/dc/terms/contributor
dcterms:contributor dcterms:issued "2008-01-14"^^xsd:date ;
                    dcterms:modified "2010-10-11"^^xsd:date .


###  http://purl.org/dc/terms/coverage
dcterms:coverage dcterms:issued "2008-01-14"^^xsd:date ;
                 dcterms:modified "2008-01-14"^^xsd:date .


###  http://purl.org/dc/terms/created
dcterms:created dcterms:issued "2000-07-11"^^xsd:date ;
                dcterms:modified "2008-01-14"^^xsd:date .


###  http://purl.org/dc/terms/creator
dcterms:creator dcterms:issued "2008-01-14"^^xsd:date ;
                dcterms:modified "2010-10-11"^^xsd:date .


###  http://purl.org/dc/terms/date
dcterms:date dcterms:issued "2008-01-14"^^xsd:date ;
             dcterms:modified "2008-01-14"^^xsd:date .


###  http://purl.org/dc/terms/dateAccepted
dcterms:dateAccepted dcterms:issued "2002-07-13"^^xsd:date ;
                     dcterms:modified "2008-01-14"^^xsd:date .


###  http://purl.org/dc/terms/dateCopyrighted
dcterms:dateCopyrighted dcterms:issued "2002-07-13"^^xsd:date ;
                        dcterms:modified "2008-01-14"^^xsd:date .


###  http://purl.org/dc/terms/dateSubmitted
dcterms:dateSubmitted dcterms:issued "2002-07-13"^^xsd:date ;
                      dcterms:modified "2008-01-14"^^xsd:date .


###  http://purl.org/dc/terms/description
dcterms:description dcterms:issued "2008-01-14"^^xsd:date ;
                    dcterms:modified "2008-01-14"^^xsd:date .


###  http://purl.org/dc/terms/educationLevel
dcterms:educationLevel dcterms:issued "2002-07-13"^^xsd:date ;
                       dcterms:modified "2008-01-14"^^xsd:date .


###  http://purl.org/dc/terms/extent
dcterms:extent dcterms:issued "2000-07-11"^^xsd:date ;
               dcterms:modified "2008-01-14"^^xsd:date .


###  http://purl.org/dc/terms/format
dcterms:format dcterms:issued "2008-01-14"^^xsd:date ;
               dcterms:modified "2008-01-14"^^xsd:date .


###  http://purl.org/dc/terms/hasFormat
dcterms:hasFormat dcterms:issued "2000-07-11"^^xsd:date ;
                  dcterms:modified "2008-01-14"^^xsd:date .


###  http://purl.org/dc/terms/hasPart
dcterms:hasPart dcterms:issued "2000-07-11"^^xsd:date ;
                dcterms:modified "2008-01-14"^^xsd:date .


###  http://purl.org/dc/terms/hasVersion
dcterms:hasVersion dcterms:issued "2000-07-11"^^xsd:date ;
                   dcterms:modified "2008-01-14"^^xsd:date .


###  http://purl.org/dc/terms/identifier
dcterms:identifier dcterms:issued "2008-01-14"^^xsd:date ;
                   dcterms:modified "2008-01-14"^^xsd:date .


###  http://purl.org/dc/terms/instructionalMethod
dcterms:instructionalMethod dcterms:issued "2005-06-13"^^xsd:date ;
                            dcterms:modified "2008-01-14"^^xsd:date .


###  http://purl.org/dc/terms/isFormatOf
dcterms:isFormatOf dcterms:issued "2000-07-11"^^xsd:date ;
                   dcterms:modified "2008-01-14"^^xsd:date .


###  http://purl.org/dc/terms/isPartOf
dcterms:isPartOf dcterms:issued "2000-07-11"^^xsd:date ;
                 dcterms:modified "2008-01-14"^^xsd:date .


###  http://purl.org/dc/terms/isReferencedBy
dcterms:isReferencedBy dcterms:issued "2000-07-11"^^xsd:date ;
                       dcterms:modified "2008-01-14"^^xsd:date .


###  http://purl.org/dc/terms/isReplacedBy
dcterms:isReplacedBy dcterms:issued "2000-07-11"^^xsd:date ;
                     dcterms:modified "2008-01-14"^^xsd:date .


###  http://purl.org/dc/terms/isRequiredBy
dcterms:isRequiredBy dcterms:issued "2000-07-11"^^xsd:date ;
                     dcterms:modified "2008-01-14"^^xsd:date .


###  http://purl.org/dc/terms/isVersionOf
dcterms:isVersionOf dcterms:issued "2000-07-11"^^xsd:date ;
                    dcterms:modified "2008-01-14"^^xsd:date .


###  http://purl.org/dc/terms/issued
dcterms:issued dcterms:issued "2000-07-11"^^xsd:date ;
               dcterms:modified "2008-01-14"^^xsd:date .


###  http://purl.org/dc/terms/language
dcterms:language dcterms:issued "2008-01-14"^^xsd:date ;
                 dcterms:modified "2008-01-14"^^xsd:date .


###  http://purl.org/dc/terms/license
dcterms:license dcterms:issued "2004-06-14"^^xsd:date ;
                dcterms:modified "2008-01-14"^^xsd:date .


###  http://purl.org/dc/terms/mediator
dcterms:mediator dcterms:issued "2001-05-21"^^xsd:date ;
                 dcterms:modified "2008-01-14"^^xsd:date .


###  http://purl.org/dc/terms/medium
dcterms:medium dcterms:issued "2000-07-11"^^xsd:date ;
               dcterms:modified "2008-01-14"^^xsd:date .


###  http://purl.org/dc/terms/modified
dcterms:modified dcterms:issued "2000-07-11"^^xsd:date ;
                 dcterms:modified "2008-01-14"^^xsd:date .


###  http://purl.org/dc/terms/provenance
dcterms:provenance dcterms:issued "2004-09-20"^^xsd:date ;
                   dcterms:modified "2008-01-14"^^xsd:date .


###  http://purl.org/dc/terms/publisher
dcterms:publisher dcterms:issued "2008-01-14"^^xsd:date ;
                  dcterms:modified "2010-10-11"^^xsd:date .


###  http://purl.org/dc/terms/references
dcterms:references dcterms:issued "2000-07-11"^^xsd:date ;
                   dcterms:modified "2008-01-14"^^xsd:date .


###  http://purl.org/dc/terms/relation
dcterms:relation dcterms:issued "2008-01-14"^^xsd:date ;
                 dcterms:modified "2008-01-14"^^xsd:date .


###  http://purl.org/dc/terms/replaces
dcterms:replaces dcterms:issued "2000-07-11"^^xsd:date ;
                 dcterms:modified "2008-01-14"^^xsd:date .


###  http://purl.org/dc/terms/requires
dcterms:requires dcterms:issued "2000-07-11"^^xsd:date ;
                 dcterms:modified "2008-01-14"^^xsd:date .


###  http://purl.org/dc/terms/rights
dcterms:rights dcterms:issued "2008-01-14"^^xsd:date ;
               dcterms:modified "2008-01-14"^^xsd:date .


###  http://purl.org/dc/terms/rightsHolder
dcterms:rightsHolder dcterms:issued "2004-06-14"^^xsd:date ;
                     dcterms:modified "2008-01-14"^^xsd:date .


###  http://purl.org/dc/terms/source
dcterms:source dcterms:issued "2008-01-14"^^xsd:date ;
               dcterms:modified "2008-01-14"^^xsd:date .


###  http://purl.org/dc/terms/spatial
dcterms:spatial dcterms:issued "2000-07-11"^^xsd:date ;
                dcterms:modified "2008-01-14"^^xsd:date .


###  http://purl.org/dc/terms/subject
dcterms:subject dcterms:issued "2008-01-14"^^xsd:date ;
                dcterms:modified "2012-06-14"^^xsd:date .


###  http://purl.org/dc/terms/tableOfContents
dcterms:tableOfContents dcterms:issued "2000-07-11"^^xsd:date ;
                        dcterms:modified "2008-01-14"^^xsd:date .


###  http://purl.org/dc/terms/temporal
dcterms:temporal dcterms:issued "2000-07-11"^^xsd:date ;
                 dcterms:modified "2008-01-14"^^xsd:date .


###  http://purl.org/dc/terms/title
dcterms:title dcterms:issued "2008-01-14"^^xsd:date ;
              dcterms:modified "2010-10-11"^^xsd:date .


###  http://purl.org/dc/terms/type
dcterms:type dcterms:issued "2008-01-14"^^xsd:date ;
             dcterms:modified "2008-01-14"^^xsd:date .


###  http://purl.org/dc/terms/valid
dcterms:valid dcterms:issued "2000-07-11"^^xsd:date ;
              dcterms:modified "2008-01-14"^^xsd:date .


###  http://purl.org/ontology/mo/
<http://purl.org/ontology/mo/> rdf:type owl:NamedIndividual ;
                               foaf:maker <http://foaf.me/zazi#me> ,
                                          <http://kurtisrandom.com/foaf.rdf#kurtjx> ,
                                          <http://raimond.me.uk/foaf.rdf#moustaki> ,
                                          <http://www.talkdigger.com/foaf/fgiasson> ,
                                          _:genid160 ,
                                          _:genid161 ,
                                          [ ]_:genid160 foaf:homepage <http://apassant.net/>_:genid161 foaf:homepage <http://simon-reinhardt.de/> .


###  http://purl.org/ontology/mo/album
mo:album rdf:type owl:NamedIndividual ,
                  mo:ReleaseType ;
         dc:description """
        One or more track issued together.
            This is a type of MusicalManifestation defined by the musical industry.
    """ ;
         dc:title "album" ;
         mo:level "1" ;
         rdfs:isDefinedBy <http://purl.org/ontology/mo/> .


###  http://purl.org/ontology/mo/audiobook
mo:audiobook rdf:type owl:NamedIndividual ,
                      mo:ReleaseType ;
             dc:description """
        Book read by a narrator without music.
        This is a type of MusicalManifestation defined by the musical industry.
    """ ;
             dc:title "audio book" ;
             mo:level "1" ;
             rdfs:isDefinedBy <http://purl.org/ontology/mo/> .


###  http://purl.org/ontology/mo/bootleg
mo:bootleg rdf:type owl:NamedIndividual ,
                    mo:ReleaseStatus ;
           dc:description "An unofficial/underground musical work or the expression of a musical work that was not sanctioned by the artist and/or the corporate body. " ;
           dc:title "bootleg" ;
           mo:level "1" ;
           rdfs:isDefinedBy <http://purl.org/ontology/mo/> .


###  http://purl.org/ontology/mo/compilation
mo:compilation rdf:type owl:NamedIndividual ,
                        mo:ReleaseType ;
               dc:description """
        Collection of previously released manifestations of a musical expression by one or more artists.
        This is a type of MusicalManifestation defined by the musical industry.
    """ ;
               dc:title "compilation" ;
               mo:level "1" ;
               rdfs:isDefinedBy <http://purl.org/ontology/mo/> .


###  http://purl.org/ontology/mo/ep
mo:ep rdf:type owl:NamedIndividual ,
               mo:ReleaseType ;
      dc:description """
            An EP
    """ ;
      dc:title "ep" ;
      mo:level "1" ;
      rdfs:isDefinedBy <http://purl.org/ontology/mo/> .


###  http://purl.org/ontology/mo/interview
mo:interview rdf:type owl:NamedIndividual ,
                      mo:ReleaseType ;
             dc:description """
        Recording of the questioning of a person.
        This is a type of MusicalManifestation defined by the musical industry.
    """ ;
             dc:title "interview" ;
             mo:level "1" ;
             rdfs:isDefinedBy <http://purl.org/ontology/mo/> .


###  http://purl.org/ontology/mo/live
mo:live rdf:type owl:NamedIndividual ,
                 mo:ReleaseType ;
        dc:description """
        A musical manifestation that was recorded live.
        This is a type of MusicalManifestation defined by the musical industry.""" ;
        dc:title "live" ;
        mo:level "1" ;
        rdfs:isDefinedBy <http://purl.org/ontology/mo/> .


###  http://purl.org/ontology/mo/official
mo:official rdf:type owl:NamedIndividual ,
                     mo:ReleaseStatus ;
            dc:description "Any musical work or the expression of a musical work officially sanctioned by the artist and/or their corporate body." ;
            dc:title "official" ;
            mo:level "1" ;
            rdfs:isDefinedBy <http://purl.org/ontology/mo/> .


###  http://purl.org/ontology/mo/promotion
mo:promotion rdf:type owl:NamedIndividual ,
                      mo:ReleaseStatus ;
             dc:description "A giveaway musical work or the expression of a musical work intended to promote an upcoming official musical work or the expression of a musical work." ;
             dc:title "promotion" ;
             mo:level "1" ;
             rdfs:isDefinedBy <http://purl.org/ontology/mo/> .


###  http://purl.org/ontology/mo/remix
mo:remix rdf:type owl:NamedIndividual ,
                  mo:ReleaseType ;
         dc:description """
        Musical manifestation that primarily contains remixed material. 
        This is a type of MusicalManifestation defined by the musical industry.
    """ ;
         dc:title "remix" ;
         mo:level "1" ;
         rdfs:isDefinedBy <http://purl.org/ontology/mo/> .


###  http://purl.org/ontology/mo/single
mo:single rdf:type owl:NamedIndividual ,
                   mo:ReleaseType ;
          dc:description "A single or record single is a type of release, typically a recording of two tracks. In most cases, the single is a song that is released separately from an album, but it can still appear on an album." ;
          dc:title "single" ;
          mo:level "1" ;
          rdfs:isDefinedBy <http://purl.org/ontology/mo/> .


###  http://purl.org/ontology/mo/soundtrack
mo:soundtrack rdf:type owl:NamedIndividual ,
                       mo:ReleaseType ;
              dc:description """
        Sound recording on a narrow strip of a motion picture film.
        This is a type of MusicalManifestation defined by the musical industry.
    """ ;
              dc:title "soundtrack" ;
              mo:level "1" ;
              rdfs:isDefinedBy <http://purl.org/ontology/mo/> .


###  http://purl.org/ontology/mo/spokenword
mo:spokenword rdf:type owl:NamedIndividual ,
                       mo:ReleaseType ;
              dc:description """
        Spoken word is a form of music or artistic performance in which lyrics, poetry, or stories are spoken rather than sung. 
        Spoken-word is often done with a musical background, but emphasis is kept on the speaker.
        This is a type of MusicalManifestation defined by the musical industry.
    """ ;
              dc:title "spoken word" ;
              mo:level "1" ;
              rdfs:isDefinedBy <http://purl.org/ontology/mo/> .


###  http://raimond.me.uk/
<http://raimond.me.uk/> rdf:type owl:NamedIndividual .


###  http://raimond.me.uk/foaf.rdf#moustaki
<http://raimond.me.uk/foaf.rdf#moustaki> rdf:type owl:NamedIndividual ;
                                         foaf:homepage <http://raimond.me.uk/> ;
                                         foaf:name "Yves Raimond" .


###  http://simon-reinhardt.de/
<http://simon-reinhardt.de/> rdf:type owl:NamedIndividual .


###  http://smiy.wordpress.com/
<http://smiy.wordpress.com/> rdf:type owl:NamedIndividual .


###  http://www.talkdigger.com/foaf/fgiasson
<http://www.talkdigger.com/foaf/fgiasson> rdf:type owl:NamedIndividual ;
                                          foaf:homepage <http://fgiasson.com/> ;
                                          foaf:name "Frédérick Giasson" .


[ foaf:name "Alexandre Passant"
] .

[ foaf:name "Simon Reinhardt"
 ] .

[ foaf:name "George Fazekas"
 ] .

#################################################################
#    Annotations
#################################################################

dcterms:Agent rdfs:label "Agent"@en ;
               rdfs:isDefinedBy dcterms: ;
               rdfs:comment "A resource that acts or has the power to act."@en ;
               dcterms:description "Examples of Agent include person, organization, and software agent."@en ;
               dcterms:hasVersion <http://dublincore.org/usage/terms/history/#Agent-001> .


dcterms:AgentClass rdfs:isDefinedBy dcterms: ;
                   rdfs:label "Agent Class"@en ;
                   rdfs:comment "A group of agents."@en ;
                   dcterms:description "Examples of Agent Class include groups seen as classes, such as students, women, charities, lecturers."@en ;
                   dcterms:hasVersion <http://dublincore.org/usage/terms/history/#AgentClass-003> .


dcterms:BibliographicResource rdfs:isDefinedBy dcterms: ;
                              dcterms:hasVersion <http://dublincore.org/usage/terms/history/#BibliographicResource-001> ;
                              rdfs:comment "A book, article, or other documentary resource."@en ;
                              rdfs:label "Bibliographic Resource"@en .


dcterms:Box rdfs:comment "The set of regions in space defined by their geographic coordinates according to the DCMI Box Encoding Scheme."@en ;
            rdfs:isDefinedBy dcterms: ;
            rdfs:seeAlso <http://dublincore.org/documents/dcmi-box/> ;
            rdfs:label "DCMI Box"@en ;
            dcterms:hasVersion <http://dublincore.org/usage/terms/history/#Box-003> .


dcterms:FileFormat dcterms:description "Examples include the formats defined by the list of Internet Media Types."@en ;
                   dcterms:hasVersion <http://dublincore.org/usage/terms/history/#FileFormat-001> ;
                   rdfs:label "File Format"@en ;
                   rdfs:comment "A digital resource format."@en ;
                   rdfs:isDefinedBy dcterms: .


dcterms:Frequency rdfs:label "Frequency"@en ;
                  dcterms:hasVersion <http://dublincore.org/usage/terms/history/#Frequency-001> ;
                  rdfs:isDefinedBy dcterms: ;
                  rdfs:comment "A rate at which something recurs."@en .


dcterms:ISO3166 rdfs:comment "The set of codes listed in ISO 3166-1 for the representation of names of countries."@en ;
                rdfs:isDefinedBy dcterms: ;
                dcterms:hasVersion <http://dublincore.org/usage/terms/history/#ISO3166-004> ;
                rdfs:label "ISO 3166"@en ;
                rdfs:seeAlso <http://www.iso.org/iso/en/prods-services/iso3166ma/02iso-3166-code-lists/list-en1.html> .


dcterms:ISO639-2 rdfs:seeAlso <http://lcweb.loc.gov/standards/iso639-2/langhome.html> ;
                 rdfs:comment "The three-letter alphabetic codes listed in ISO639-2 for the representation of names of languages."@en ;
                 rdfs:isDefinedBy dcterms: ;
                 rdfs:label "ISO 639-2"@en ;
                 dcterms:hasVersion <http://dublincore.org/usage/terms/history/#ISO639-2-003> .


dcterms:ISO639-3 rdfs:label "ISO 639-3"@en ;
                 rdfs:comment "The set of three-letter codes listed in ISO 639-3 for the representation of names of languages."@en ;
                 dcterms:hasVersion <http://dublincore.org/usage/terms/history/#ISO639-3-001> ;
                 rdfs:isDefinedBy dcterms: ;
                 rdfs:seeAlso <http://www.sil.org/iso639-3/> .


dcterms:Jurisdiction dcterms:hasVersion <http://dublincore.org/usage/terms/history/#Jurisdiction-001> ;
                     rdfs:label "Jurisdiction"@en ;
                     rdfs:comment "The extent or range of judicial, law enforcement, or other authority."@en ;
                     rdfs:isDefinedBy dcterms: .


dcterms:LicenseDocument rdfs:isDefinedBy dcterms: ;
                        rdfs:label "License Document"@en ;
                        rdfs:comment "A legal document giving official permission to do something with a Resource."@en ;
                        dcterms:hasVersion <http://dublincore.org/usage/terms/history/#LicenseDocument-001> .


dcterms:LinguisticSystem dcterms:hasVersion <http://dublincore.org/usage/terms/history/#LinguisticSystem-001> ;
                         dcterms:description "Examples include written, spoken, sign, and computer languages."@en ;
                         rdfs:isDefinedBy dcterms: ;
                         rdfs:comment "A system of signs, symbols, sounds, gestures, or rules used in communication."@en ;
                         rdfs:label "Linguistic System"@en .


dcterms:Location dcterms:hasVersion <http://dublincore.org/usage/terms/history/#Location-001> ;
                 rdfs:label "Location"@en ;
                 rdfs:isDefinedBy dcterms: ;
                 rdfs:comment "A spatial region or named place."@en .


dcterms:LocationPeriodOrJurisdiction rdfs:label "Location, Period, or Jurisdiction"@en ;
                                     rdfs:comment "A location, period of time, or jurisdiction."@en ;
                                     rdfs:isDefinedBy dcterms: ;
                                     dcterms:hasVersion <http://dublincore.org/usage/terms/history/#LocationPeriodOrJurisdiction-001> .


dcterms:MediaType rdfs:comment "A file format or physical medium."@en ;
                  rdfs:isDefinedBy dcterms: ;
                  rdfs:label "Media Type"@en ;
                  dcterms:hasVersion <http://dublincore.org/usage/terms/history/#MediaType-001> .


dcterms:MediaTypeOrExtent rdfs:isDefinedBy dcterms: ;
                          rdfs:comment "A media type or extent."@en ;
                          rdfs:label "Media Type or Extent"@en ;
                          dcterms:hasVersion <http://dublincore.org/usage/terms/history/#MediaTypeOrExtent-001> .


dcterms:MethodOfAccrual rdfs:comment "A method by which resources are added to a collection."@en ;
                        rdfs:isDefinedBy dcterms: ;
                        dcterms:hasVersion <http://dublincore.org/usage/terms/history/#MethodOfAccrual-001> ;
                        rdfs:label "Method of Accrual"@en .


dcterms:MethodOfInstruction rdfs:label "Method of Instruction"@en ;
                            rdfs:comment "A process that is used to engender knowledge, attitudes, and skills."@en ;
                            dcterms:hasVersion <http://dublincore.org/usage/terms/history/#MethodOfInstruction-001> ;
                            rdfs:isDefinedBy dcterms: .


dcterms:Period rdfs:seeAlso <http://dublincore.org/documents/dcmi-period/> ;
               rdfs:comment "The set of time intervals defined by their limits according to the DCMI Period Encoding Scheme."@en ;
               rdfs:label "DCMI Period"@en ;
               rdfs:isDefinedBy dcterms: ;
               dcterms:hasVersion <http://dublincore.org/usage/terms/history/#Period-003> .


dcterms:PeriodOfTime rdfs:comment "An interval of time that is named or defined by its start and end dates."@en ;
                     dcterms:hasVersion <http://dublincore.org/usage/terms/history/#PeriodOfTime-001> ;
                     rdfs:isDefinedBy dcterms: ;
                     rdfs:label "Period of Time"@en .


dcterms:PhysicalMedium dcterms:hasVersion <http://dublincore.org/usage/terms/history/#PhysicalMedium-001> ;
                       dcterms:description "Examples include paper, canvas, or DVD."@en ;
                       rdfs:isDefinedBy dcterms: ;
                       rdfs:label "Physical Medium"@en ;
                       rdfs:comment "A physical material or carrier."@en .


dcterms:PhysicalResource rdfs:isDefinedBy dcterms: ;
                         rdfs:comment "A material thing."@en ;
                         dcterms:hasVersion <http://dublincore.org/usage/terms/history/#PhysicalResource-001> ;
                         rdfs:label "Physical Resource"@en .


dcterms:Point rdfs:comment "The set of points in space defined by their geographic coordinates according to the DCMI Point Encoding Scheme."@en ;
              rdfs:label "DCMI Point"@en ;
              dcterms:hasVersion <http://dublincore.org/usage/terms/history/#Point-003> ;
              rdfs:seeAlso <http://dublincore.org/documents/dcmi-point/> ;
              rdfs:isDefinedBy dcterms: .


dcterms:Policy rdfs:label "Policy"@en ;
               rdfs:isDefinedBy dcterms: ;
               rdfs:comment "A plan or course of action by an authority, intended to influence and determine decisions, actions, and other matters."@en ;
               dcterms:hasVersion <http://dublincore.org/usage/terms/history/#Policy-001> .


dcterms:ProvenanceStatement rdfs:label "Provenance Statement"@en ;
                            rdfs:isDefinedBy dcterms: ;
                            rdfs:comment "A statement of any changes in ownership and custody of a resource since its creation that are significant for its authenticity, integrity, and interpretation."@en ;
                            dcterms:hasVersion <http://dublincore.org/usage/terms/history/#ProvenanceStatement-001> .


dcterms:RFC1766 rdfs:isDefinedBy dcterms: ;
                dcterms:hasVersion <http://dublincore.org/usage/terms/history/#RFC1766-003> ;
                rdfs:comment "The set of tags, constructed according to RFC 1766, for the identification of languages."@en ;
                rdfs:seeAlso <http://www.ietf.org/rfc/rfc1766.txt> ;
                rdfs:label "RFC 1766"@en .


dcterms:RFC3066 rdfs:label "RFC 3066"@en ;
                rdfs:isDefinedBy dcterms: ;
                dcterms:description "RFC 3066 has been obsoleted by RFC 4646."@en ;
                rdfs:comment "The set of tags constructed according to RFC 3066 for the identification of languages."@en ;
                rdfs:seeAlso <http://www.ietf.org/rfc/rfc3066.txt> ;
                dcterms:hasVersion <http://dublincore.org/usage/terms/history/#RFC3066-002> .


dcterms:RFC4646 dcterms:description "RFC 4646 obsoletes RFC 3066."@en ;
                dcterms:hasVersion <http://dublincore.org/usage/terms/history/#RFC4646-001> ;
                rdfs:seeAlso <http://www.ietf.org/rfc/rfc4646.txt> ;
                rdfs:isDefinedBy dcterms: ;
                rdfs:label "RFC 4646"@en ;
                rdfs:comment "The set of tags constructed according to RFC 4646 for the identification of languages."@en .


dcterms:RFC5646 rdfs:seeAlso <http://www.ietf.org/rfc/rfc5646.txt> ;
                dcterms:hasVersion <http://dublincore.org/usage/terms/history/#RFC5646-001> ;
                rdfs:comment "The set of tags constructed according to RFC 5646 for the identification of languages."@en ;
                rdfs:label "RFC 5646"@en ;
                dcterms:description "RFC 5646 obsoletes RFC 4646."@en ;
                rdfs:isDefinedBy dcterms: .


dcterms:RightsStatement rdfs:label "Rights Statement"@en ;
                        rdfs:isDefinedBy dcterms: ;
                        rdfs:comment "A statement about the intellectual property rights (IPR) held in or over a Resource, a legal document giving official permission to do something with a resource, or a statement about access rights."@en ;
                        dcterms:hasVersion <http://dublincore.org/usage/terms/history/#RightsStatement-001> .


dcterms:SizeOrDuration rdfs:label "Size or Duration"@en ;
                       dcterms:hasVersion <http://dublincore.org/usage/terms/history/#SizeOrDuration-001> ;
                       dcterms:description "Examples include a number of pages, a specification of length, width, and breadth, or a period in hours, minutes, and seconds."@en ;
                       rdfs:comment "A dimension or extent, or a time taken to play or execute."@en ;
                       rdfs:isDefinedBy dcterms: .


dcterms:Standard rdfs:comment "A basis for comparison; a reference point against which other things can be evaluated."@en ;
                 rdfs:label "Standard"@en ;
                 rdfs:isDefinedBy dcterms: ;
                 dcterms:hasVersion <http://dublincore.org/usage/terms/history/#Standard-001> .


dcterms:URI rdfs:comment "The set of identifiers constructed according to the generic syntax for Uniform Resource Identifiers as specified by the Internet Engineering Task Force."@en ;
            rdfs:isDefinedBy dcterms: ;
            rdfs:seeAlso <http://www.ietf.org/rfc/rfc3986.txt> ;
            dcterms:hasVersion <http://dublincore.org/usage/terms/history/#URI-003> ;
            rdfs:label "URI"@en .


dcterms:W3CDTF rdfs:label "W3C-DTF"@en ;
               rdfs:comment "The set of dates and times constructed according to the W3C Date and Time Formats Specification."@en ;
               rdfs:isDefinedBy dcterms: ;
               dcterms:hasVersion <http://dublincore.org/usage/terms/history/#W3CDTF-003> ;
               rdfs:seeAlso <http://www.w3.org/TR/NOTE-datetime> .


dcterms:abstract rdfs:label "Abstract"@en ;
                 dcterms:hasVersion <http://dublincore.org/usage/terms/history/#abstract-003> ;
                 rdfs:isDefinedBy dcterms: ;
                 rdfs:comment "A summary of the resource."@en .


dcterms:accessRights dcterms:description "Access Rights may include information regarding access or restrictions based on privacy, security, or other policies."@en ;
                     rdfs:comment "Information about who can access the resource or an indication of its security status."@en ;
                     rdfs:label "Access Rights"@en ;
                     dcterms:hasVersion <http://dublincore.org/usage/terms/history/#accessRights-002> ;
                     rdfs:isDefinedBy dcterms: .


dcterms:accrualMethod rdfs:label "Accrual Method"@en ;
                      dcterms:hasVersion <http://dublincore.org/usage/terms/history/#accrualMethod-003> ;
                      rdfs:comment "The method by which items are added to a collection."@en ;
                      rdfs:isDefinedBy dcterms: .


dcterms:accrualPeriodicity rdfs:label "Accrual Periodicity"@en ;
                           dcterms:hasVersion <http://dublincore.org/usage/terms/history/#accrualPeriodicity-003> ;
                           rdfs:comment "The frequency with which items are added to a collection."@en ;
                           rdfs:isDefinedBy dcterms: .


dcterms:accrualPolicy rdfs:isDefinedBy dcterms: ;
                      dcterms:hasVersion <http://dublincore.org/usage/terms/history/#accrualPolicy-003> ;
                      rdfs:comment "The policy governing the addition of items to a collection."@en ;
                      rdfs:label "Accrual Policy"@en .


dcterms:alternative rdfs:comment "An alternative name for the resource."@en ;
                    rdfs:isDefinedBy dcterms: ;
                    dcterms:hasVersion <http://dublincore.org/usage/terms/history/#alternative-003> ;
                    dcterms:description "The distinction between titles and alternative titles is application-specific."@en ;
                    rdfs:label "Alternative Title"@en .


dcterms:audience rdfs:comment "A class of entity for whom the resource is intended or useful."@en ;
                 dcterms:hasVersion <http://dublincore.org/usage/terms/history/#audience-003> ;
                 rdfs:label "Audience"@en ;
                 rdfs:isDefinedBy dcterms: .


dcterms:available rdfs:isDefinedBy dcterms: ;
                  rdfs:comment "Date (often a range) that the resource became or will become available."@en ;
                  rdfs:label "Date Available"@en ;
                  dcterms:hasVersion <http://dublincore.org/usage/terms/history/#available-003> .


dcterms:bibliographicCitation dcterms:description "Recommended practice is to include sufficient bibliographic detail to identify the resource as unambiguously as possible."@en ;
                              rdfs:label "Bibliographic Citation"@en ;
                              dcterms:hasVersion <http://dublincore.org/usage/terms/history/#bibliographicCitation-002> ;
                              rdfs:comment "A bibliographic reference for the resource."@en ;
                              rdfs:isDefinedBy dcterms: .


dcterms:conformsTo rdfs:isDefinedBy dcterms: ;
                   rdfs:label "Conforms To"@en ;
                   rdfs:comment "An established standard to which the described resource conforms."@en ;
                   dcterms:hasVersion <http://dublincore.org/usage/terms/history/#conformsTo-003> .


dcterms:contributor rdfs:comment "An entity responsible for making contributions to the resource."@en ;
                    rdfs:isDefinedBy dcterms: ;
                    dcterms:description "Examples of a Contributor include a person, an organization, or a service."@en ;
                    dcterms:hasVersion <http://dublincore.org/usage/terms/history/#contributorT-001> ;
                    rdfs:label "Contributor"@en .


dcterms:coverage rdfs:isDefinedBy dcterms: ;
                 dcterms:hasVersion <http://dublincore.org/usage/terms/history/#coverageT-001> ;
                 rdfs:label "Coverage"@en ;
                 dcterms:description "Spatial topic and spatial applicability may be a named place or a location specified by its geographic coordinates. Temporal topic may be a named period, date, or date range. A jurisdiction may be a named administrative entity or a geographic place to which the resource applies. Recommended best practice is to use a controlled vocabulary such as the Thesaurus of Geographic Names [TGN]. Where appropriate, named places or time periods can be used in preference to numeric identifiers such as sets of coordinates or date ranges."@en ;
                 rdfs:comment "The spatial or temporal topic of the resource, the spatial applicability of the resource, or the jurisdiction under which the resource is relevant."@en .


dcterms:created rdfs:isDefinedBy dcterms: ;
                rdfs:comment "Date of creation of the resource."@en ;
                dcterms:hasVersion <http://dublincore.org/usage/terms/history/#created-003> ;
                rdfs:label "Date Created"@en .


dcterms:creator rdfs:comment "An entity primarily responsible for making the resource."@en ;
                dcterms:hasVersion <http://dublincore.org/usage/terms/history/#creatorT-002> ;
                rdfs:isDefinedBy dcterms: ;
                rdfs:label "Creator"@en ;
                dcterms:description "Examples of a Creator include a person, an organization, or a service."@en .


dcterms:date rdfs:isDefinedBy dcterms: ;
             dcterms:hasVersion <http://dublincore.org/usage/terms/history/#dateT-001> ;
             rdfs:comment "A point or period of time associated with an event in the lifecycle of the resource."@en ;
             dcterms:description "Date may be used to express temporal information at any level of granularity.  Recommended best practice is to use an encoding scheme, such as the W3CDTF profile of ISO 8601 [W3CDTF]."@en ;
             rdfs:label "Date"@en .


dcterms:dateAccepted dcterms:hasVersion <http://dublincore.org/usage/terms/history/#dateAccepted-002> ;
                     dcterms:description "Examples of resources to which a Date Accepted may be relevant are a thesis (accepted by a university department) or an article (accepted by a journal)."@en ;
                     rdfs:label "Date Accepted"@en ;
                     rdfs:comment "Date of acceptance of the resource."@en ;
                     rdfs:isDefinedBy dcterms: .


dcterms:dateCopyrighted rdfs:isDefinedBy dcterms: ;
                        rdfs:label "Date Copyrighted"@en ;
                        rdfs:comment "Date of copyright."@en ;
                        dcterms:hasVersion <http://dublincore.org/usage/terms/history/#dateCopyrighted-002> .


dcterms:dateSubmitted rdfs:comment "Date of submission of the resource."@en ;
                      dcterms:description "Examples of resources to which a Date Submitted may be relevant are a thesis (submitted to a university department) or an article (submitted to a journal)."@en ;
                      rdfs:label "Date Submitted"@en ;
                      dcterms:hasVersion <http://dublincore.org/usage/terms/history/#dateSubmitted-002> ;
                      rdfs:isDefinedBy dcterms: .


dcterms:description rdfs:label "Description"@en ;
                    rdfs:isDefinedBy dcterms: ;
                    dcterms:hasVersion <http://dublincore.org/usage/terms/history/#descriptionT-001> ;
                    rdfs:comment "An account of the resource."@en ;
                    dcterms:description "Description may include but is not limited to: an abstract, a table of contents, a graphical representation, or a free-text account of the resource."@en .


dcterms:educationLevel rdfs:isDefinedBy dcterms: ;
                       rdfs:label "Audience Education Level"@en ;
                       rdfs:comment "A class of entity, defined in terms of progression through an educational or training context, for which the described resource is intended."@en ;
                       dcterms:hasVersion <http://dublincore.org/usage/terms/history/#educationLevel-002> .


dcterms:extent rdfs:isDefinedBy dcterms: ;
               rdfs:comment "The size or duration of the resource."@en ;
               rdfs:label "Extent"@en ;
               dcterms:hasVersion <http://dublincore.org/usage/terms/history/#extent-003> .


dcterms:format dcterms:hasVersion <http://dublincore.org/usage/terms/history/#formatT-001> ;
               rdfs:comment "The file format, physical medium, or dimensions of the resource."@en ;
               dcterms:description "Examples of dimensions include size and duration. Recommended best practice is to use a controlled vocabulary such as the list of Internet Media Types [MIME]."@en ;
               rdfs:isDefinedBy dcterms: ;
               rdfs:label "Format"@en .


dcterms:hasFormat rdfs:isDefinedBy dcterms: ;
                  <http://www.w3.org/2004/02/skos/core#note> "This term is intended to be used with non-literal values as defined in the DCMI Abstract Model (http://dublincore.org/documents/abstract-model/).  As of December 2007, the DCMI Usage Board is seeking a way to express this intention with a formal range declaration."@en ;
                  dcterms:hasVersion <http://dublincore.org/usage/terms/history/#hasFormat-003> ;
                  rdfs:label "Has Format"@en ;
                  rdfs:comment "A related resource that is substantially the same as the pre-existing described resource, but in another format."@en .


dcterms:hasPart rdfs:isDefinedBy dcterms: ;
                <http://www.w3.org/2004/02/skos/core#note> "This term is intended to be used with non-literal values as defined in the DCMI Abstract Model (http://dublincore.org/documents/abstract-model/).  As of December 2007, the DCMI Usage Board is seeking a way to express this intention with a formal range declaration."@en ;
                rdfs:label "Has Part"@en ;
                rdfs:comment "A related resource that is included either physically or logically in the described resource."@en ;
                dcterms:hasVersion <http://dublincore.org/usage/terms/history/#hasPart-003> .


dcterms:hasVersion dcterms:hasVersion <http://dublincore.org/usage/terms/history/#hasVersion-003> ;
                   rdfs:isDefinedBy dcterms: ;
                   rdfs:comment "A related resource that is a version, edition, or adaptation of the described resource."@en ;
                   <http://www.w3.org/2004/02/skos/core#note> "This term is intended to be used with non-literal values as defined in the DCMI Abstract Model (http://dublincore.org/documents/abstract-model/).  As of December 2007, the DCMI Usage Board is seeking a way to express this intention with a formal range declaration."@en ;
                   rdfs:label "Has Version"@en .


dcterms:identifier dcterms:hasVersion <http://dublincore.org/usage/terms/history/#identifierT-001> ;
                   rdfs:isDefinedBy dcterms: ;
                   dcterms:description "Recommended best practice is to identify the resource by means of a string conforming to a formal identification system. "@en ;
                   rdfs:comment "An unambiguous reference to the resource within a given context."@en ;
                   rdfs:label "Identifier"@en .


dcterms:instructionalMethod dcterms:description "Instructional Method will typically include ways of presenting instructional materials or conducting instructional activities, patterns of learner-to-learner and learner-to-instructor interactions, and mechanisms by which group and individual levels of learning are measured.  Instructional methods include all aspects of the instruction and learning processes from planning and implementation through evaluation and feedback."@en ;
                            rdfs:label "Instructional Method"@en ;
                            rdfs:comment "A process, used to engender knowledge, attitudes and skills, that the described resource is designed to support."@en ;
                            dcterms:hasVersion <http://dublincore.org/usage/terms/history/#instructionalMethod-002> ;
                            rdfs:isDefinedBy dcterms: .


dcterms:isFormatOf dcterms:hasVersion <http://dublincore.org/usage/terms/history/#isFormatOf-003> ;
                   rdfs:comment "A related resource that is substantially the same as the described resource, but in another format."@en ;
                   <http://www.w3.org/2004/02/skos/core#note> "This term is intended to be used with non-literal values as defined in the DCMI Abstract Model (http://dublincore.org/documents/abstract-model/).  As of December 2007, the DCMI Usage Board is seeking a way to express this intention with a formal range declaration."@en ;
                   rdfs:isDefinedBy dcterms: ;
                   rdfs:label "Is Format Of"@en .


dcterms:isPartOf rdfs:label "Is Part Of"@en ;
                 dcterms:hasVersion <http://dublincore.org/usage/terms/history/#isPartOf-003> ;
                 <http://www.w3.org/2004/02/skos/core#note> "This term is intended to be used with non-literal values as defined in the DCMI Abstract Model (http://dublincore.org/documents/abstract-model/).  As of December 2007, the DCMI Usage Board is seeking a way to express this intention with a formal range declaration."@en ;
                 rdfs:isDefinedBy dcterms: ;
                 rdfs:comment "A related resource in which the described resource is physically or logically included."@en .


dcterms:isReferencedBy rdfs:label "Is Referenced By"@en ;
                       rdfs:comment "A related resource that references, cites, or otherwise points to the described resource."@en ;
                       <http://www.w3.org/2004/02/skos/core#note> "This term is intended to be used with non-literal values as defined in the DCMI Abstract Model (http://dublincore.org/documents/abstract-model/).  As of December 2007, the DCMI Usage Board is seeking a way to express this intention with a formal range declaration."@en ;
                       rdfs:isDefinedBy dcterms: ;
                       dcterms:hasVersion <http://dublincore.org/usage/terms/history/#isReferencedBy-003> .


dcterms:isReplacedBy rdfs:isDefinedBy dcterms: ;
                     rdfs:label "Is Replaced By"@en ;
                     rdfs:comment "A related resource that supplants, displaces, or supersedes the described resource."@en ;
                     <http://www.w3.org/2004/02/skos/core#note> "This term is intended to be used with non-literal values as defined in the DCMI Abstract Model (http://dublincore.org/documents/abstract-model/).  As of December 2007, the DCMI Usage Board is seeking a way to express this intention with a formal range declaration."@en ;
                     dcterms:hasVersion <http://dublincore.org/usage/terms/history/#isReplacedBy-003> .


dcterms:isRequiredBy rdfs:isDefinedBy dcterms: ;
                     <http://www.w3.org/2004/02/skos/core#note> "This term is intended to be used with non-literal values as defined in the DCMI Abstract Model (http://dublincore.org/documents/abstract-model/).  As of December 2007, the DCMI Usage Board is seeking a way to express this intention with a formal range declaration."@en ;
                     rdfs:label "Is Required By"@en ;
                     dcterms:hasVersion <http://dublincore.org/usage/terms/history/#isRequiredBy-003> ;
                     rdfs:comment "A related resource that requires the described resource to support its function, delivery, or coherence."@en .


dcterms:isVersionOf rdfs:label "Is Version Of"@en ;
                    rdfs:comment "A related resource of which the described resource is a version, edition, or adaptation."@en ;
                    rdfs:isDefinedBy dcterms: ;
                    <http://www.w3.org/2004/02/skos/core#note> "This term is intended to be used with non-literal values as defined in the DCMI Abstract Model (http://dublincore.org/documents/abstract-model/).  As of December 2007, the DCMI Usage Board is seeking a way to express this intention with a formal range declaration."@en ;
                    dcterms:hasVersion <http://dublincore.org/usage/terms/history/#isVersionOf-003> ;
                    dcterms:description "Changes in version imply substantive changes in content rather than differences in format."@en .


dcterms:issued rdfs:comment "Date of formal issuance (e.g., publication) of the resource."@en ;
               rdfs:isDefinedBy dcterms: ;
               dcterms:hasVersion <http://dublincore.org/usage/terms/history/#issued-003> ;
               rdfs:label "Date Issued"@en .


dcterms:language rdfs:label "Language"@en ;
                 dcterms:hasVersion <http://dublincore.org/usage/terms/history/#languageT-001> ;
                 rdfs:isDefinedBy dcterms: ;
                 dcterms:description "Recommended best practice is to use a controlled vocabulary such as RFC 4646 [RFC4646]."@en ;
                 rdfs:comment "A language of the resource."@en .


dcterms:license rdfs:label "License"@en ;
                rdfs:comment "A legal document giving official permission to do something with the resource."@en ;
                dcterms:hasVersion <http://dublincore.org/usage/terms/history/#license-002> ;
                rdfs:isDefinedBy dcterms: .


dcterms:mediator dcterms:description "In an educational context, a mediator might be a parent, teacher, teaching assistant, or care-giver."@en ;
                 rdfs:comment "An entity that mediates access to the resource and for whom the resource is intended or useful."@en ;
                 dcterms:hasVersion <http://dublincore.org/usage/terms/history/#mediator-003> ;
                 rdfs:isDefinedBy dcterms: ;
                 rdfs:label "Mediator"@en .


dcterms:medium rdfs:isDefinedBy dcterms: ;
               rdfs:label "Medium"@en ;
               rdfs:comment "The material or physical carrier of the resource."@en ;
               dcterms:hasVersion <http://dublincore.org/usage/terms/history/#medium-003> .


dcterms:modified rdfs:isDefinedBy dcterms: ;
                 rdfs:label "Date Modified"@en ;
                 dcterms:hasVersion <http://dublincore.org/usage/terms/history/#modified-003> ;
                 rdfs:comment "Date on which the resource was changed."@en .


dcterms:provenance rdfs:comment "A statement of any changes in ownership and custody of the resource since its creation that are significant for its authenticity, integrity, and interpretation."@en ;
                   rdfs:isDefinedBy dcterms: ;
                   dcterms:description "The statement may include a description of any changes successive custodians made to the resource."@en ;
                   dcterms:hasVersion <http://dublincore.org/usage/terms/history/#provenance-002> ;
                   rdfs:label "Provenance"@en .


dcterms:publisher rdfs:label "Publisher"@en ;
                  dcterms:hasVersion <http://dublincore.org/usage/terms/history/#publisherT-001> ;
                  dcterms:description "Examples of a Publisher include a person, an organization, or a service."@en ;
                  rdfs:isDefinedBy dcterms: ;
                  rdfs:comment "An entity responsible for making the resource available."@en .


dcterms:references rdfs:comment "A related resource that is referenced, cited, or otherwise pointed to by the described resource."@en ;
                   rdfs:label "References"@en ;
                   dcterms:hasVersion <http://dublincore.org/usage/terms/history/#references-003> ;
                   rdfs:isDefinedBy dcterms: ;
                   <http://www.w3.org/2004/02/skos/core#note> "This term is intended to be used with non-literal values as defined in the DCMI Abstract Model (http://dublincore.org/documents/abstract-model/).  As of December 2007, the DCMI Usage Board is seeking a way to express this intention with a formal range declaration."@en .


dcterms:relation <http://www.w3.org/2004/02/skos/core#note> "This term is intended to be used with non-literal values as defined in the DCMI Abstract Model (http://dublincore.org/documents/abstract-model/).  As of December 2007, the DCMI Usage Board is seeking a way to express this intention with a formal range declaration."@en ;
                 rdfs:isDefinedBy dcterms: ;
                 dcterms:hasVersion <http://dublincore.org/usage/terms/history/#relationT-001> ;
                 dcterms:description "Recommended best practice is to identify the related resource by means of a string conforming to a formal identification system. "@en ;
                 rdfs:label "Relation"@en ;
                 rdfs:comment "A related resource."@en .


dcterms:replaces <http://www.w3.org/2004/02/skos/core#note> "This term is intended to be used with non-literal values as defined in the DCMI Abstract Model (http://dublincore.org/documents/abstract-model/).  As of December 2007, the DCMI Usage Board is seeking a way to express this intention with a formal range declaration."@en ;
                 rdfs:label "Replaces"@en ;
                 dcterms:hasVersion <http://dublincore.org/usage/terms/history/#replaces-003> ;
                 rdfs:comment "A related resource that is supplanted, displaced, or superseded by the described resource."@en ;
                 rdfs:isDefinedBy dcterms: .


dcterms:requires dcterms:hasVersion <http://dublincore.org/usage/terms/history/#requires-003> ;
                 rdfs:label "Requires"@en ;
                 rdfs:comment "A related resource that is required by the described resource to support its function, delivery, or coherence."@en ;
                 rdfs:isDefinedBy dcterms: ;
                 <http://www.w3.org/2004/02/skos/core#note> "This term is intended to be used with non-literal values as defined in the DCMI Abstract Model (http://dublincore.org/documents/abstract-model/).  As of December 2007, the DCMI Usage Board is seeking a way to express this intention with a formal range declaration."@en .


dcterms:rights rdfs:isDefinedBy dcterms: ;
               rdfs:label "Rights"@en ;
               rdfs:comment "Information about rights held in and over the resource."@en ;
               dcterms:hasVersion <http://dublincore.org/usage/terms/history/#rightsT-001> ;
               dcterms:description "Typically, rights information includes a statement about various property rights associated with the resource, including intellectual property rights."@en .


dcterms:rightsHolder rdfs:isDefinedBy dcterms: ;
                     dcterms:hasVersion <http://dublincore.org/usage/terms/history/#rightsHolder-002> ;
                     rdfs:comment "A person or organization owning or managing rights over the resource."@en ;
                     rdfs:label "Rights Holder"@en .


dcterms:source rdfs:label "Source"@en ;
               <http://www.w3.org/2004/02/skos/core#note> "This term is intended to be used with non-literal values as defined in the DCMI Abstract Model (http://dublincore.org/documents/abstract-model/).  As of December 2007, the DCMI Usage Board is seeking a way to express this intention with a formal range declaration."@en ;
               rdfs:isDefinedBy dcterms: ;
               dcterms:hasVersion <http://dublincore.org/usage/terms/history/#sourceT-001> ;
               rdfs:comment "A related resource from which the described resource is derived."@en ;
               dcterms:description "The described resource may be derived from the related resource in whole or in part. Recommended best practice is to identify the related resource by means of a string conforming to a formal identification system."@en .


dcterms:spatial rdfs:label "Spatial Coverage"@en ;
                rdfs:isDefinedBy dcterms: ;
                rdfs:comment "Spatial characteristics of the resource."@en ;
                dcterms:hasVersion <http://dublincore.org/usage/terms/history/#spatial-003> .


dcterms:subject dcterms:hasVersion <http://dublincore.org/usage/terms/history/#subjectT-002> ;
                <http://www.w3.org/2004/02/skos/core#note> "This term is intended to be used with non-literal values as defined in the DCMI Abstract Model (http://dublincore.org/documents/abstract-model/).  As of December 2007, the DCMI Usage Board is seeking a way to express this intention with a formal range declaration."@en ;
                rdfs:label "Subject"@en ;
                rdfs:comment "The topic of the resource."@en ;
                dcterms:description "Typically, the subject will be represented using keywords, key phrases, or classification codes. Recommended best practice is to use a controlled vocabulary."@en ;
                rdfs:isDefinedBy dcterms: .


dcterms:tableOfContents rdfs:comment "A list of subunits of the resource."@en ;
                        rdfs:isDefinedBy dcterms: ;
                        rdfs:label "Table Of Contents"@en ;
                        dcterms:hasVersion <http://dublincore.org/usage/terms/history/#tableOfContents-003> .


dcterms:temporal rdfs:label "Temporal Coverage"@en ;
                 dcterms:hasVersion <http://dublincore.org/usage/terms/history/#temporal-003> ;
                 rdfs:comment "Temporal characteristics of the resource."@en ;
                 rdfs:isDefinedBy dcterms: .


dcterms:title rdfs:label "Title"@en ;
              rdfs:comment "A name given to the resource."@en ;
              dcterms:hasVersion <http://dublincore.org/usage/terms/history/#titleT-002> ;
              rdfs:isDefinedBy dcterms: .


dcterms:type rdfs:isDefinedBy dcterms: ;
             dcterms:description "Recommended best practice is to use a controlled vocabulary such as the DCMI Type Vocabulary [DCMITYPE]. To describe the file format, physical medium, or dimensions of the resource, use the Format element."@en ;
             rdfs:comment "The nature or genre of the resource."@en ;
             rdfs:label "Type"@en ;
             dcterms:hasVersion <http://dublincore.org/usage/terms/history/#typeT-001> .


dcterms:valid rdfs:comment "Date (often a range) of validity of a resource."@en ;
              rdfs:label "Date Valid"@en ;
              dcterms:hasVersion <http://dublincore.org/usage/terms/history/#valid-003> ;
              rdfs:isDefinedBy dcterms: .


mo:derived_from vs:term_status "testing" ;
                rdfs:label "derived from" ;
                rdfs:comment "A related signal from which the described signal is derived." ;
                rdfs:isDefinedBy <http://purl.org/ontology/mo/> ;
                mo:level "1" .


mo:genre rdfs:label "genre" ;
         rdfs:comment """
        Associates an event (like a performance or a recording) to a particular musical genre.
        Further version of this property may also include works and scores in the domain.
    """ ;
         vs:term_status "stable" ;
         rdfs:isDefinedBy <http://purl.org/ontology/mo/> ;
         mo:level "2" .


###  Generated by the OWL API (version 4.2.8.20170104-2310) https://github.com/owlcs/owlapi
